@prefix delleg: <http://parliament.uk/ontologies/delegated-legislation/> . 
@prefix xsd: <http://www.w3.org/2001/XMLSchema#> . 
@prefix rdf: <http://www.w3.org/1999/02/22-rdf-syntax-ns#> .
@prefix dcterms: <http://purl.org/dc/terms/> .
@prefix owl:     <http://www.w3.org/2002/07/owl#> .
@prefix rdfs:    <http://www.w3.org/2000/01/rdf-schema#> .
@prefix foaf:	<http://xmlns.com/foaf/0.1/> .

<http://parliament.uk/ontologies/delegated-legislation/> 
    rdf:type owl:Ontology ;
    dcterms:title "Delegated legislation ontology"@en ;
    dcterms:created "2023-02-01"^^xsd:date ;
	dcterms:rights "Open Parliament Licence v3.0"@en ;
    dcterms:description "A model describing delegated legislation as expressions of works."@en ;
	foaf:depiction <https://ukparliament.github.io/ontologies/delegated-legislation/delegated-legislation.svg> ;
	foaf:maker
		[ foaf:name "David Beamish" ],
		[ foaf:name "Robert Brook"; foaf:homepage <https://robert-brook.com/> ],
		[ foaf:name "Nerys Davies" ],
		[ foaf:name "Jack Dent" ],
		[ foaf:name "Samu Lang" ],
		[ foaf:name "Lucinda Maer" ],
		[ foaf:name "Silver Oliver" ],
		[ foaf:name "Claire Searle" ],
		[ foaf:name "John Sheridan" ],
		[ foaf:name "Michael Smethurst"; foaf:homepage <http://smethur.st/> ],
	    [ foaf:name "Anya Somerville" ],
	    [ foaf:name "Jayne Sunley" ],
	    [ foaf:name "Matthew Waddington" ],
		[ foaf:name "Jane White" ].


#######  Classes #####

delleg:PublishedDraftUnderEUWA2018Work rdf:type owl:Class ;
	rdfs:label "Published draft under the European Union (Withdrawal) Act 2018 work"@en ;
	rdfs:comment "A draft published under the duties laid out in paragraph 14 of schedule 8 of the European Union (Withdrawal) Act 2018. A Minister has a duty to publish such a draft 28 joint sitting days before the laying of an instrument intending to amend or revoke subordinate legislation under section 2(2) of the European Communities Act 1972, including subordinate legislation implementing EU directives."@en ;
	rdfs:isDefinedBy <http://parliament.uk/ontologies/delegated-legislation/> .
	
delleg:ProposedDraftRemedialOrderWork rdf:type owl:Class ;
	rdfs:label "Proposed draft remedial order work"@en ;
	rdfs:comment "A proposal for a draft remedial order. Under paragraph 3(1) of schedule 2 of the Human Rights Act 1998, the Minister has a duty to lay before Parliament 'a document which contains a draft of the proposed order'. This document must lay before Parliament for a period of 60 sitting days, beginning with the day on which it was laid."@en ;
	rdfs:isDefinedBy <http://parliament.uk/ontologies/delegated-legislation/> .

delleg:ProposedNegativeStatutoryInstrumentWork rdf:type owl:Class ;
	rdfs:label "Proposed negative statutory instrument work"@en ;
	rdfs:comment "A regulation made under a power or powers set out in clause 7, 8 or 9 of the European Union (Withdrawal) Act 2018, or under schedule 5 of the Future Relationship Act 2020, which government ministers propose be laid under the negative procedure. Sifting committees of either House may recommend that any subsequent statutory instrument or instruments be laid under the affirmative procedure."@en ;
	rdfs:isDefinedBy <http://parliament.uk/ontologies/delegated-legislation/> .

delleg:DraftStatutoryInstrumentWork rdf:type owl:Class ;
	rdfs:label "Draft statutory instrument work"@en ;
	rdfs:comment "An instrument laid in draft before Parliament subject to either a negative, affirmative or super affirmative procedure. An instrument under the draft negative procedure may be made into law, if not objected to within the scrutiny period. An instrument under the draft affirmative procedure may be made into law, having been approved by Parliament. An instrument under the draft super affirmative procedure may be made into law, having been approved by Parliament within the approval period."@en ;
	rdfs:isDefinedBy <http://parliament.uk/ontologies/delegated-legislation/> .

delleg:MadeStatutoryInstrumentWork rdf:type owl:Class ;
	rdfs:label "Made statutory instrument work"@en ;
	rdfs:comment "Statutory instruments as signed into law. Made statutory instruments may result from a draft laid before Parliament, or may be laid as made, or may not be laid if the enabling legislation does not set out a duty to lay. Made statutory instruments laid before Parliament are subject to a negative, affirmative or super affirmative procedure, or none. An instrument under the made negative procedure remains law, unless objected to within the scrutiny period. An instrument under the made affirmative procedure or made super affirmative procedure remains law, if approved by Parliament within the approval period."@en ;
	rdfs:isDefinedBy <http://parliament.uk/ontologies/delegated-legislation/> .
	
delleg:PaperExpression rdf:type owl:Class ;
	rdfs:label "Paper expression"@en ;
	rdfs:comment "A paper made available to a House, being an expression of a paper work."@en ;
	rdfs:isDefinedBy <http://parliament.uk/ontologies/delegated-legislation/> .
	
delleg:PublishedDraftUnderEUWA2018Expression rdf:type owl:Class ;
	rdfs:subClassOf delleg:PaperExpression ;
	rdfs:label "Published draft under the European Union (Withdrawal) Act 2018 expression"@en ;
	rdfs:comment "A published draft laid under the European Union (Withdrawal) Act 2018, being an expression of a published draft under the European Union (Withdrawal) Act 2018 work."@en ;
	rdfs:isDefinedBy <http://parliament.uk/ontologies/delegated-legislation/> .
	
delleg:ProposedDraftRemedialOrderExpression rdf:type owl:Class ;
	rdfs:subClassOf delleg:PaperExpression ;
	rdfs:label "Proposed draft remedial order expression"@en ;
	rdfs:comment "A proposed draft remedial order, being an expression of a proposed draft remedial order work."@en ;
	rdfs:isDefinedBy <http://parliament.uk/ontologies/delegated-legislation/> .
	
delleg:ProposedNegativeStatutoryInstrumentExpression rdf:type owl:Class ;
	rdfs:subClassOf delleg:PaperExpression ;
	rdfs:label "Proposed negative statutory instrument expression"@en ;
	rdfs:comment "A proposed negative statutory instrument, being an expression of a proposed negative statutory instrument work."@en ;
	rdfs:isDefinedBy <http://parliament.uk/ontologies/delegated-legislation/> .

delleg:DraftStatutoryInstrumentExpression rdf:type owl:Class ;
	rdfs:subClassOf delleg:PaperExpression ;
	rdfs:label "Draft statutory instrument expression"@en ;
	rdfs:comment "A draft statutory instrument, being an expression of a draft statutory instrument work."@en ;
	rdfs:isDefinedBy <http://parliament.uk/ontologies/delegated-legislation/> .

delleg:MadeStatutoryInstrumentExpression rdf:type owl:Class ;
	rdfs:subClassOf delleg:PaperExpression ;
	rdfs:label "Made statutory instrument expression"@en ;
	rdfs:comment "A made statutory instrument, being an expression of a made statutory instrument work."@en ;
	rdfs:isDefinedBy <http://parliament.uk/ontologies/delegated-legislation/> .

							#edited to here

##### Object properties ####
	
delleg:publishedDraftUnderEUWA2018ExpressionOf rdf:type owl:ObjectProperty ;
	rdfs:label "Published draft under EUWA 2018 expression of"@en ;
	rdfs:comment "Relates a published draft under the European Union (Withdrawal) Act 2018 to the work it expresses. A work may have one or more expressions. An expression is of one work."@en ;
	rdfs:domain delleg:PublishedDraftUnderEUWA2018Expression ;
	rdfs:range delleg:PublishedDraftUnderEUWA2018Work ;
	rdfs:isDefinedBy <http://parliament.uk/ontologies/delegated-legislation/> .

delleg:proposedDraftRemedialOrderExpressionOf rdf:type owl:ObjectProperty ;
	rdfs:label "Proposed draft remedial order expression of"@en ;
	rdfs:comment "Relates a proposed draft remedial order to the work it expresses. A work may have one or more expressions. An expression is of one work."@en ;
	rdfs:domain delleg:ProposedDraftRemedialOrderExpression ;
	rdfs:range delleg:ProposedDraftRemedialOrderWork ;
	rdfs:isDefinedBy <http://parliament.uk/ontologies/delegated-legislation/> .

delleg:proposedNegativeStatutoryInstrumentExpressionOf rdf:type owl:ObjectProperty ;
	rdfs:label "Proposed negative statutory instrument expression of"@en ;
	rdfs:comment "Relates a proposed negative statutory instrument to the work it expresses. A work may have one or more expressions. An expression is of one work."@en ;
	rdfs:domain delleg:ProposedNegativeStatutoryInstrumentExpression ;
	rdfs:range delleg:ProposedNegativeStatutoryInstrumentWork ;
	rdfs:isDefinedBy <http://parliament.uk/ontologies/delegated-legislation/> .
	
delleg:draftStatutoryInstrumentExpressionOf rdf:type owl:ObjectProperty ;
	rdfs:label "Draft statutory instrument expression of"@en ;
	rdfs:comment "Relates a draft statutory instrument to the work it expresses. A work may have one or more expressions. An expression is of one work."@en ;
	rdfs:domain delleg:DraftStatutoryInstrumentExpression ;
	rdfs:range delleg:DraftStatutoryInstrumentWork ;
	rdfs:isDefinedBy <http://parliament.uk/ontologies/delegated-legislation/> .
	
delleg:madeStatutoryInstrumentExpressionOf rdf:type owl:ObjectProperty ;
	rdfs:label "Made statutory instrument expression of"@en ;
	rdfs:comment "Relates a made statutory instrument to the work it expresses. A work may have one or more expressions. An expression is of one work."@en ;
	rdfs:domain delleg:MadeStatutoryInstrumentExpression ;
	rdfs:range delleg:MadeStatutoryInstrumentWork ;
	rdfs:isDefinedBy <http://parliament.uk/ontologies/delegated-legislation/> .