@prefix pws: <http://parliament.uk/ontologies/written-statement/> . 
@prefix xsd: <http://www.w3.org/2001/XMLSchema#> . 
@prefix rdf: <http://www.w3.org/1999/02/22-rdf-syntax-ns#> .
@prefix dcterms: <http://purl.org/dc/terms/> .
@prefix owl:     <http://www.w3.org/2002/07/owl#> .
@prefix rdfs:    <http://www.w3.org/2000/01/rdf-schema#> .
@prefix foaf:	<http://xmlns.com/foaf/0.1/> .

<http://parliament.uk/ontologies/written-statement/> 
    rdf:type owl:Ontology ;
    dcterms:title "Written statement ontology"@en ;
    dcterms:created "2021-12-20"^^xsd:date ;
	dcterms:rights "Open Parliament Licence v3.0"@en ;
    dcterms:description "A model describing written statements made to Parliament as works and expressions of those works."@en ;
	foaf:depiction <https://ukparliament.github.io/ontologies/written-statement/written-statement.svg> ;
	foaf:maker
		[ foaf:name "Emma Bainbridge" ],
		[ foaf:name "Robert Brook"; foaf:homepage <https://robert-brook.com/> ],
		[ foaf:name "Ned Morrell" ],
		[ foaf:name "Michael Smethurst"; foaf:homepage <http://smethur.st/> ],
	    [ foaf:name "Anya Somerville" ] .


#######  Classes #####

pws:WrittenStatementWork rdf:type owl:Class ;
	rdfs:label "Written statement work"@en ;
	rdfs:comment "A written statement made to Parliament as realised in an expression made to a House."@en ;
	rdfs:isDefinedBy <http://parliament.uk/ontologies/written-statement/> .
	
pws:WrittenStatementExpression rdf:type owl:Class ;
	rdfs:label "Written statement expression"@en ;
	rdfs:comment "The expression of a written statement as made to a House."@en ;
	rdfs:isDefinedBy <http://parliament.uk/ontologies/written-statement/> .
	
				

#######  Object properties ##### 
	
pws:expressionOf rdf:type owl:ObjectProperty ;
	rdfs:label "Expression of"@en ;
	rdfs:comment "Relates a written statement expression to the written statement work realised by that expression. A written statement work has one written statement expression when a statement is made to one House. A written statement work has two written statement expressions when a statement is made to both Houses. A written statement expression realises one written statement work."@en ;
	rdfs:domain pws:WrittenStatementExpression ;
	rdfs:range pws:WrittenStatementWork ;
	rdfs:isDefinedBy <http://parliament.uk/ontologies/written-statement/> .
	

					
##### Data properties ####	
	
pws:statementText rdf:type owl:DatatypeProperty ;
	rdfs:label "Statement text"@en ;
	rdfs:comment "Relates a written statement expression to the text of that expression."@en ;
	rdfs:domain pws:WrittenStatementExpression ;
	rdfs:range rdf:langString ;
	rdfs:isDefinedBy <http://parliament.uk/ontologies/written-statement/> .
	
pws:uin rdf:type owl:DatatypeProperty ;
	rdfs:label "UIN"@en ;
	rdfs:comment "Relates a written statement expression to the UIN of that expression. A UIN is an alphanumeric identifier."@en ;
	rdfs:domain pws:WrittenStatementExpression ;
	rdfs:range rdfs:Literal ;
	rdfs:isDefinedBy <http://parliament.uk/ontologies/written-statement/> .