@prefix making: <http://parliament.uk/ontologies/making/> . 
@prefix xsd: <http://www.w3.org/2001/XMLSchema#> . 
@prefix rdf: <http://www.w3.org/1999/02/22-rdf-syntax-ns#> .
@prefix dcterms: <http://purl.org/dc/terms/> .
@prefix owl:     <http://www.w3.org/2002/07/owl#> .
@prefix rdfs:    <http://www.w3.org/2000/01/rdf-schema#> .
@prefix foaf:	<http://xmlns.com/foaf/0.1/> .

<http://parliament.uk/ontologies/making/> 
    rdf:type owl:Ontology ;
    dcterms:title "Making ontology"@en ;
    dcterms:created "2023-03-17"^^xsd:date ;
	dcterms:rights "Open Parliament Licence v3.0"@en ;
    dcterms:description "A model describing the reporting to a House by a formal body."@en ;
	foaf:depiction <https://ukparliament.github.io/ontologies/making/making.svg> ;
	foaf:maker 
		[ foaf:name "Michael Smethurst"; foaf:homepage <http://smethur.st/> ],
		[ foaf:name "Anya Somerville" ].


#######  Classes #####
	
making:MakingAvailable rdf:type owl:Class ;
	rdfs:label "Making available"@en ;
	rdfs:comment "The act of making a thing available to a House or to a House by means of its Library."@en ;
	rdfs:isDefinedBy <http://parliament.uk/ontologies/making/> .

making:MadeAvailableThing rdf:type owl:Class ;
	rdfs:label "Made available thing"@en ;
	rdfs:comment "A thing made available to a House or to a House by means of its Library."@en ;
	rdfs:isDefinedBy <http://parliament.uk/ontologies/making/> .
	
making:Making rdf:type owl:Class ;
	rdfs:subClassOf making:MakingAvailable ;
	rdfs:label "Making"@en ;
	rdfs:comment "The act of making a written statement available to a House."@en ;
	rdfs:isDefinedBy <http://parliament.uk/ontologies/making/> .
	
making:WrittenStatementExpression rdf:type owl:Class ;
	rdfs:subClassOf making:MadeAvailableThing ;
	rdfs:label "Written statement expression"@en ;
	rdfs:comment "The expression of a written statement as made to a House."@en ;
	rdfs:isDefinedBy <http://parliament.uk/ontologies/making/> .
	
	

#######  Object properties ##### 
	
making:resultsIn rdf:type owl:ObjectProperty ;
	rdfs:label "Results in"@en ;
	rdfs:comment "Relates an act of making a written statement expression available to the written statement expression being made available. An act of making results in one written statement expression. A written statement expression results from one act of making."@en ;
	rdfs:domain making:Making ;
	rdfs:range making:WrittenStatementExpression ;
	rdfs:isDefinedBy <http://parliament.uk/ontologies/making/> .