@prefix pt: <http://parliament.uk/ontologies/tabling/> . 
@prefix xsd: <http://www.w3.org/2001/XMLSchema#> . 
@prefix rdf: <http://www.w3.org/1999/02/22-rdf-syntax-ns#> .
@prefix dcterms: <http://purl.org/dc/terms/> .
@prefix owl:     <http://www.w3.org/2002/07/owl#> .
@prefix rdfs:    <http://www.w3.org/2000/01/rdf-schema#> .

<http://parliament.uk/ontologies/tabling/> 
    rdf:type owl:Ontology ;
    dcterms:title "Tabling ontology"@en ;
    dcterms:created "01/12/2017"^^xsd:date ;
	dcterms:rights "Open Parliament Licence v3.0"@en ;
    dcterms:description "Ontology to describe the activity of members tabling parliamentary questions, motions, amendments and nominations."@en .


#######  Classes ##### 	

pt:Member rdf:type owl:Class ;
	rdfs:label "Member"@en ;
	rdfs:comment "A current or former Member of a House."@en ;
	rdf:isDefinedBy <http://parliament.uk/ontologies/tabling/> .

pt:Tabling rdf:type owl:Class ;
	rdfs:label "Tabling"@en ;
	rdfs:comment "The act of tabling a business item  into either the House of Commons or House of Lords. Note that not all tabling goes through the Table Offices."@en ;
	rdf:isDefinedBy <http://parliament.uk/ontologies/tabling/> .

pt:House rdf:type owl:Class ;
	rdfs:label "House"@en ;
	rdfs:comment "A parliamentary house e.g. the House of Lords."@en ;
	rdf:isDefinedBy <http://parliament.uk/ontologies/tabling/> .

pt:WrittenNotice rdf:type owl:Class ;
	rdfs:label "WrittenNotice"@en ;
	rdfs:comment "Official notice of an item of business."@en ;
	rdf:isDefinedBy <http://parliament.uk/ontologies/tabling/> .

pt:TableableThing rdf:type owl:Class ;
	rdfs:label "TableableThing"@en ;
	rdfs:comment "Any item of business which can be tabled. e.g. a motion, parliamentary question, amendment or nomination."@en ;
	rdf:isDefinedBy <http://parliament.uk/ontologies/tabling/> .

	
##### Object properties ####

pt:requests rdf:type owl:ObjectProperty ;
	rdfs:label "requests"@en ;
	rdfs:comment "Relates a member to an act of tabling."@en ;
	rdfs:domain pt:Member ;
	rdfs:range pt:Tabling ;
	rdf:isDefinedBy <http://parliament.uk/ontologies/tabling/> .
	
pt:givesNotice rdf:type owl:ObjectProperty ;
	rdfs:label "givesNotice"@en ;
	rdfs:comment "Relates an act of tabling to a written notice."@en ;
	rdfs:domain pt:Tabling ;
	rdfs:range pt:WrittenNotice ;
	rdf:isDefinedBy <http://parliament.uk/ontologies/tabling/> .
	
pt:tabledIn rdf:type owl:ObjectProperty ;
	rdfs:label "tabledIn"@en ;
	rdfs:comment "Relates an act of tabling to the House where the tabling happens."@en ;
	rdfs:domain pt:Tabling ;
	rdfs:range pt:House ;
	rdf:isDefinedBy <http://parliament.uk/ontologies/tabling/> .
	
pt:tables rdf:type owl:ObjectProperty ;
	rdfs:label "tables"@en ;
	rdfs:comment "Relates an act of tabling to the business item being tabled."@en ;
	rdfs:domain pt:Tabling ;
	rdfs:range pt:TableableThing ;
	rdf:isDefinedBy <http://parliament.uk/ontologies/tabling/> .
	

				
	
##### Data properties ####	

pt:tabledAt rdf:type owl:DatatypeProperty ;
	rdfs:label "tabledAt"@en ;
	rdfs:comment "Relates an act of tabling to the date time at which it happened."@en ;
	rdfs:domain pt:Tabling ;
	rdfs:range xsd:dateTime ;
	rdf:isDefinedBy <http://parliament.uk/ontologies/tabling/> .
	
pt:isInterestDeclared rdf:type owl:DatatypeProperty ;
	rdfs:label "isInterestDeclared"@en ;
	rdfs:comment "Relates an act of tabling to whether or not the Member doing the tabling declared an interest at the time it was tabled. Note that this is a boolean and does not describe or link to any definition of the nature of the interest."@en ;
	rdfs:domain pt:Tabling ;
	rdfs:range xsd:boolean ;
	rdf:isDefinedBy <http://parliament.uk/ontologies/tabling/> .	