@prefix report: <http://parliament.uk/ontologies/reporting/> . 
@prefix xsd: <http://www.w3.org/2001/XMLSchema#> . 
@prefix rdf: <http://www.w3.org/1999/02/22-rdf-syntax-ns#> .
@prefix dcterms: <http://purl.org/dc/terms/> .
@prefix owl:     <http://www.w3.org/2002/07/owl#> .
@prefix rdfs:    <http://www.w3.org/2000/01/rdf-schema#> .
@prefix foaf:	<http://xmlns.com/foaf/0.1/> .

<http://parliament.uk/ontologies/reporting/> 
    rdf:type owl:Ontology ;
    dcterms:title "Reporting ontology"@en ;
    dcterms:created "2023-02-07"^^xsd:date ;
	dcterms:rights "Open Parliament Licence v3.0"@en ;
    dcterms:description "A model describing the reporting to a House by a formal body."@en ;
	foaf:depiction <https://ukparliament.github.io/ontologies/reporting/reporting.svg> ;
	foaf:maker 
		[ foaf:name "Jayne Bosworth" ],
		[ foaf:name "Robert Brook"; foaf:homepage <https://robert-brook.com/> ],
		[ foaf:name "Gordon Clarke" ],
		[ foaf:name "Claire Searle" ],
		[ foaf:name "Michael Smethurst"; foaf:homepage <http://smethur.st/> ],
		[ foaf:name "Anya Somerville" ].


#######  Classes #####
	
report:MakingAvailable rdf:type owl:Class ;
	rdfs:label "Making available"@en ;
	rdfs:comment "The act of making a thing available to a House or to a House by means of its Library."@en ;
	rdfs:isDefinedBy <http://parliament.uk/ontologies/reporting/> .

report:MadeAvailableThing rdf:type owl:Class ;
	rdfs:label "Made available thing"@en ;
	rdfs:comment "A thing made available to a House or to a House by means of its Library."@en ;
	rdfs:isDefinedBy <http://parliament.uk/ontologies/reporting/> .
	
report:Reporting rdf:type owl:Class ;
	rdfs:subClassOf report:MakingAvailable ;
	rdfs:label "Reporting"@en ;
	rdfs:comment "The act of reporting to a House by a formal body."@en ;
	rdfs:isDefinedBy <http://parliament.uk/ontologies/reporting/> .

report:PaperExpression rdf:type owl:Class ;
	rdfs:label "Paper expression"@en ;
	rdfs:comment "A paper made available to a House, being an expression of a paper work."@en ;
	rdfs:isDefinedBy <http://parliament.uk/ontologies/reporting/> .
	
report:ReportedThing rdf:type owl:Class ;
	rdfs:subClassOf report:MadeAvailableThing ;
	rdfs:subClassOf report:PaperExpression ;
	rdfs:label "Reported thing"@en ;
	rdfs:comment "A thing having been reported to a House by a formal body, for example: the selection of a chair, a committee report, an evidence session or correspondence."@en ;
	rdfs:isDefinedBy <http://parliament.uk/ontologies/reporting/> .
	
	

#######  Object properties ##### 
	
report:resultsIn rdf:type owl:ObjectProperty ;
	rdfs:label "Results in"@en ;
	rdfs:comment "Relates an act of reporting to the thing being reported. An act of reporting results in one or more reported things. A reported thing results from one act of reporting."@en ;
	rdfs:domain report:Reporting ;
	rdfs:range report:ReportedThing ;
	rdfs:isDefinedBy <http://parliament.uk/ontologies/reporting/> .