@prefix pdep: <http://parliament.uk/ontologies/depositing/> . 
@prefix xsd: <http://www.w3.org/2001/XMLSchema#> . 
@prefix rdf: <http://www.w3.org/1999/02/22-rdf-syntax-ns#> .
@prefix dcterms: <http://purl.org/dc/terms/> .
@prefix owl:     <http://www.w3.org/2002/07/owl#> .
@prefix rdfs:    <http://www.w3.org/2000/01/rdf-schema#> .
@prefix foaf:	<http://xmlns.com/foaf/0.1/> .

<http://parliament.uk/ontologies/depositing/> 
    rdf:type owl:Ontology ;
    dcterms:title "Depositing ontology"@en ;
    dcterms:created "2022-12-01"^^xsd:date ;
	dcterms:rights "Open Parliament Licence v3.0"@en ;
    dcterms:description "A model describing commitments to deposit and the resulting deposits into a House, by means of its Library."@en ;
	foaf:depiction <https://ukparliament.github.io/ontologies/depositing/depositing.svg> ;
	foaf:maker 
		[ foaf:name "Robert Brook"; foaf:homepage <https://robert-brook.com/> ],
		[ foaf:name "Karen Cox" ],
		[ foaf:name "Andrew Dommett" ],
		[ foaf:name "John Greenhead" ],
		[ foaf:name "Ann Reilly" ],
		[ foaf:name "Michael Smethurst"; foaf:homepage <http://smethur.st/> ],
		[ foaf:name "Anya Somerville" ].




#######  Classes #####
	
pdep:MakingAvailable rdf:type owl:Class ;
	rdfs:label "Making available"@en ;
	rdfs:comment "The act of making a thing available to a House or to a House by means of its Library."@en ;
	rdfs:isDefinedBy <http://parliament.uk/ontologies/depositing/> .

pdep:MadeAvailableThing rdf:type owl:Class ;
	rdfs:label "Made available thing"@en ;
	rdfs:comment "A thing made available to a House or to a House by means of its Library."@en ;
	rdfs:isDefinedBy <http://parliament.uk/ontologies/depositing/> .

pdep:ParliamentaryPaper rdf:type owl:Class ;
	rdfs:label "Parliamentary paper"@en ;
	rdfs:comment "Papers made available to or published under the authority of Parliament."@en ;
	rdfs:isDefinedBy <http://parliament.uk/ontologies/depositing/> .
	
pdep:Depositing rdf:type owl:Class ;
	rdfs:subClassOf pdep:MakingAvailable ;
	rdfs:label "Depositing"@en ;
	rdfs:comment "The act of making information available to a House by means of its Library."@en ;
	rdfs:isDefinedBy <http://parliament.uk/ontologies/depositing/> .
	
pdep:DepositedPaper rdf:type owl:Class ;
	rdfs:subClassOf pdep:ParliamentaryPaper ;
	rdfs:subClassOf pdep:MadeAvailableThing ;
	rdfs:label "Deposited paper"@en ;
	rdfs:comment "A paper deposited in a Library of a House."@en ;
	rdfs:isDefinedBy <http://parliament.uk/ontologies/depositing/> .

pdep:CommittingThing rdf:type owl:Class ;
	rdfs:label "Committing thing"@en ;
	rdfs:comment "A thing in which a commitment to deposit is made, for example: an oral contribution to a parliamentary proceeding, a letter to a Library or a written statement."@en ;
	rdfs:isDefinedBy <http://parliament.uk/ontologies/depositing/> .

pdep:Commitment rdf:type owl:Class ;
	rdfs:label "Commitment"@en ;
	rdfs:comment "A commitment to deposit information in a Library or Libraries."@en ;
	rdfs:isDefinedBy <http://parliament.uk/ontologies/depositing/> .

pdep:Incumbency rdf:type owl:Class ;
	rdfs:label "Incumbency"@en ;
	rdfs:comment "The holding of a position by a person, including the time period for which this was the case. For example, Philip Hammond holding the position of Foreign Secretary between two dates."@en ;
	rdfs:isDefinedBy <http://parliament.uk/ontologies/depositing/> .

pdep:ParliamentaryPeriod rdf:type owl:Class ;
	rdfs:label "Parliamentary period"@en ;
	rdfs:comment "The time period of a single Parliament between the date of its first assembly after a general election and its dissolution. A Parliament period contains contiguous session and prorogation periods. During a parliament period Parliament is either in session or prorogued. The start date of a Parliament may be changed by subsequent proclamations. A Parliament ends at the next dissolution. While the Fixed-term Parliaments Act 2011 was in force, the date of dissolution was determined by that Act or was named in a proclamation following a vote in Parliament for an early general election. The next Parliament began on the date named in the proclamation issued following a dissolution. Before the Fixed-term Parliaments Act 2011 came into force and after that Act was repealed by the Dissolution and Calling of Parliament Act 2022, the date of dissolution is fixed by proclamation. The dissolution proclamation also names the date for Parliament to reassemble. Parliament periods are the same across both Houses. Parliaments are numbered ordinally from the first Parliament of the United Kingdom, sitting in 1801."@en ;
	rdfs:isDefinedBy <http://parliament.uk/ontologies/depositing/> .

pdep:Visibility rdf:type owl:Class ;
	rdfs:label "Visibility"@en ;
	rdfs:comment "The visibility of a deposited paper, being either publicly visible, publicly visible in a redacted form or available to Members only."@en ;
	rdfs:isDefinedBy <http://parliament.uk/ontologies/depositing/> .
	
	

#######  Object properties ##### 
	
pdep:leadsTo rdf:type owl:ObjectProperty ;
	rdfs:label "Leads to"@en ;
	rdfs:comment "Relates a credited contribution in which the intention to make a commitment is made to a committing thing. Credited contributions may include the phrase, 'I will write to the Library'. These are known as 'will writes'. Such a contribution should lead to one committing thing in the form of a letter of commitment to the Library. A letter of commitment may result from one credited contribution, or none."@en ;
	rdfs:domain pdep:CreditedContribution ;
	rdfs:range pdep:CommittingThing ;
	rdfs:isDefinedBy <http://parliament.uk/ontologies/depositing/> .
	
pdep:makesCommitment rdf:type owl:ObjectProperty ;
	rdfs:label "Makes commitment"@en ;
	rdfs:comment "Relates a committing thing to the commitment made. A committing thing includes one commitment. A commitment is included in one committing thing."@en ;
	rdfs:domain pdep:CommittingThing ;
	rdfs:range pdep:Commitment ;
	rdfs:isDefinedBy <http://parliament.uk/ontologies/depositing/> .
	
pdep:madeBy rdf:type owl:ObjectProperty ;
	rdfs:label "Made by"@en ;
	rdfs:comment "Relates a commitment to the incumbency of a person in a position making that commitment. A commitment is made by one incumbency."@en ;
	rdfs:domain pdep:Commitment ;
	rdfs:range pdep:Incumbency ;
	rdfs:isDefinedBy <http://parliament.uk/ontologies/depositing/> .
	
pdep:madeDuring rdf:type owl:ObjectProperty ;
	rdfs:label "Made during"@en ;
	rdfs:comment "Relates a commitment to the parliamentary period during which the commitment was made. A commitment is made during one parliamentary period."@en ;
	rdfs:domain pdep:Commitment ;
	rdfs:range pdep:ParliamentaryPeriod ;
	rdfs:isDefinedBy <http://parliament.uk/ontologies/depositing/> .
	
pdep:resultsFrom rdf:type owl:ObjectProperty ;
	rdfs:label "Results from"@en ;
	rdfs:comment "Relates a deposit to the commitment to make that deposit. A deposit results from one commitment. A commitment may result in one or more deposits, or none. Where a commitment has not yet resulted in a deposit, the House of Lords Library contacts the person who made the commitment."@en ;
	rdfs:domain pdep:Deposit ;
	rdfs:range pdep:Commitment ;
	rdfs:isDefinedBy <http://parliament.uk/ontologies/depositing/> .
	
pdep:resultsIn rdf:type owl:ObjectProperty ;
	rdfs:label "Results in"@en ;
	rdfs:comment "Relates a deposit to the paper it deposits. A deposit may result in one or more deposited papers."@en ;
	rdfs:domain pdep:Deposit ;
	rdfs:range pdep:DepositedPaper ;
	rdfs:isDefinedBy <http://parliament.uk/ontologies/depositing/> .
	
pdep:corrects rdf:type owl:ObjectProperty ;
	rdfs:label "Corrects"@en ;
	rdfs:comment "Relates a deposited paper to the deposited paper it corrects. A deposited paper may correct one deposited paper, or none. A deposited paper may be corrected by one deposited paper, or none."@en ;
	rdfs:domain pdep:DepositedPaper ;
	rdfs:range pdep:DepositedPaper ;
	rdfs:isDefinedBy <http://parliament.uk/ontologies/depositing/> .
	
pdep:hasVisibility rdf:type owl:ObjectProperty ;
	rdfs:label "Has visibility"@en ;
	rdfs:comment "Relates a deposited paper to the visibility of that deposited paper. A deposited paper has one visibility assigned."@en ;
	rdfs:domain pdep:DepositedPaper ;
	rdfs:range pdep:Visibility ;
	rdfs:isDefinedBy <http://parliament.uk/ontologies/depositing/> .

				

#######  Data properties #####

pdep:madeOn rdf:type owl:DatatypeProperty ;
	rdfs:label "Made on"@en ;
	rdfs:comment "Relates a commitment to the date on which that commitment was made."@en ;
	rdfs:domain pdep:Commitment ;
	rdfs:range xsd:date ;
	rdfs:isDefinedBy <http://parliament.uk/ontologies/depositing/> .
	
pdep:isStanding rdf:type owl:DatatypeProperty ;
	rdfs:label "Is standing"@en ;
	rdfs:comment "Used to record whether a commitment is standing. A standing commitment leads to more than one deposit over time."@en ;
	rdfs:domain pdep:Commitment ;
	rdfs:range xsd:boolean ;
	rdfs:isDefinedBy <http://parliament.uk/ontologies/depositing/> .
	
pdep:isArtefact rdf:type owl:DatatypeProperty ;
	rdfs:label "Is artefact"@en ;
	rdfs:comment "Used to record whether the deposited paper is an artefact, for example: a deposit of a breathalyzer would be recorded as an artefact."@en ;
	rdfs:domain pdep:DepositedPaper ;
	rdfs:range xsd:boolean ;
	rdfs:isDefinedBy <http://parliament.uk/ontologies/depositing/> .