@prefix pbish: <http://parliament.uk/ontologies/bishopric/> . 
@prefix xsd: <http://www.w3.org/2001/XMLSchema#> . 
@prefix rdf: <http://www.w3.org/1999/02/22-rdf-syntax-ns#> .
@prefix dcterms: <http://purl.org/dc/terms/> .
@prefix owl:     <http://www.w3.org/2002/07/owl#> .
@prefix rdfs:    <http://www.w3.org/2000/01/rdf-schema#> .
@prefix foaf:	<http://xmlns.com/foaf/0.1/> .
@prefix pcite: <http://parliament.uk/ontologies/citation/> .

<http://parliament.uk/ontologies/bishopric/> 
    rdf:type owl:Ontology ;
    dcterms:title "Bishopric ontology"@en ;
    dcterms:created "2022-11-08"^^xsd:date ;
	dcterms:rights "Open Parliament Licence v3.0"@en ;
    dcterms:description ""@en;
	foaf:depiction <https://ukparliament.github.io/ontologies/bishopric/bishopric.svg> ;
	foaf:maker
		[ foaf:name "Robert Brook"; foaf:homepage <https://robert-brook.com/> ],
		[ foaf:name "Ned Morrell" ],
		[ foaf:name "Anna Murphy" ],
		[ foaf:name "Michael Smethurst"; foaf:homepage <http://smethur.st/> ],
		[ foaf:name "Anya Somerville" ].


#######  Classes #####
	
pbish:Bishopric rdf:type owl:Class ;
	rdfs:label "Bishopric"@en ;
	rdfs:comment ""@en ;
	rdfs:isDefinedBy <http://parliament.uk/ontologies/bishopric/> .
	
	
	
	
	
	
	
	
	
	
	

	
#######  Object properties ##### 

pcite:hasCitation rdf:type owl:ObjectProperty ;
	rdfs:label "Has citation"@en ;
	rdfs:comment "Relates a citing thing to a citation. A citing thing includes one or more citations. A citation is included in one citing thing."@en ;
	rdfs:domain pcite:CitingThing ;
	rdfs:range pcite:Citation ;
	rdfs:isDefinedBy <http://parliament.uk/ontologies/citation/> .

pcite:refersTo rdf:type owl:ObjectProperty ;
	rdfs:label "Refers to"@en ;
	rdfs:comment "Relates a citation to the thing being cited. A cited thing may have one or more citations. A citation is to one cited thing."@en ;
	rdfs:domain pcite:Citation ;
	rdfs:range pcite:CitedThing ;
	rdfs:isDefinedBy <http://parliament.uk/ontologies/citation/> .

pcite:hasDocumentType rdf:type owl:ObjectProperty ;
	rdfs:label "Has document type"@en ;
	rdfs:comment "Relates a citation to the document type of the thing at the URI being cited. A citation has one document type, or none."@en ;
	rdfs:domain pcite:Citation ;
	rdfs:range pcite:DocumentType ;
	rdfs:isDefinedBy <http://parliament.uk/ontologies/citation/> .
	
	

#######  Data properties #####

pcite:hasUri rdf:type owl:DatatypeProperty ;
	rdfs:label "Has URI"@en ;
	rdfs:comment "Relates a citation to the URI of the thing being cited."@en ;
	rdfs:domain pcite:Citation ;
	rdfs:range rdfs:Literal ;
	rdfs:isDefinedBy <http://parliament.uk/ontologies/citation/> .
