@prefix parea: <http://parliament.uk/ontologies/geographic-area/> . 
@prefix xsd: <http://www.w3.org/2001/XMLSchema#> . 
@prefix rdf: <http://www.w3.org/1999/02/22-rdf-syntax-ns#> .
@prefix dcterms: <http://purl.org/dc/terms/> .
@prefix owl:     <http://www.w3.org/2002/07/owl#> .
@prefix rdfs:    <http://www.w3.org/2000/01/rdf-schema#> .
@prefix foaf:	<http://xmlns.com/foaf/0.1/> .

<http://parliament.uk/ontologies/geographic-area/> 
    rdf:type owl:Ontology ;
    dcterms:title "Geographic area ontology"@en ;
    dcterms:created "2021-09-28"^^xsd:date ;
	dcterms:rights "Open Parliament Licence v3.0"@en ;
    dcterms:description "A model describing geographic areas in the UK - being constituency areas, local authority areas, countries, and statistical regions within England - and the containment relationships between such areas."@en ;
	foaf:depiction <https://ukparliament.github.io/ontologies/geographic-area/geographic-area-period.svg> ;
	foaf:maker
		[ foaf:name "Carl Baker" ],
		[ foaf:name "Robert Brook"; foaf:homepage <https://robert-brook.com/> ],
		[ foaf:name "Ned Morrell" ],
		[ foaf:name "Mark Sandford" ],
		[ foaf:name "Michael Smethurst"; foaf:homepage <http://smethur.st/> ],
		[ foaf:name "Anya Somerville" ] .


#######  Classes #####

parea:GeographicArea rdf:type owl:Class ;
	rdfs:label "Geographic area"@en ;
	rdfs:comment "A named area of geography."@en ;
	rdfs:isDefinedBy <http://parliament.uk/ontologies/geographic-area/> .
	
parea:GeographicAreaEstablishedByStatute rdf:type owl:Class ;
	rdfs:subClassOf parea:GeographicArea ;
	rdfs:label "Geographic area established by statute"@en ;
	rdfs:comment "A geographic area established by an Act of Parliament or a made statutory instrument."@en ;
	rdfs:isDefinedBy <http://parliament.uk/ontologies/geographic-area/> .
	
parea:ConstituencyArea rdf:type owl:Class ;
	rdfs:subClassOf parea:GeographicAreaEstablishedByStatute ;
	rdfs:label "Constituency area"@en ;
	rdfs:comment "The geographic area of a UK Parliament constituency."@en ;
	rdfs:isDefinedBy <http://parliament.uk/ontologies/geographic-area/> .
	
parea:UpperTierLocalAuthorityArea rdf:type owl:Class ;
	rdfs:subClassOf parea:GeographicAreaEstablishedByStatute ;
	rdfs:label "Upper tier local authority area"@en ;
	rdfs:comment "The geographic area in which an upper tier local authority may exercise its powers."@en ;
	rdfs:isDefinedBy <http://parliament.uk/ontologies/geographic-area/> .

parea:LowerTierLocalAuthorityArea rdf:type owl:Class ;
	rdfs:subClassOf parea:GeographicAreaEstablishedByStatute ;
	rdfs:label "Lower tier local authority area"@en ;
	rdfs:comment "The geographic area in which a lower tier local authority may exercise its powers."@en ;
	rdfs:isDefinedBy <http://parliament.uk/ontologies/geographic-area/> .

parea:CombinedAuthorityArea rdf:type owl:Class ;
	rdfs:subClassOf parea:GeographicAreaEstablishedByStatute ;
	rdfs:label "Combined authority area"@en ;
	rdfs:comment "The geographic area in which a combined authority may exercise its powers. A combined authority may be created in England under powers set out in the Local Democracy, Economic Development and Construction Act 2009."@en ;
	rdfs:isDefinedBy <http://parliament.uk/ontologies/geographic-area/> .
	
parea:Region rdf:type owl:Class ;
	rdfs:subClassOf parea:GeographicArea ;
	rdfs:label "Region"@en ;
	rdfs:comment "A statistical region in England corresponding to a NUTS level 1 region."@en ;
	rdfs:isDefinedBy <http://parliament.uk/ontologies/geographic-area/> .
	
parea:Country rdf:type owl:Class ;
	rdfs:subClassOf parea:GeographicArea ;
	rdfs:label "Country"@en ;
	rdfs:comment "A country in the United Kingdom."@en ;
	rdfs:isDefinedBy <http://parliament.uk/ontologies/geographic-area/> .
	
parea:BoundarySet rdf:type owl:Class ;
	rdfs:label "Boundary set"@en ;
	rdfs:comment "A boundary set for UK Parliament constituency areas, as proposed in a boundary review by the Boundary Commission and established by statute."@en ;
	rdfs:isDefinedBy <http://parliament.uk/ontologies/geographic-area/> .

parea:StatutoryThing rdf:type owl:Class ;
	rdfs:label "Statutory thing"@en ;
	rdfs:comment "A statutory thing, for example: an Act of Parliament or a made statutory instrument."@en ;
	rdfs:isDefinedBy <http://parliament.uk/ontologies/geographic-area/> .
	
	
	
#######  Object properties ##### 

parea:whollyContainedBy rdf:type owl:ObjectProperty ;
	rdfs:label "Wholly contained by"@en ;
	rdfs:comment "Relates a geographic area to the geographic area it is wholly contained by. A constituency area may be wholly contained by a lower tier local authority area or by an upper tier local authority area. A constituency area in England is wholly contained by an English region. A constituency area is wholly contained by a country. A lower tier local authority area may be wholly contained by a constituency area. A lower tier local authority area is wholly contained by an upper tier local authority area, except where the lower tier local authority area is also the upper tier local authority area. An upper tier local authority area may be wholly contained by a constituency area. As at November 2021, an upper tier local authority area is wholly contained by a combined authority area, where a combined authority area exists.An upper tier local authority area in England is wholly contained by an English region. An upper tier local authority area is wholly contained by a country. A combined authority area may be wholly contained by an English region. A combined authority area is wholly contained by the country of England. An English region is wholly contained by the country of England."@en ;
	rdfs:domain parea:GeographicArea ;
	rdfs:range parea:GeographicArea ;
	rdfs:isDefinedBy <http://parliament.uk/ontologies/geographic-area/> .

parea:partlyContainedBy rdf:type owl:ObjectProperty ;
	rdfs:label "Partly contained by"@en ;
	rdfs:comment "Relates a geographic area to a geographic area it is partly contained by. A constituency area may be partly contained by a lower tier local authority area, by an upper tier local authority area, or by neither. A lower tier local authority area or an upper tier local authority area may be partly contained by a constituency area. The Local Democracy, Economic Development and Construction Act 2009 does not preclude an upper tier local authority area being partly contained by a combined authority area. As at November 2021, no upper tier local authority area is partly contained by a combined authority area."@en ;
	rdfs:domain parea:GeographicArea ;
	rdfs:range parea:GeographicArea ;
	rdfs:isDefinedBy <http://parliament.uk/ontologies/geographic-area/> .

parea:definedBy rdf:type owl:ObjectProperty ;
	rdfs:label "Defined by"@en ;
	rdfs:comment "Relates a constituency area to the boundary set it was defined by."@en ;
	rdfs:domain parea:ConstituencyArea ;
	rdfs:range parea:BoundarySet ;
	rdfs:isDefinedBy <http://parliament.uk/ontologies/geographic-area/> .

parea:establishedBy rdf:type owl:ObjectProperty ;
	rdfs:label "Established by"@en ;
	rdfs:comment "Relates a geographic area established by statute to the statutory thing it was established by."@en ;
	rdfs:domain parea:GeographicAreaEstablishedByStatute ;
	rdfs:range parea:StatutoryThing ;
	rdfs:isDefinedBy <http://parliament.uk/ontologies/geographic-area/> .
	
parea:boundarySetEstablishedBy rdf:type owl:ObjectProperty ;
	rdfs:label "Boundary set established by"@en ;
	rdfs:comment "Relates a boundary set to the statutory thing it was established by."@en ;
	rdfs:domain parea:BoundarySet ;
	rdfs:range parea:StatutoryThing ;
	rdfs:isDefinedBy <http://parliament.uk/ontologies/geographic-area/> .

parea:isAlsoUpperTierLocalAuthorityArea rdf:type owl:ObjectProperty ;
	rdfs:label "Is also upper tier local authority area"@en ;
	rdfs:comment "Relates a lower tier local authority area to an upper tier local authority area where the lower tier local authority area is also the upper tier local authority area."@en ;
	rdfs:domain parea:LowerTierLocalAuthorityArea ;
	rdfs:range parea:UpperTierLocalAuthorityArea ;
	rdfs:isDefinedBy <http://parliament.uk/ontologies/geographic-area/> .
	
	
	
#######  Data properties ##### 

parea:ons_code rdf:type owl:DatatypeProperty ;
	rdfs:label "ONS code"@en ;
	rdfs:comment "Relates a geographic area to its code as assigned by the Office of National Statistics."@en ;
	rdfs:domain parea:GeographicArea ;
	rdfs:range rdfs:Literal ;
	rdfs:isDefinedBy <http://parliament.uk/ontologies/geographic-area/> .

parea:geometry rdf:type owl:DatatypeProperty ;
	rdfs:label "Geometry"@en ;
	rdfs:comment "Relates a geographic area to the geometry describing the boundaries of that area."@en ;
	rdfs:domain parea:GeographicArea ;
	rdfs:range rdfs:Literal ;
	rdfs:isDefinedBy <http://parliament.uk/ontologies/geographic-area/> .

parea:appliesFrom rdf:type owl:DatatypeProperty ;
	rdfs:label "Applies from"@en ;
	rdfs:comment "Relates a boundary set to the date that boundary set applies from."@en ;
	rdfs:domain parea:BoundarySet ;
	rdfs:range xsd:date ;
	rdfs:isDefinedBy <http://parliament.uk/ontologies/geographic-area/> .