@prefix pordertoprint: <http://parliament.uk/ontologies/order-to-print/> . 
@prefix xsd: <http://www.w3.org/2001/XMLSchema#> . 
@prefix rdf: <http://www.w3.org/1999/02/22-rdf-syntax-ns#> .
@prefix dcterms: <http://purl.org/dc/terms/> .
@prefix owl:     <http://www.w3.org/2002/07/owl#> .
@prefix rdfs:    <http://www.w3.org/2000/01/rdf-schema#> .
@prefix foaf:	<http://xmlns.com/foaf/0.1/> .

<http://parliament.uk/ontologies/order-to-print/> 
    rdf:type owl:Ontology ;
    dcterms:title "Order to print ontology"@en ;
    dcterms:created "2023-02-26"^^xsd:date ;
	dcterms:rights "Open Parliament Licence v3.0"@en ;
    dcterms:description "A model describing an order to print by a House."@en;
	foaf:depiction <https://ukparliament.github.io/ontologies/order-to-print/order-to-print.svg> ;
	foaf:maker 
		[ foaf:name "Jayne Bosworth" ],
		[ foaf:name "Robert Brook"; foaf:homepage <https://robert-brook.com/> ],
		[ foaf:name "Ned Morrell" ],
		[ foaf:name "Claire Searle" ],
		[ foaf:name "Michael Smethurst"; foaf:homepage <http://smethur.st/> ],
		[ foaf:name "Anya Somerville" ] .


#######  Classes #####
	
pordertoprint:MakingAvailable rdf:type owl:Class ;
	rdfs:label "Making available"@en ;
	rdfs:comment "The act of making a thing available to a House or to a House by means of its Library."@en ;
	rdfs:isDefinedBy <http://parliament.uk/ontologies/order-to-print/> .
	
pordertoprint:OrderToPrint rdf:type owl:Class ;
	rdfs:subClassOf pordertoprint:MakingAvailable ;
	rdfs:label "Order to print"@en ;
	rdfs:comment "The ordering, by a House, of a paper to be printed."@en ;
	rdfs:isDefinedBy <http://parliament.uk/ontologies/order-to-print/> .

pordertoprint:MadeAvailableThing rdf:type owl:Class ;
	rdfs:label "Made available thing"@en ;
	rdfs:comment "A thing made available to a House or to a House by means of its Library."@en ;
	rdfs:isDefinedBy <http://parliament.uk/ontologies/order-to-print/> .

pordertoprint:PaperExpression rdf:type owl:Class ;
	rdfs:label "Paper expression"@en ;
	rdfs:comment "A paper made available to a House, being an expression of a paper work."@en ;
	rdfs:isDefinedBy <http://parliament.uk/ontologies/order-to-print/> .
	
pordertoprint:PrintedPaper rdf:type owl:Class ;
	rdfs:subClassOf pordertoprint:MadeAvailableThing ;
	rdfs:subClassOf pordertoprint:PaperExpression ;
	rdfs:label "Printed paper"@en ;
	rdfs:comment "A paper printed by order of a House."@en ;
	rdfs:isDefinedBy <http://parliament.uk/ontologies/order-to-print/> .
	
	
#######  Object properties ##### 
	
pordertoprint:resultsIn rdf:type owl:ObjectProperty ;
	rdfs:label "Results in"@en ;
	rdfs:comment "Relates an act of ordering to print to the paper which has been printed. An act of ordering to print results in one printed paper. A printed paper is the result of one act of ordering to print."@en ;
	rdfs:domain pordertoprint:OrderToPrint ;
	rdfs:range pordertoprint:PrintedPaper ;
	rdfs:isDefinedBy <http://parliament.uk/ontologies/order-to-print/> .