@prefix ppresent: <http://parliament.uk/ontologies/presentation/> . 
@prefix xsd: <http://www.w3.org/2001/XMLSchema#> . 
@prefix rdf: <http://www.w3.org/1999/02/22-rdf-syntax-ns#> .
@prefix dcterms: <http://purl.org/dc/terms/> .
@prefix owl:     <http://www.w3.org/2002/07/owl#> .
@prefix rdfs:    <http://www.w3.org/2000/01/rdf-schema#> .
@prefix foaf:	<http://xmlns.com/foaf/0.1/> .

<http://parliament.uk/ontologies/presentation/> 
    rdf:type owl:Ontology ;
    dcterms:title "Presentation ontology"@en ;
    dcterms:created "2022-08-03"^^xsd:date ;
	dcterms:rights "Open Parliament Licence v3.0"@en ;
    dcterms:description "A model describing the presentation of papers into a House."@en;
	foaf:depiction <https://ukparliament.github.io/ontologies/presentation/presentation.svg> ;
	foaf:maker 
		[ foaf:name "Jayne Bosworth" ],
		[ foaf:name "Robert Brook"; foaf:homepage <https://robert-brook.com/> ],
		[ foaf:name "Ned Morrell" ],
		[ foaf:name "Michael Smethurst"; foaf:homepage <http://smethur.st/> ],
		[ foaf:name "Anya Somerville" ].


#######  Classes #####
	
ppresent:MakingAvailable rdf:type owl:Class ;
	rdfs:label "Making available"@en ;
	rdfs:comment "The act of making a thing available to a House or to a House by means of its Library."@en ;
	rdfs:isDefinedBy <http://parliament.uk/ontologies/presentation/> .
	
ppresent:Presentation rdf:type owl:Class ;
	rdfs:subClassOf ppresent:MakingAvailable ;
	rdfs:label "Presentation"@en ;
	rdfs:comment "The act of presenting a paper to a House."@en ;
	rdfs:isDefinedBy <http://parliament.uk/ontologies/presentation/> .
	
ppresent:ParliamentaryPaper rdf:type owl:Class ;
	rdfs:label "Parliamentary paper"@en ;
	rdfs:comment "Papers laid into or published under the authority of Parliament."@en ;
	rdfs:isDefinedBy <http://parliament.uk/ontologies/presentation/> .

ppresent:MadeAvailableThing rdf:type owl:Class ;
	rdfs:label "Made available thing"@en ;
	rdfs:comment "A thing made available to a House or to a House by means of its Library."@en ;
	rdfs:isDefinedBy <http://parliament.uk/ontologies/presentation/> .
	
ppresent:PresentedPaper rdf:type owl:Class ;
	rdfs:subClassOf ppresent:ParliamentaryPaper ;
	rdfs:subClassOf ppresent:MadeAvailableThing ;
	rdfs:label "Presented paper"@en ;
	rdfs:comment "A paper having been presented to a House."@en ;
	rdfs:isDefinedBy <http://parliament.uk/ontologies/presentation/> .
	
	

#######  Object properties ##### 
	
ppresent:resultsIn rdf:type owl:ObjectProperty ;
	rdfs:label "Results in"@en ;
	rdfs:comment "Relates an act of presenting a paper to the paper having been presented."@en ;
	rdfs:domain ppresent:Presentation ;
	rdfs:range ppresent:PresentedPaper ;
	rdfs:isDefinedBy <http://parliament.uk/ontologies/presentation/> .