@prefix parea-overlap: <http://parliament.uk/ontologies/geographic-area-overlap/> . 
@prefix xsd: <http://www.w3.org/2001/XMLSchema#> . 
@prefix rdf: <http://www.w3.org/1999/02/22-rdf-syntax-ns#> .
@prefix dcterms: <http://purl.org/dc/terms/> .
@prefix owl:     <http://www.w3.org/2002/07/owl#> .
@prefix rdfs:    <http://www.w3.org/2000/01/rdf-schema#> .
@prefix foaf:	<http://xmlns.com/foaf/0.1/> .

<http://parliament.uk/ontologies/geographic-area-overlap/> 
    rdf:type owl:Ontology ;
    dcterms:title "Geographic area overlap ontology"@en ;
    dcterms:created "2023-12-05"^^xsd:date ;
	dcterms:rights "Open Parliament Licence v3.0"@en ;
    dcterms:description "A model describing overlaps in area, number of residential properties or total population from a named geographic area to a succeeding or preceding named geographic area, for example: a UK Parliament constituency."@en ;
	foaf:depiction <https://ukparliament.github.io/ontologies/geographic-area-overlap/geographic-area-overlap.svg> ;
	foaf:maker
		[ foaf:name "Carl Baker" ],
		[ foaf:name "Robert Brook"; foaf:homepage <https://robert-brook.com/> ],
		[ foaf:name "Ned Morrell" ],
		[ foaf:name "Michael Smethurst"; foaf:homepage <http://smethur.st/> ] .


#######  Classes #####

parea-overlap:GeographicArea rdf:type owl:Class ;
	rdfs:label "Geographic area"@en ;
	rdfs:comment "A named area of geography."@en ;
	rdfs:isDefinedBy <http://parliament.uk/ontologies/geographic-area-overlap/> .
	
parea-overlap:GeographicAreaOverlap rdf:type owl:Class ;
	rdfs:label "Geographic area overlap"@en ;
	rdfs:comment "The overlap between a preceding and succeeding geographic area."@en ;
	rdfs:isDefinedBy <http://parliament.uk/ontologies/geographic-area-overlap/> .
	
	
	
#######  Object properties ##### 

parea-overlap:precedingGeographicArea rdf:type owl:ObjectProperty ;
	rdfs:label "Preceding geographic area"@en ;
	rdfs:comment "Relates a geographic area overlap to the preceding geographic area. A geographic area overlap relates to one preceding geographic area."@en ;
	rdfs:domain parea-overlap:GeographicAreaOverlap ;
	rdfs:range parea-overlap:GeographicArea ;
	rdfs:isDefinedBy <http://parliament.uk/ontologies/geographic-area-overlap/> .
	
parea-overlap:succeedingGeographicArea rdf:type owl:ObjectProperty ;
	rdfs:label "Succeeding geographic area"@en ;
	rdfs:comment "Relates a geographic area overlap to the succeeding geographic area. A geographic area overlap relates to one succeeding geographic area."@en ;
	rdfs:domain parea-overlap:GeographicAreaOverlap ;
	rdfs:range parea-overlap:GeographicArea ;
	rdfs:isDefinedBy <http://parliament.uk/ontologies/geographic-area-overlap/> .
	
	
	
#######  Data properties ##### 

parea-overlap:precedingAreaOverlap rdf:type owl:DatatypeProperty ;
	rdfs:label "Preceding area overlap"@en ;
	rdfs:comment "Used to record the proportion of the area of the preceding geographic area forming part of the succeeding geographic area."@en ;
	rdfs:domain parea-overlap:GeographicAreaOverlap ;
	rdfs:range xsd:float ;
	rdfs:isDefinedBy <http://parliament.uk/ontologies/geographic-area-overlap/> .
	
parea-overlap:succeedingAreaOverlap rdf:type owl:DatatypeProperty ;
	rdfs:label "Succeeding area overlap"@en ;
	rdfs:comment "Used to record the proportion of the area of the succeeding geographic area formed from part of the preceding geographic area."@en ;
	rdfs:domain parea-overlap:GeographicAreaOverlap ;
	rdfs:range xsd:float ;
	rdfs:isDefinedBy <http://parliament.uk/ontologies/geographic-area-overlap/> .
	
parea-overlap:precedingResidentialOverlap rdf:type owl:DatatypeProperty ;
	rdfs:label "Preceding residential overlap"@en ;
	rdfs:comment "Used to record the proportion of residential properties in the preceding geographic area forming part of the succeeding geographic area."@en ;
	rdfs:domain parea-overlap:GeographicAreaOverlap ;
	rdfs:range xsd:float ;
	rdfs:isDefinedBy <http://parliament.uk/ontologies/geographic-area-overlap/> .
	
parea-overlap:succeedingResidentialOverlap rdf:type owl:DatatypeProperty ;
	rdfs:label "Succeeding residential overlap"@en ;
	rdfs:comment "Used to record the proportion of residential properties in the succeeding geographic area formed from part of the preceding geographic area."@en ;
	rdfs:domain parea-overlap:GeographicAreaOverlap ;
	rdfs:range xsd:float ;
	rdfs:isDefinedBy <http://parliament.uk/ontologies/geographic-area-overlap/> .
	
parea-overlap:precedingPopulationOverlap rdf:type owl:DatatypeProperty ;
	rdfs:label "Preceding population overlap"@en ;
	rdfs:comment "Used to record the proportion of the population of the preceding geographic area forming part of the succeeding geographic area."@en ;
	rdfs:domain parea-overlap:GeographicAreaOverlap ;
	rdfs:range xsd:float ;
	rdfs:isDefinedBy <http://parliament.uk/ontologies/geographic-area-overlap/> .
	
parea-overlap:succeedingPopulationOverlap rdf:type owl:DatatypeProperty ;
	rdfs:label "Succeeding population overlap"@en ;
	rdfs:comment "Used to record the proportion of the population in the succeeding geographic area formed from part of the preceding geographic area."@en ;
	rdfs:domain parea-overlap:GeographicAreaOverlap ;
	rdfs:range xsd:float ;
	rdfs:isDefinedBy <http://parliament.uk/ontologies/geographic-area-overlap/> .
	
# edited to here

parea-overlap:formedFromWholeOf rdf:type owl:DatatypeProperty ;
	rdfs:label "Formed from whole of"@en ;
	rdfs:comment "Used to record whether the whole of the preceding geographic area went to form all or part of the succeeding geographic area, being based on area overlaps."@en ;
	rdfs:domain parea-overlap:GeographicAreaOverlap ;
	rdfs:range xsd:boolean ;
	rdfs:isDefinedBy <http://parliament.uk/ontologies/geographic-area-overlap/> .
	
parea-overlap:formsWholeOf rdf:type owl:DatatypeProperty ;
	rdfs:label "Forms whole of"@en ;
	rdfs:comment "Used to record whether the whole of the succeeding geographic area was formed from all or part of the preceding geographic area, being based on area overlaps."@en ;
	rdfs:domain parea-overlap:GeographicAreaOverlap ;
	rdfs:range xsd:boolean ;
	rdfs:isDefinedBy <http://parliament.uk/ontologies/geographic-area-overlap/> .