@prefix pqa: <http://parliament.uk/ontologies/question-and-answer/> . 
@prefix xsd: <http://www.w3.org/2001/XMLSchema#> . 
@prefix rdf: <http://www.w3.org/1999/02/22-rdf-syntax-ns#> .
@prefix dcterms: <http://purl.org/dc/terms/> .
@prefix owl:     <http://www.w3.org/2002/07/owl#> .
@prefix rdfs:    <http://www.w3.org/2000/01/rdf-schema#> .
@prefix foaf:	<http://xmlns.com/foaf/0.1/> .

<http://parliament.uk/ontologies/question-and-answer/> 
    rdf:type owl:Ontology ;
    dcterms:title "Question and answer ontology"@en ;
    dcterms:created "2016-10-10"^^xsd:date ;
	dcterms:rights "Open Parliament Licence v3.0"@en ;
    dcterms:description "A model describing questions and answers in Parliament, types and forms of answers expected - and allocations to answering bodies."@en ;
	foaf:depiction <https://ukparliament.github.io/ontologies/question-and-answer/question-and-answer.svg> ;
	foaf:maker
		[ foaf:name "Robert Brook"; foaf:homepage <https://robert-brook.com/> ],
		[ foaf:name "Ned Morrell" ],
		[ foaf:name "Michael Smethurst"; foaf:homepage <http://smethur.st/> ],
	    [ foaf:name "Anya Somerville" ].


#######  Classes ##### 	

pqa:Incumbency rdf:type owl:Class ;
	rdfs:label "Incumbency"@en ;
	rdfs:comment "The holding of a position by a person, including the time period for which this was the case. For example, Philip Hammond holding the position of Foreign Secretary between two dates."@en ;
	rdfs:isDefinedBy <http://parliament.uk/ontologies/question-and-answer/> .
	
pqa:ParliamentaryQuestion rdf:type owl:Class ;
    rdfs:subClassOf pqa:Question ;
	rdfs:label "Parliamentary question"@en ;
	rdfs:comment "Parliamentary questions - often referred to as PQs - are a means by which Members may seek information from an answering body, or ask a Secretary of State to take a particular action. They are usually asked of a Minister in a Government department, though questions can be asked of Members representing non-departmental bodies, for example: Church Commissioners. Parliamentary questions can be asked in expectation of either a written or an oral answer, spoken by a Member in the Chamber. Parliamentary questions are tabled in the Table Office of the Lords or the Commons."@en ;
	rdfs:isDefinedBy <http://parliament.uk/ontologies/question-and-answer/> .
	
pqa:UrgentQuestion rdf:type owl:Class ;
    rdfs:subClassOf pqa:Question ;
	rdfs:label "Urgent question"@en ;
	rdfs:comment "Urgent questions are a means by which Members of the House of Commons may ask a Minister a question which the Member considers requires an immediate answer. In the House of Lords such questions are referred to as private notice questions. Urgent questions and private notice questions are applied for to the Speaker or the Lord Speaker rather than being tabled in the Table Office: the text of an urgent question or a private notice question does not appear on the Order Paper. A debate in the Chamber takes place if an application is granted."@en ;
	rdfs:isDefinedBy <http://parliament.uk/ontologies/question-and-answer/> .
	
pqa:BusinessQuestion rdf:type owl:Class ;
    rdfs:subClassOf pqa:Question ;
	rdfs:label "Business question"@en ;
	rdfs:comment "Business questions are a means by which Members of the House of Commons may ask the Leader of the House about forthcoming business. Both question and answer will be spoken in the Chamber."@en ;
	rdfs:isDefinedBy <http://parliament.uk/ontologies/question-and-answer/> .
	
pqa:Question rdf:type owl:Class ;
	rdfs:label "Question"@en ;
	rdfs:comment "A question may be an oral or written parliamentary question, an urgent  - or private notice - question or a business question. A question is asked by a Member of a House of an answering body."@en ;
	rdfs:isDefinedBy <http://parliament.uk/ontologies/question-and-answer/> .
	
pqa:AnswerExpectedAs rdf:type owl:Class ;
	rdfs:label "Answer expected as"@en ;
	rdfs:comment "A time-bound means of defining the form of answer expected for a question, being oral or written. In the House of Commons, a question tabled in expectation of an oral answer may change to a question in expectation of a written answer - and would have two Answer Expected As relationships: one for the first period when the form of answer expected is oral and one for the second period when the form of answer expected is written."@en ;
	rdfs:isDefinedBy <http://parliament.uk/ontologies/question-and-answer/> .

pqa:FormOfAnswer rdf:type owl:Class ;
	rdfs:label "Form of answer"@en ;
	rdfs:comment "The form in which an answer is given, being either oral or written."@en ;
	rdfs:isDefinedBy <http://parliament.uk/ontologies/question-and-answer/> .
	
pqa:AnswerExpectedAsChange rdf:type owl:Class ;
	rdfs:label "Answer expected as change"@en ;
	rdfs:comment "In the House of Commons, the change from an expectation of an oral answer to an expectation of a written answer. The change of expectation may be because the Member tabling the question is unable to attend the Chamber at the time the question was due to be answered, or because a question may be due in the Chamber but may not be reached because the allocated time runs out. In the case of a Member not being present, they may either withdraw or unstar the question. Unstarring removes the question from the Order Paper and changes the form of the answer expected to written. When a question is not reached, the question is given a written answer unless the Member withdraws the question. In the House of Lords, a different Member attends the Chamber and asks the question on the tabling Member's behalf when the tabling Member cannot attend. There is no requirement for unstarring. In the House of Lords, questions tabled in expectation of an oral answer are always reached. There is no requirement for handling questions not reached."@en ;
	rdfs:isDefinedBy <http://parliament.uk/ontologies/question-and-answer/> .
	
pqa:AnswerExpectedAsChangeReason rdf:type owl:Class ;
	rdfs:label "Answer expected as change reason"@en ;
	rdfs:comment "The reason, being either unstarred or not reached, for a change in the expected form of an answer."@en ;
	rdfs:isDefinedBy <http://parliament.uk/ontologies/question-and-answer/> .
	
pqa:Answer rdf:type owl:Class ;
    rdfs:subClassOf pqa:PursuableThing ;
	rdfs:label "Answer"@en ;
	rdfs:comment "An answer to a question given by a Member, usually a Minister, on behalf of an answering body."@en ;
	rdfs:isDefinedBy <http://parliament.uk/ontologies/question-and-answer/> .
	
pqa:OrganisationAccountableToParliament rdf:type owl:Class ;
	rdfs:label "Organisation accountable to Parliament"@en ;
	rdfs:comment "An organisation accountable to Parliament: being a Government department, a Government organisation, a non-governmental organisation with a duty to answer questions or an organisation with a duty to lay papers."@en ;
	rdfs:isDefinedBy <http://parliament.uk/ontologies/question-and-answer/> .
	
pqa:AnsweringBody rdf:type owl:Class ;
    rdfs:subClassOf pqa:OrganisationAccountableToParliament ;
	rdfs:label "Answering body"@en ;
	rdfs:comment "A body of whom Members can ask questions. In the House of Commons this may be a government department, a Parliamentary body or a body external to Parliament, for example: the House of Commons Commission or Church Commissioners. In the House of Lords, questions are addressed to Her Majesty's Government rather than to a department or body. In the House of Lords, the Table Office assigns written and private notice questions to an answering body. For questions in expectation of an oral answer, no assignment takes place."@en ;
	rdfs:isDefinedBy <http://parliament.uk/ontologies/question-and-answer/> .
	
pqa:AnsweringBodyAllocation rdf:type owl:Class ;
	rdfs:label "Answering body allocation"@en ;
	rdfs:comment "An allocation to the answering body to which a question is directed, either at tabling or when asked in the House. The allocation to an answering body may change over time, if an answering body transfers responsibility to another answering body."@en ;
	rdfs:isDefinedBy <http://parliament.uk/ontologies/question-and-answer/> .
	
pqa:Transferral rdf:type owl:Class ;
	rdfs:label "Transferral"@en ;
	rdfs:comment "The act of one answering body transferring responsibility for answering a question to another answering body."@en ;
	rdfs:isDefinedBy <http://parliament.uk/ontologies/question-and-answer/> .
	
pqa:PursuableThing rdf:type owl:Class ;
	rdfs:label "Pursuable thing"@en ;
	rdfs:comment "A thing being cited in a question. The question is asked as a follow up to the pursuable thing, for example: pursuant to a previous answer or a ministerial statement."@en ;
	rdfs:isDefinedBy <http://parliament.uk/ontologies/question-and-answer/> .
	
pqa:AnswerType rdf:type owl:Class ;
	rdfs:label "Answer type"@en ;
	rdfs:comment "The type of a given answer - being a dissolution answer, a prorogation answer, a holding answer, a substantive answer or a substantive answer as corrected."@en ;
	rdfs:isDefinedBy <http://parliament.uk/ontologies/question-and-answer/> .
	
pqa:DelegatedAnswer rdf:type owl:Class ;
    rdfs:subClassOf pqa:Answer ;
	rdfs:label "Delegated answer"@en ;
	rdfs:comment "A written answer containing material contributed by an organisation to which the answering body delegates responsibility for the provision of information necessary to answer the question, for example: an answer provided by the Cabinet Office, containing material contributed by the UK Statistics Authority."@en ;
	rdfs:isDefinedBy <http://parliament.uk/ontologies/question-and-answer/> .
	
pqa:DelegatedAnswerBody rdf:type owl:Class ;
	rdfs:label "Delegated answer body"@en ;
	rdfs:comment "An organisation that may provide an answering body with information necessary to answer a question allocated to that answering body."@en ;
	rdfs:isDefinedBy <http://parliament.uk/ontologies/question-and-answer/> .
	
pqa:LibraryDeposit rdf:type owl:Class ;
	rdfs:label "Library deposit"@en ;
	rdfs:comment "A paper or set of papers placed by a Minister, or the Speaker, or the Lord Speaker, in the Library of either House, or in both."@en ;
	rdfs:isDefinedBy <http://parliament.uk/ontologies/question-and-answer/> .
	
pqa:Document rdf:type owl:Class ;
	rdfs:label "Document"@en ;
	rdfs:comment "A document."@en ;
	rdfs:isDefinedBy <http://parliament.uk/ontologies/question-and-answer/> .

	

#######  Object properties ##### 

pqa:allocation rdf:type owl:ObjectProperty ;
	rdfs:label "Allocation"@en ;
	rdfs:comment "Relates a question to the allocation of that question to an answering body. A question will have one allocation at any one time but may have more than one allocation over time. An allocation is always of one question."@en ;
	rdfs:domain pqa:Question ;
	rdfs:range pqa:AnsweringBodyAllocation ;
	rdfs:isDefinedBy <http://parliament.uk/ontologies/question-and-answer/> .

pqa:allocatedTo rdf:type owl:ObjectProperty ;
	rdfs:label "Allocated to"@en ;
	rdfs:comment "Relates the allocation of a question to an answering body to that answering body. An allocation is always to one answering body. An answering body may have many allocations."@en ;
	rdfs:domain pqa:AnsweringBodyAllocation ;
	rdfs:range pqa:AnsweringBody ;
	rdfs:isDefinedBy <http://parliament.uk/ontologies/question-and-answer/> .

pqa:startsAllocation rdf:type owl:ObjectProperty ;
	rdfs:label "Starts allocation"@en ;
	rdfs:comment "Relates an act of transferral to the answering body allocation started by that transferral. A transferral always starts one allocation. An allocation may be started by one transferral, or none."@en ;
	rdfs:domain pqa:Transferral ;
	rdfs:range pqa:AnsweringBodyAllocation ;
	rdfs:isDefinedBy <http://parliament.uk/ontologies/question-and-answer/> .

pqa:endsAllocation rdf:type owl:ObjectProperty ;
	rdfs:label "Ends allocation"@en ;
	rdfs:comment "Relates an act of transferral to the answering body allocation ended by that transferral. A transferral always ends one allocation. An allocation may be ended by one transferral, or none."@en ;
	rdfs:domain pqa:Transferral ;
	rdfs:range pqa:AnsweringBodyAllocation ;
	rdfs:isDefinedBy <http://parliament.uk/ontologies/question-and-answer/> .

pqa:answerTo rdf:type owl:ObjectProperty ;
	rdfs:label "Answer to"@en ;
	rdfs:comment "Relates an answer to the question or questions it answers. An answering body may group questions for answer, in order to provide one answer in response to that group of questions. A question may have one or more answers provided over time, for example: a holding answer may be replaced by a substantive answer which may then be in receipt of a correcting answer."@en ;
	rdfs:domain pqa:Answer ;
	rdfs:range pqa:Question ;
	rdfs:isDefinedBy <http://parliament.uk/ontologies/question-and-answer/> .
	
pqa:fromAnsweringBody rdf:type owl:ObjectProperty ;
	rdfs:label "From answering body"@en ;
	rdfs:comment "Relates an answer to the answering body that provided it. An answer is provided by one answering body."@en ;
	rdfs:domain pqa:Answer ;
	rdfs:range pqa:AnsweringBody ;
	rdfs:isDefinedBy <http://parliament.uk/ontologies/question-and-answer/> .
	
pqa:askedBy rdf:type owl:ObjectProperty ;
	rdfs:label "Asked by"@en ;
	rdfs:comment "Relates a question to an incumbency of the person asking the question. A Member in the House of Lords tabling a question in expectation of an oral answer may nominate another Member to be present in the Chamber to receive the answer."@en ;
	rdfs:domain pqa:Question ;
	rdfs:range pqa:Incumbency ;
	rdfs:isDefinedBy <http://parliament.uk/ontologies/question-and-answer/> .
	
pqa:pursuantTo rdf:type owl:ObjectProperty ;
	rdfs:label "Pursuant to"@en ;
	rdfs:comment "Relates a question to an item of parliamentary business cited in that question."@en ;
	rdfs:domain pqa:Question ;
	rdfs:range pqa:PursuableThing ;
	rdfs:isDefinedBy <http://parliament.uk/ontologies/question-and-answer/> .
	
pqa:answeredBy rdf:type owl:ObjectProperty ;
	rdfs:label "Answered by"@en ;
	rdfs:comment "Relates an answer to an incumbency of the person providing the answer. Answers are provided by a person incumbent in a position in government or in a non-departmental answering body with a duty to answer parliamentary questions. For questions in receipt of an oral answer in the House of Lords, this may be the incumbency held by a person in a position as a government whip. [February 2022] Data for questions and answers identifies the Member providing the answer, but not the incumbency in a position with a duty to provide an answer. For this reason, we may need to fall back on pointing to a House seat incumbency."@en ;
	rdfs:domain pqa:Answer ;
	rdfs:range pqa:Incumbency ;
	rdfs:isDefinedBy <http://parliament.uk/ontologies/question-and-answer/> .
	
									# edited to here
	
pqa:hasAnswerType rdf:type owl:ObjectProperty ;
	rdfs:label "Has answer type"@en ;
	rdfs:comment "Relates an answer to its type i.e. a holding answer, substantive answer or corrected substantive answer."@en ;
	rdfs:domain pqa:Answer ;
	rdfs:range pqa:AnswerType ;
	rdfs:isDefinedBy <http://parliament.uk/ontologies/question-and-answer/> .
	
pqa:replacesAnswer rdf:type owl:ObjectProperty ;
	rdfs:label "Replaces answer"@en ;
	rdfs:comment "Relates an answer to a subsequent answer given to the same question e.g. a holding answer to a substantive answer, or a substantive answer to a corrected answer, a corrected answer to a further corrected answer. Substantive answers replace holding answers in whole, whereas corrected answers may replace a previous answer in whole or in part."@en ;
	rdfs:domain pqa:Answer ;
	rdfs:range pqa:Answer ;
	rdfs:isDefinedBy <http://parliament.uk/ontologies/question-and-answer/> .

pqa:refersToPreviousAnswer rdf:type owl:ObjectProperty ;
	rdfs:label "Refers to previous answer"@en ;
	rdfs:comment "Relates an answer to a previous answer that answers the question in whole or in part e.g. 'I refer the honourable X to the answer given...'"@en ;
	rdfs:domain pqa:Answer ;
	rdfs:range pqa:Answer ;
	rdfs:isDefinedBy <http://parliament.uk/ontologies/question-and-answer/> .
	
pqa:delegatedTo rdf:type owl:ObjectProperty ;
	rdfs:label "Delegated to"@en ;
	rdfs:comment "Relates a delegated answer to the arm's length body that provided it."@en ;
	rdfs:domain pqa:DelegatedAnswer ;
	rdfs:range pqa:DelegatedAnswerBody ;
	rdfs:isDefinedBy <http://parliament.uk/ontologies/question-and-answer/> .
	
pqa:refersToLibraryDeposit rdf:type owl:ObjectProperty ;
	rdfs:label "Refers to Library deposit"@en ;
	rdfs:comment "Relates an answer to a Library deposit i.e. the answer to a question may include a commitment to deposit papers in the Libraries of either House."@en ;
	rdfs:domain pqa:Answer ;
	rdfs:range pqa:LibraryDeposit ;
	rdfs:isDefinedBy <http://parliament.uk/ontologies/question-and-answer/> .
	
pqa:refersToDocument rdf:type owl:ObjectProperty ;
	rdfs:label "Refers to document"@en ;
	rdfs:comment "Relates a written answer to a document provided by the answering body. This may be provided as an attachment to the answer text. The document might form part or all of the answer."@en ;
	rdfs:domain pqa:Answer ;
	rdfs:range pqa:Document ;
	rdfs:isDefinedBy <http://parliament.uk/ontologies/question-and-answer/> .
	
pqa:answerExpectedAs rdf:type owl:ObjectProperty ;
	rdfs:label "Answer expected as"@en ;
	rdfs:comment "Relates a question to a time-bound means of capturing the format of the answer expected (either oral or written)."@en ;
	rdfs:domain pqa:Question ;
	rdfs:range pqa:AnswerExpectedAs ;
	rdfs:isDefinedBy <http://parliament.uk/ontologies/question-and-answer/> .
	
pqa:answerExpectedInForm rdf:type owl:ObjectProperty ;
	rdfs:label "Answer expected in form"@en ;
	rdfs:comment "Relates an answer being expected at at a point in time to the form the answer is expected in."@en ;
	rdfs:domain pqa:AnswerExpectedAs ;
	rdfs:range pqa:FormOfAnswer ;
	rdfs:isDefinedBy <http://parliament.uk/ontologies/question-and-answer/> .
	
pqa:changedFrom rdf:type owl:ObjectProperty ;
	rdfs:label "Changed from"@en ;
	rdfs:comment "Relates a change in the form of answer expected to the expectation prior to that change."@en ;
	rdfs:domain pqa:AnswerExpectedAsChange ;
	rdfs:range pqa:AnswerExpectedAs ;
	rdfs:isDefinedBy <http://parliament.uk/ontologies/question-and-answer/> .
	
pqa:changedTo rdf:type owl:ObjectProperty ;
	rdfs:label "Changed to"@en ;
	rdfs:comment "Relates a change in the form of answer expected to the expectation subsequent to that change."@en ;
	rdfs:domain pqa:AnswerExpectedAsChange ;
	rdfs:range pqa:AnswerExpectedAs ;
	rdfs:isDefinedBy <http://parliament.uk/ontologies/question-and-answer/> .

pqa:hasChangeReason rdf:type owl:ObjectProperty ;
	rdfs:label "Has change reason"@en ;
	rdfs:comment "Relates a change in the form of answer expected to the reason for that change."@en ;
	rdfs:domain pqa:AnswerExpectedAsChange ;
	rdfs:range pqa:AnswerExpectedAsChangeReason ;
	rdfs:isDefinedBy <http://parliament.uk/ontologies/question-and-answer/> .
		

#######  Data properties ##### 
	
pqa:dateForAnswer rdf:type owl:DatatypeProperty ;
	rdfs:label "Date for answer"@en ;
	rdfs:comment "Relates a Parliamentary Question to a date for answer. For an ordinary written question this is expected to be within 7 days of tabling. If the Member requests an earlier answer they must raise it as a named day question. See isDateForAnswerNamed."@en ;
	rdfs:domain pqa:ParliamentaryQuestion ;
	rdfs:range xsd:date ;
	rdfs:isDefinedBy <http://parliament.uk/ontologies/question-and-answer/> .
	
pqa:isDateForAnswerNamed rdf:type owl:DatatypeProperty ;
	rdfs:label "Is date for answer named"@en ;
	rdfs:comment "Determines if the Member tabling a written parliamentary question has requested that it be answered by a named day. Note that named day questions can only be tabled in the House of Commons. Most written questions are ordinary and the value here is false. By convention a Member can expect such questions to be answered within 7 days of tabling. Named day questions are used to elicit a faster response."@en ;
	rdfs:domain pqa:ParliamentaryQuestion ;
	rdfs:range xsd:boolean ;
	rdfs:isDefinedBy <http://parliament.uk/ontologies/question-and-answer/> .
	
pqa:heading rdf:type owl:DatatypeProperty ;
	rdfs:label "Heading"@en ;
	rdfs:comment "Relates a question to its heading text. For a written parliamentary question this is supplied by the Indexing and Data Management Section in the House of Commons Library. For oral parliamentary questions, the headings are supplied by Lords or Commons Hansard."@en ;
	rdfs:domain pqa:Question ;
	rdfs:range rdf:langString ;
	rdfs:isDefinedBy <http://parliament.uk/ontologies/question-and-answer/> .
	
pqa:questionText rdf:type owl:DatatypeProperty ;
	rdfs:label "Question text"@en ;
	rdfs:comment "Relates a question to the actual text of the question as asked by the Member."@en ;
	rdfs:domain pqa:Question ;
	rdfs:range rdf:langString ;
	rdfs:isDefinedBy <http://parliament.uk/ontologies/question-and-answer/> .
	
pqa:interestsDeclared rdf:type owl:DatatypeProperty ;
	rdfs:label "Interests declared"@en ;
	rdfs:comment "Indicates whether the Member asking the question has declared they have interests which may be relevant to the subject matter of the question."@en ;
	rdfs:domain pqa:Question ;
	rdfs:range xsd:boolean ;
	rdfs:isDefinedBy <http://parliament.uk/ontologies/question-and-answer/> .
	
pqa:isQuestionSubstantive rdf:type owl:DatatypeProperty ;
	rdfs:label "Is question substantive"@en ;
	rdfs:comment "Indicates if a question is substantive. If true the question text will be meaningful and constitute the actual question that the Member wished to ask. If false the question text will be boilerplate text asking about a government department or the Prime Minister's appointments (respectively topical questions and Prime Minister's questions in the House of Commons). This will be answered in the Chamber, after which the asking Member will ask a supplementary question. This is a device to enable Members to ask supplementary questions on any topical subject without notice. It only applies to parliamentary questions expecting an oral answer and only applies in the House of Commons. The process for topical questions in the House of Lords differs slightly from that in the House of Commons, in that all questions tabled are substantive. Here topical refers to the shorter notice period allowed when tabling a question."@en ;
	rdfs:domain pqa:ParliamentaryQuestion ;
	rdfs:range xsd:boolean ;
	rdfs:isDefinedBy <http://parliament.uk/ontologies/question-and-answer/> .	
	
pqa:answerText rdf:type owl:DatatypeProperty ;
	rdfs:label "Answer text"@en ;
	rdfs:comment "Relates an answer to the actual text of the answer as supplied by the answering body."@en ;
	rdfs:domain pqa:Answer ;
	rdfs:range rdf:langString ;
	rdfs:isDefinedBy <http://parliament.uk/ontologies/question-and-answer/> .	
	
pqa:isAnswerOral rdf:type owl:DatatypeProperty ;
	rdfs:label "Is answer oral"@en ;
	rdfs:comment "Determines if the answer is given orally in the Chamber. If true the answer is oral. If false the answer is written. The distinction only applies to answers to parliamentary questions. All other answers are always oral."@en ;
	rdfs:domain pqa:Answer ;
	rdfs:range xsd:boolean ;
	rdfs:isDefinedBy <http://parliament.uk/ontologies/question-and-answer/> .
	