@prefix related <http://parliament.uk/ontologies/related/> . 
@prefix xsd: <http://www.w3.org/2001/XMLSchema#> . 
@prefix rdf: <http://www.w3.org/1999/02/22-rdf-syntax-ns#> .
@prefix dcterms: <http://purl.org/dc/terms/> .
@prefix owl:     <http://www.w3.org/2002/07/owl#> .
@prefix rdfs:    <http://www.w3.org/2000/01/rdf-schema#> .
@prefix foaf:	<http://xmlns.com/foaf/0.1/> .

<http://parliament.uk/ontologies/related/> 
    rdf:type owl:Ontology ;
    dcterms:title "Related item ontology"@en ;
    dcterms:created "2023-03-23"^^xsd:date ;
	dcterms:rights "Open Parliament Licence v3.0"@en ;
    dcterms:description ""@en;
	foaf:depiction <https://ukparliament.github.io/ontologies/related/related.svg> ;
	foaf:maker 
		[ foaf:name "Jayne Bosworth" ],
		[ foaf:name "Robert Brook"; foaf:homepage <https://robert-brook.com/> ],
		[ foaf:name "Ned Morrell" ],
		[ foaf:name "Michael Smethurst"; foaf:homepage <http://smethur.st/> ],
		[ foaf:name "Anya Somerville" ].


#######  Classes #####
	
related:Thing rdf:type owl:Class ;
	rdfs:label "Thing"@en ;
	rdfs:comment "A thing."@en ;
	rdfs:isDefinedBy <http://parliament.uk/ontologies/related/> .
	
related:Relationship rdf:type owl:Class ;
	rdfs:label "Relationship"@en ;
	rdfs:comment "A relationship from a thing to either a thing or a document at a URI."@en ;
	rdfs:isDefinedBy <http://parliament.uk/ontologies/related/> .
	
related:DocumentType rdf:type owl:Class ;
	rdfs:label "DocumentType"@en ;
	rdfs:comment "The type of the document being cited, for example: a standing order or a section of legislation."@en ;
	rdfs:isDefinedBy <http://parliament.uk/ontologies/related/> .
	
related:RelationshipType rdf:type owl:Class ;
	rdfs:label "Relationship type"@en ;
	rdfs:comment "The type of a relationship."@en ;
	rdfs:isDefinedBy <http://parliament.uk/ontologies/related/> .
	

	
#######  Object properties ##### 

related:relationshipFrom rdf:type owl:ObjectProperty ;
	rdfs:label "Relationship from"@en ;
	rdfs:comment "Relates a relationship to the thing the relationship is from."@en ;
	rdfs:domain related:Relationship ;
	rdfs:range related:Thing ;
	rdfs:isDefinedBy <http://parliament.uk/ontologies/related/> .
	
related:relationshipTo rdf:type owl:ObjectProperty ;
	rdfs:label "Relationship to"@en ;
	rdfs:comment "Relates a relationship to the thing the relationship is to."@en ;
	rdfs:domain related:Relationship ;
	rdfs:range related:Thing ;
	rdfs:isDefinedBy <http://parliament.uk/ontologies/related/> .
	
related:hasDocumentType rdf:type owl:ObjectProperty ;
	rdfs:label "Has document type"@en ;
	rdfs:comment "Relates a relationship to the document type of the thing at the URI being related to."@en ;
	rdfs:domain related:Relationship ;
	rdfs:range related:DocumentType ;
	rdfs:isDefinedBy <http://parliament.uk/ontologies/related/> .
	
related:hasType rdf:type owl:ObjectProperty ;
	rdfs:label "Has type"@en ;
	rdfs:comment "Relates a relationship to its type."@en ;
	rdfs:domain related:Relationship ;
	rdfs:range related:RelationshipType ;
	rdfs:isDefinedBy <http://parliament.uk/ontologies/related/> .
	
related:inverse rdf:type owl:ObjectProperty ;
	rdfs:label "Inverse"@en ;
	rdfs:comment "Relates a relationship type to its inverse relationship type."@en ;
	rdfs:domain related:RelationshipType ;
	rdfs:range related:RelationshipType ;
	rdfs:isDefinedBy <http://parliament.uk/ontologies/related/> .
	
	

#######  Data properties #####

related:hasUri rdf:type owl:DatatypeProperty ;
	rdfs:label "Has URI"@en ;
	rdfs:comment "Relates a relationship to the URI of the thing being related to."@en ;
	rdfs:domain related:Relationship ;
	rdfs:range rdfs:Literal ;
	rdfs:isDefinedBy <http://parliament.uk/ontologies/related/> .