@prefix related-item: <http://parliament.uk/ontologies/related-item/> . 
@prefix xsd: <http://www.w3.org/2001/XMLSchema#> . 
@prefix rdf: <http://www.w3.org/1999/02/22-rdf-syntax-ns#> .
@prefix dcterms: <http://purl.org/dc/terms/> .
@prefix owl:     <http://www.w3.org/2002/07/owl#> .
@prefix rdfs:    <http://www.w3.org/2000/01/rdf-schema#> .
@prefix foaf:	<http://xmlns.com/foaf/0.1/> .

<http://parliament.uk/ontologies/related-item/> 
    rdf:type owl:Ontology ;
    dcterms:title "Related item ontology"@en ;
    dcterms:created "2023-03-23"^^xsd:date ;
	dcterms:rights "Open Parliament Licence v3.0"@en ;
    dcterms:description "Provides a means to link from a modelled thing to either another modelled thing or a thing at a URI by means of a typed relationship."@en;
	foaf:depiction <https://ukparliament.github.io/ontologies/related-item/related-item.svg> ;
	foaf:maker 
		[ foaf:name "Jayne Bosworth" ],
		[ foaf:name "Robert Brook"; foaf:homepage <https://robert-brook.com/> ],
		[ foaf:name "Ned Morrell" ],
		[ foaf:name "Michael Smethurst"; foaf:homepage <http://smethur.st/> ],
		[ foaf:name "Anya Somerville" ].


#######  Classes #####
	
related-item:Thing rdf:type owl:Class ;
	rdfs:label "Thing"@en ;
	rdfs:comment "A thing."@en ;
	rdfs:isDefinedBy <http://parliament.uk/ontologies/related-item/> .
	
related-item:Relationship rdf:type owl:Class ;
	rdfs:label "Relationship"@en ;
	rdfs:comment "A relationship from a modelled thing to either another modelled thing or a document at a URI."@en ;
	rdfs:isDefinedBy <http://parliament.uk/ontologies/related-item/> .
	
related-item:RelationshipType rdf:type owl:Class ;
	rdfs:label "Relationship type"@en ;
	rdfs:comment "The type of a relationship, for example: cites, announces, corrects or commits to."@en ;
	rdfs:isDefinedBy <http://parliament.uk/ontologies/related-item/> .
	
related-item:WebDocument rdf:type owl:Class ;
	rdfs:label "Web document"@en ;
	rdfs:comment "A document available on the web."@en ;
	rdfs:isDefinedBy <http://parliament.uk/ontologies/related-item/> .
	
related-item:DocumentType rdf:type owl:Class ;
	rdfs:label "DocumentType"@en ;
	rdfs:comment "The type of the document being cited, for example: a standing order or legislation."@en ;
	rdfs:isDefinedBy <http://parliament.uk/ontologies/related-item/> .
	

	

	
#######  Object properties ##### 

related-item:relationshipFromThing rdf:type owl:ObjectProperty ;
	rdfs:label "Relationship from thing"@en ;
	rdfs:comment "Relates a relationship to the thing the relationship relates from. A relationship relates from one thing."@en ;
	rdfs:domain related-item:Relationship ;
	rdfs:range related-item:Thing ;
	rdfs:isDefinedBy <http://parliament.uk/ontologies/related-item/> .
	
related-item:relationshipToThing rdf:type owl:ObjectProperty ;
	rdfs:label "Relationship to things"@en ;
	rdfs:comment "Relates a relationship to the thing the relationship relates to. A relationship relates to one thing, or none."@en ;
	rdfs:domain related-item:Relationship ;
	rdfs:range related-item:Thing ;
	rdfs:isDefinedBy <http://parliament.uk/ontologies/related-item/> .
	
related-item:hasRelationshipType rdf:type owl:ObjectProperty ;
	rdfs:label "Has relationship type"@en ;
	rdfs:comment "Relates a relationship to its type. A relationship is of one type."@en ;
	rdfs:domain related-item:Relationship ;
	rdfs:range related-item:RelationshipType ;
	rdfs:isDefinedBy <http://parliament.uk/ontologies/related-item/> .

related-item:inverse rdf:type owl:ObjectProperty ;
	rdfs:label "Inverse"@en ;
	rdfs:comment "Relates a relationship type to its inverse relationship type, for example: corrects to corrected by."@en ;
	rdfs:domain related-item:RelationshipType ;
	rdfs:range related-item:RelationshipType ;
	rdfs:isDefinedBy <http://parliament.uk/ontologies/related-item/> .
	
related-item:relationshipToWebDocument rdf:type owl:ObjectProperty ;
	rdfs:label "Relationship to web document"@en ;
	rdfs:comment "Relates a relationship to a web document. A relationship relates to one web document, or none."@en ;
	rdfs:domain related-item:Relationship ;
	rdfs:range related-item:Thing ;
	rdfs:isDefinedBy <http://parliament.uk/ontologies/related-item/> .
	
related-item:hasDocumentType rdf:type owl:ObjectProperty ;
	rdfs:label "Has document type"@en ;
	rdfs:comment "Relates a web document to its type. A web document has one document type, or none."@en ;
	rdfs:domain related-item:WebDocument ;
	rdfs:range related-item:DocumentType ;
	rdfs:isDefinedBy <http://parliament.uk/ontologies/related-item/> .
	


#######  Data properties #####

related-item:uri rdf:type owl:DatatypeProperty ;
	rdfs:label "URI"@en ;
	rdfs:comment "Relates a web document to its URI."@en ;
	rdfs:domain related-item:WebDocument ;
	rdfs:range rdfs:Literal ;
	rdfs:isDefinedBy <http://parliament.uk/ontologies/related-item/> .