@prefix papertype: <http://parliament.uk/ontologies/paper-type/> . 
@prefix xsd: <http://www.w3.org/2001/XMLSchema#> . 
@prefix rdf: <http://www.w3.org/1999/02/22-rdf-syntax-ns#> .
@prefix dcterms: <http://purl.org/dc/terms/> .
@prefix owl:     <http://www.w3.org/2002/07/owl#> .
@prefix rdfs:    <http://www.w3.org/2000/01/rdf-schema#> .
@prefix foaf:	<http://xmlns.com/foaf/0.1/> .

<http://parliament.uk/ontologies/paper-type/> 
    rdf:type owl:Ontology ;
    dcterms:title "Paper type ontology"@en ;
    dcterms:created "2023-01-19"^^xsd:date ;
	dcterms:rights "Open Parliament Licence v3.0"@en ;
    dcterms:description "A model describing the relationships between types of papers."@en ;
	foaf:depiction <https://ukparliament.github.io/ontologies/paper-type/paper-type.svg> ;
	foaf:maker
		[ foaf:name "Jayne Bosworth" ],
		[ foaf:name "Robert Brook"; foaf:homepage <https://robert-brook.com/> ],
		[ foaf:name "Claire Searle" ],
		[ foaf:name "Michael Smethurst"; foaf:homepage <http://smethur.st/> ],
		[ foaf:name "Anya Somerville" ].
		
		
		
#######  Classes ##### 	

papertype:PaperExpression rdf:type owl:Class ;
	rdfs:label "Paper expression"@en ;
	rdfs:comment "A paper made available to a House, being an expression of a paper work."@en ;
	rdfs:isDefinedBy <http://parliament.uk/ontologies/paper-type/> .
	
papertype:TreatyExpression rdf:type owl:Class ;
	rdfs:subClassOf papertype:PaperExpression ;
	rdfs:label "Treaty expression"@en ;
	rdfs:comment "A written agreement between states - or between states and international organisations - which is binding under international law."@en ;
	rdfs:isDefinedBy <http://parliament.uk/ontologies/paper-type/> .
	
papertype:ExplanatoryMemorandumExpression rdf:type owl:Class ;
	rdfs:subClassOf papertype:PaperExpression ;
	rdfs:label "Explanatory memorandum expression"@en ;
	rdfs:comment "A paper intended to explain the purpose, policy objectives and policy implications of an instrument being subject to parliamentary procedure."@en ;
	rdfs:isDefinedBy <http://parliament.uk/ontologies/paper-type/> .
	
papertype:ExplanatoryNoteExpression rdf:type owl:Class ;
	rdfs:subClassOf papertype:PaperExpression ;
	rdfs:label "Explanatory note expression"@en ;
	rdfs:comment "A paper intended to explain the purpose of a bill."@en ;
	rdfs:isDefinedBy <http://parliament.uk/ontologies/paper-type/> .
	
papertype:BillExpression rdf:type owl:Class ;
	rdfs:subClassOf papertype:PaperExpression ;
	rdfs:label "Bill expression"@en ;
	rdfs:comment "An expression of a bill work at a point in time. A new expression of the bill work is created by any amendment being made to the bill, or when a bill passes from the first House to the second House."@en ;
	rdfs:isDefinedBy <http://parliament.uk/ontologies/paper-type/> .
	
papertype:BillWork rdf:type owl:Class ;
	rdfs:label "Bill work"@en ;
	rdfs:comment "A proposal for a new Act of Parliament."@en ;
	rdfs:isDefinedBy <http://parliament.uk/ontologies/paper-type/> .
	
papertype:EnabledThing rdf:type owl:Class ;
	rdfs:subClassOf papertype:PaperExpression ;
	rdfs:label "Enabled thing"@en ;
	rdfs:comment "A thing which is intended to exercise a power set out in statute."@en ;
	rdfs:isDefinedBy <http://parliament.uk/ontologies/paper-type/> .
	
papertype:ImpactAssessmentExpression rdf:type owl:Class ;
	rdfs:subClassOf papertype:PaperExpression ;
	rdfs:label "Impact assessment expression"@en ;
	rdfs:comment "A paper, provided by the government, intended to set out the objectives of policy proposals and the costs, benefits and risks of different ways of achieving those objectives."@en ;
	rdfs:isDefinedBy <http://parliament.uk/ontologies/paper-type/> .
		
		
		
#######  Object properties ##### 
	
papertype:enabledThingHasImpactAssessment rdf:type owl:ObjectProperty ;
	rdfs:label "Enabled thing has impact assessment"@en ;
	rdfs:comment "Relates an enabled thing to the impact assessment for that thing. An enabled thing has one or more impact assessments, or none."@en ;
	rdfs:domain papertype:EnabledThing ;
	rdfs:range papertype:ImpactAssessmentExpression ;
	rdfs:isDefinedBy <http://parliament.uk/ontologies/paper-type/> .
	
papertype:treatyHasExplanatoryMemorandum rdf:type owl:ObjectProperty ;
	rdfs:label "Treaty has explanatory memorandum"@en ;
	rdfs:comment "Relates a treaty expression to the explanatory memorandum for that treaty expression. A treaty expression has one or more explanatory memoranda, or none."@en ;
	rdfs:domain papertype:TreatyExpression ;
	rdfs:range papertype:ExplanatoryMemorandumExpression ;
	rdfs:isDefinedBy <http://parliament.uk/ontologies/paper-type/> .
	
papertype:enabledThingHasExplanatoryMemorandum rdf:type owl:ObjectProperty ;
	rdfs:label "Enabled thing has explanatory memorandum"@en ;
	rdfs:comment "Relates an enabled thing to the explanatory memorandum for that thing. An enabled thing has one or more explanatory memoranda, or none."@en ;
	rdfs:domain papertype:EnabledThing ;
	rdfs:range papertype:ExplanatoryMemorandumExpression ;
	rdfs:isDefinedBy <http://parliament.uk/ontologies/paper-type/> .
	
papertype:hasExplanatoryNote rdf:type owl:ObjectProperty ;
	rdfs:label "Has explanatory note"@en ;
	rdfs:comment "Relates a bill expression to the explanatory note for that expression. A bill expression has one or more explanatory notes, or none."@en ;
	rdfs:domain papertype:BillExpression ;
	rdfs:range papertype:ExplanatoryNoteExpression ;
	rdfs:isDefinedBy <http://parliament.uk/ontologies/paper-type/> .
	
papertype:billHasImpactAssessment rdf:type owl:ObjectProperty ;
	rdfs:label "Bill has impact assessment"@en ;
	rdfs:comment "Relates a bill work to the impact assessment for that work. A bill work has one or more impact assessments, or none."@en ;
	rdfs:domain papertype:BillWork ;
	rdfs:range papertype:ImpactAssessmentExpression ;
	rdfs:isDefinedBy <http://parliament.uk/ontologies/paper-type/> .