@prefix ppapertype: <http://parliament.uk/ontologies/parliamentary-paper-type/> . 
@prefix xsd: <http://www.w3.org/2001/XMLSchema#> . 
@prefix rdf: <http://www.w3.org/1999/02/22-rdf-syntax-ns#> .
@prefix dcterms: <http://purl.org/dc/terms/> .
@prefix owl:     <http://www.w3.org/2002/07/owl#> .
@prefix rdfs:    <http://www.w3.org/2000/01/rdf-schema#> .
@prefix foaf:	<http://xmlns.com/foaf/0.1/> .

<http://parliament.uk/ontologies/parliamentary-paper-type/> 
    rdf:type owl:Ontology ;
    dcterms:title "Parliamentary paper type ontology"@en ;
    dcterms:created "2023-01-19"^^xsd:date ;
	dcterms:rights "Open Parliament Licence v3.0"@en ;
    dcterms:description ""@en ;
	foaf:depiction <https://ukparliament.github.io/ontologies/parliamentary-paper-type/parliamentary-paper-type.svg> ;
	foaf:maker
		[ foaf:name "Jayne Bosworth" ],
		[ foaf:name "Claire Searle" ],
		[ foaf:name "Michael Smethurst"; foaf:homepage <http://smethur.st/> ],
		[ foaf:name "Anya Somerville" ].
		
		
		
#######  Classes ##### 	

ppapertype:ParliamentaryPaperWork rdf:type owl:Class ;
	rdfs:label "Parliamentary paper work"@en ;
	rdfs:comment "A parliamentary paper as a single intellectual work, as defined in the Functional Requirements for Bibliographic Records specification."@en ;
	rdfs:isDefinedBy <http://parliament.uk/ontologies/parliamentary-paper/> .
	
	
	
	
	
	
	
	
				

#######  Object properties ##### 
	
ppaper:expressionOf rdf:type owl:ObjectProperty ;
	rdfs:label "Expression of"@en ;
	rdfs:comment "Relates a parliamentary paper expression to the work that paper is an expression of. A parliamentary paper expression is an expression of one parliamentary paper work. A parliamentary paper work is expressed as one or more parliamentary papers."@en ;
	rdfs:domain ppaper:ParliamentaryPaperExpression ;
	rdfs:range ppaper:ParliamentaryPaperWork ;
	rdfs:isDefinedBy <http://parliament.uk/ontologies/parliamentary-paper/> .

	
	
#######  Data properties ##### 

ppaper:prefix rdf:type owl:DatatypeProperty ;
	rdfs:label "Prefix"@en ;
	rdfs:comment "Relates a paper series to the prefix which is combined with a paper series item identifier to form the 'number' of a parliamentary paper as an item in that series."@en ;
	rdfs:domain ppaper:PaperSeries ;
	rdfs:range rdfs:Literal ;
	rdfs:isDefinedBy <http://parliament.uk/ontologies/parliamentary-paper/> .