@prefix pfb: <http://parliament.uk/ontologies/formal-body/> . 
@prefix xsd: <http://www.w3.org/2001/XMLSchema#> . 
@prefix rdf: <http://www.w3.org/1999/02/22-rdf-syntax-ns#> .
@prefix dcterms: <http://purl.org/dc/terms/> .
@prefix owl:     <http://www.w3.org/2002/07/owl#> .
@prefix rdfs:    <http://www.w3.org/2000/01/rdf-schema#> .
@prefix foaf:	<http://xmlns.com/foaf/0.1/> .

<http://parliament.uk/ontologies/formal-body/> 
    rdf:type owl:Ontology ;
    dcterms:title "Formal body ontology"@en ;
    dcterms:created "2017-08-29"^^xsd:date ;
	dcterms:rights "Open Parliament Licence v3.0"@en ;
    dcterms:description "An ontology describing formally constituted bodies, including committees."@en ;
	foaf:depiction <https://ukparliament.github.io/ontologies/formal-body/formal-body.png> ;
	foaf:maker
		[ foaf:name "James Bowman" ],
		[ foaf:name "Robert Brook"; foaf:homepage <https://robert-brook.com/> ],
		[ foaf:name "Gordon Clark" ],
		[ foaf:name "Edward McCarthy" ],
		[ foaf:name "Silver Oliver" ],
		[ foaf:name "Michael Smethurst"; foaf:homepage <http://smethur.st/> ],
	    [ foaf:name "Anya Somerville" ].


#######  Classes ##### 	

pfb:FormalBody rdf:type owl:Class ;
	rdfs:label "Formal body"@en ;
	rdfs:comment "A group formally constituted by Parliament to conduct specific business within Parliament, for example: a committee or a group acting as a committee. Formal groups are subject to parliamentary procedure and operate under parliamentary privilege. A formal body may be established by means of procedure - for example: by Standing Order - or by another process, for example: selection of the Advisory Panel on Works of Art by the Lords’ Speaker. A formal body may be established under statute, for example: the Intelligence and Security Committee of Parliament, by means of the Intelligence Services Act 1994 and the Justice and Security Act 2013. People in a formal body are Members of the House of Commons or of the House of Lords. A formal body may be joint, taking membership from both Houses. Groups with informally constituted memberships are not formal groups, for example: All-Party Parliamentary Groups. Informally constituted groups are not subject to parliamentary procedure and do not operate under parliamentary privilege."@en ;
	rdfs:isDefinedBy <http://parliament.uk/ontologies/formal-body/> .
	
pfb:ParliamentaryCommittee rdf:type owl:Class ;
	rdfs:subClassOf pfb:FormalBody ;
	rdfs:label "Parliamentary committee"@en ;
	rdfs:comment "A parliamentary committee is constituted and has members appointed by one or both Houses, by means of a motion or Standing Order."@en ;
	rdfs:isDefinedBy <http://parliament.uk/ontologies/formal-body/> .

pfb:SelectCommittee rdf:type owl:Class ;
	rdfs:subClassOf pfb:ParliamentaryCommittee ;
	rdfs:label "Select Committee"@en ;
	rdfs:comment "There are Select Committees in both the House of Commons and the House of Lords. Select Committees conduct inquiries into and report on matters as directed by their remit. The results of inquiries are public. The government may be expected to respond to a published inquiry. Select Committees in the House of Commons are primarily concerned with examining the work of government departments. Select Committees in the House of Lords concentrate on broader themes rather than on individual government departments. When a Select Committee in the House of Lords is not deliberating, any peer may attend and speak at the committee. When a Select Committee in the House of Lords is deliberating, peers without membership of the committee may not attend, unless invited by the Committee to do so. Any peer not being a member of a Select Committee in the House of Lords cannot vote in that committee."@en ;
	rdfs:isDefinedBy <http://parliament.uk/ontologies/formal-body/> .

pfb:GeneralCommittee rdf:type owl:Class ;
	rdfs:subClassOf pfb:ParliamentaryCommittee ;
	rdfs:label "General Committee"@en ;
	rdfs:comment "The House of Commons has General Committees: their primary role is to consider proposed legislation. The House of Lords does not have General Committees, meeting as a whole House to consider proposed legislation. General Committees include Committees on Bills, Grand Committees considering matters specific to the devolved nations of the UK, and General Committees on delegated legislation and European documents."@en ;
	rdfs:isDefinedBy <http://parliament.uk/ontologies/formal-body/> .

pfb:NonSelectCommittee rdf:type owl:Class ;
	rdfs:subClassOf pfb:ParliamentaryCommittee ;
	rdfs:label "Non-Select Committee"@en ;
	rdfs:comment "The House of Lords has non-Select Committees, fulfilling a similar function to the General Committees of the House of Commons. Any Peer may attend, speak and vote in a non-Select Committee - including those not being members of the committee."@en ;
	rdfs:isDefinedBy <http://parliament.uk/ontologies/formal-body/> .

pfb:StatutoryCommittee rdf:type owl:Class ;
	rdfs:subClassOf pfb:FormalBody ;
	rdfs:label "Statutory Committee"@en ;
	rdfs:comment "Statutory Committees are committees constituted by means of legislation, for example: the Ecclesiastical Committee, by the Church of England Assembly (Powers) Act 1919."@en ;
	rdfs:isDefinedBy <http://parliament.uk/ontologies/formal-body/> .

pfb:InformallyConstitutedCommittee rdf:type owl:Class ;
	rdfs:subClassOf pfb:FormalBody ;
	rdfs:label "Informally constituted committee"@en ;
	rdfs:comment "An informally constituted committee is a committee-like formal body, not established under Parliamentary procedure or by statute."@en ;
	rdfs:isDefinedBy <http://parliament.uk/ontologies/formal-body/> .

pfb:FocusCategory rdf:type owl:Class ;
	rdfs:label "Focus category"@en ;
	rdfs:comment "A focus category provides a way to aggregate formal bodies by the type of thing they focus on or scrutinise, for example: a type of legislation, one or more government departments, matters specific to devolved nations. Eventually, the type of the thing focussed on may be derived from any ‘focus’ relationships, together with the types of the things being focussed on. Presently, the things that focus categories point at have insufficient definition to support a determination of their type, for example: the Scottish Grand Committee would have a library subject heading or concept of Scotland as a focus category, typed as a geographic entity rather than as a devolved nation. Aggregating a list of formal bodies with a focus on devolved nations would not be possible from the 'focus' relationships alone: the focus category gives a higher level means to group formal bodies by interest areas. A focus category is able to be populated regardless of whether the thing focussed on is sufficiently defined, for example: 'focus' may point to a named item of legislation, with the focus category recording that the formal body was constituted to scrutinise a specific item of legislation but without identifying which."@en ;
	rdfs:isDefinedBy <http://parliament.uk/ontologies/formal-body/> .
	
pfb:House rdf:type owl:Class ;
	rdfs:label "House"@en ;
	rdfs:comment "A parliamentary House, for example: the House of Lords"@en ;
	rdfs:isDefinedBy <http://parliament.uk/ontologies/formal-body/> .
	
pfb:WorkPackage rdf:type owl:Class ;
	rdfs:label "Work package"@en ;
	rdfs:comment "A group of business items under a procedure or as determined by a committee, for example: business items considered during the passage of a particular Statutory Instrument or Public Bill, or during an inquiry by a Select Committee."@en ;
	rdfs:isDefinedBy <http://parliament.uk/ontologies/formal-body/> .

pfb:Inquiry rdf:type owl:Class ;
	rdfs:subClassOf pfb:WorkPackage ;
	rdfs:label "Inquiry"@en ;
	rdfs:comment "A type of work package investigating a specific subject or policy area."@en ;
	rdfs:isDefinedBy <http://parliament.uk/ontologies/formal-body/> .
		
pfb:InquiryScope rdf:type owl:Class ;
	rdfs:label "Inquiry scope"@en ;
	rdfs:comment "The scope or terms of reference of an inquiry, setting out the context, constraints and questions which the inquiry seeks to address."@en ;
	rdfs:isDefinedBy <http://parliament.uk/ontologies/formal-body/> .
	
pfb:WorkPackageType rdf:type owl:Class ;
	rdfs:label "Work package type"@en ;
	rdfs:comment "A description of the type of a work package. Whilst inquiries have a specific Inquiry subclass, work package type describes work packages which are not associated with inquiries, for example: a collection of hearings before a person is appointed to a public body or a set of hearings where a government minister appears before a committee."@en ;
	rdfs:isDefinedBy <http://parliament.uk/ontologies/formal-body/> .
	
pfb:BusinessItem rdf:type owl:Class ;
	rdfs:label "Business item"@en ;
	rdfs:comment "An item of business conducted either within or outside Parliament, for example: a second reading debate, the tabling of an Early Day Motion, a laying of a paper, the making of a Statutory Instrument by a government minister."@en ;
	rdfs:isDefinedBy <http://parliament.uk/ontologies/formal-body/> .
	
pfb:Focus rdf:type owl:Class ;
	rdfs:label "Focus"@en ;
	rdfs:comment "A focus area for a formal body or work package, for example: a government department, a type of legislation, an item of legislation or a SKOS type concept."@en ;
	rdfs:isDefinedBy <http://parliament.uk/ontologies/formal-body/> .
	
	# edited to here
	
	
#######  Object properties ##### 

pfb:belongsToHouse rdf:type owl:ObjectProperty ;
	rdfs:label "Belongs to House"@en ;
	rdfs:comment "Relates a formal body to the House or Houses it belongs to. A joint committee will belong to both Houses."@en ;
	rdfs:domain pfb:FormalBody ;
	rdfs:range pfb:House ;
	rdfs:isDefinedBy <http://parliament.uk/ontologies/formal-body/> .

pfb:hasLeadHouse rdf:type owl:ObjectProperty ;
	rdfs:label "Has lead House"@en ;
	rdfs:comment "A joint committee will have a lead House responsible for its administration."@en ;
	rdfs:domain pfb:FormalBody ;
	rdfs:range pfb:House ;
	rdfs:isDefinedBy <http://parliament.uk/ontologies/formal-body/> .
	
pfb:hasParentFormalBody rdf:type owl:ObjectProperty ;
	rdfs:label "Has parent formal body"@en ;
	rdfs:comment "Allows for committees to have sub-committees and sub-committees to have parent committees."@en ;
	rdfs:domain pfb:FormalBody ;
	rdfs:range pfb:FormalBody ;
	rdfs:isDefinedBy <http://parliament.uk/ontologies/formal-body/> .
	
pfb:undertakesWorkPackage rdf:type owl:ObjectProperty ;
	rdfs:label "Undertakes work package"@en ;
	rdfs:comment "Allows for formal bodies to take on work packages like inquiries. A joint inquiry will have more than one associated formal body."@en ;
	rdfs:domain pfb:FormalBody ;
	rdfs:range pfb:WorkPackage ;
	rdfs:isDefinedBy <http://parliament.uk/ontologies/formal-body/> .

pfb:hasParentWorkPackage rdf:type owl:ObjectProperty ;
	rdfs:label "Has parent work package"@en ;
	rdfs:comment "Allows for work packages to have parent work packages. e.g. a sub-inquiry can belong to a wider inquiry."@en ;
	rdfs:domain pfb:WorkPackage ;
	rdfs:range pfb:WorkPackage ;
	rdfs:isDefinedBy <http://parliament.uk/ontologies/formal-body/> .
	
pfb:hasInquiryScope rdf:type owl:ObjectProperty ;
	rdfs:label "Has inquiry scope"@en ;
	rdfs:comment "Relates an inquiry to its scope or terms of reference."@en ;
	rdfs:domain pfb:Inquiry ;
	rdfs:range pfb:InquiryScope ;
	rdfs:isDefinedBy <http://parliament.uk/ontologies/formal-body/> .
	
pfb:hasWorkPackageType rdf:type owl:ObjectProperty ;
	rdfs:label "Has work package type"@en ;
	rdfs:comment "Defines the type of a work package where the work package is not an inquiry."@en ;
	rdfs:domain pfb:WorkPackage ;
	rdfs:range pfb:WorkPackageType ;
	rdfs:isDefinedBy <http://parliament.uk/ontologies/formal-body/> .
	
pfb:formsPartOf rdf:type owl:ObjectProperty ;
	rdfs:label "Forms part of"@en ;
	rdfs:comment "Relates a business item to a work package it forms part of. One or more business items may form part of a work package. A business item may form part of one or more work packages. For example, a meeting of the Joint Committee on Statutory Instruments may consider one or more SIs, each SI being the focus of a separate work package."@en ;
	rdfs:domain pfb:BusinessItem ;
	rdfs:range pfb:WorkPackage ;
	rdfs:isDefinedBy <http://parliament.uk/ontologies/formal-body/> .
	
pfb:hasAgent rdf:type owl:ObjectProperty ;
	rdfs:label "Has agent"@en ;
	rdfs:comment "Associates a business item with the formal body responsible for organising it. A business item may be run by more than one formal body. For example, a joint evidence session."@en ;
	rdfs:domain pfb:BusinessItem ;
	rdfs:range pfb:FormalBody ;
	rdfs:isDefinedBy <http://parliament.uk/ontologies/formal-body/> .
	
pfb:formalBodyFocus rdf:type owl:ObjectProperty ;
	rdfs:label "Formal body focus"@en ;
	rdfs:comment "Associates a formal body with its area of focus."@en ;
	rdfs:domain pfb:FormalBody ;
	rdfs:range pfb:Focus ;
	rdfs:isDefinedBy <http://parliament.uk/ontologies/formal-body/> .

pfb:workPackageFocus rdf:type owl:ObjectProperty ;
	rdfs:label "Work package focus"@en ;
	rdfs:comment "Associates a work package with its area of focus."@en ;
	rdfs:domain pfb:WorkPackage ;
	rdfs:range pfb:Focus ;
	rdfs:isDefinedBy <http://parliament.uk/ontologies/formal-body/> .

pfb:hasFocusCategory rdf:type owl:ObjectProperty ;
	rdfs:label "Has focus category"@en ;
	rdfs:comment "Relates a formal body to its focus category."@en ;
	rdfs:domain pfb:FormalBody ;
	rdfs:range pfb:FocusCategory ;
	rdfs:isDefinedBy <http://parliament.uk/ontologies/formal-body/> .
				

#######  Data properties ##### 

pfb:remit rdf:type owl:DatatypeProperty ;
	rdfs:label "Remit"@en ;
	rdfs:comment "The task or area of activity officially assigned to a formal body. This is a textual description as opposed to Focus which points at entities to describe the areas to be examined."@en ;
	rdfs:domain pfb:FormalBody ;
	rdfs:range rdf:langString ;
	rdfs:isDefinedBy <http://parliament.uk/ontologies/formal-body/> .