@prefix ppaper: <http://parliament.uk/ontologies/parliamentary-paper/> . 
@prefix xsd: <http://www.w3.org/2001/XMLSchema#> . 
@prefix rdf: <http://www.w3.org/1999/02/22-rdf-syntax-ns#> .
@prefix dcterms: <http://purl.org/dc/terms/> .
@prefix owl:     <http://www.w3.org/2002/07/owl#> .
@prefix rdfs:    <http://www.w3.org/2000/01/rdf-schema#> .
@prefix foaf:	<http://xmlns.com/foaf/0.1/> .

<http://parliament.uk/ontologies/parliamentary-paper/> 
    rdf:type owl:Ontology ;
    dcterms:title "Parliamentary paper ontology"@en ;
    dcterms:created "2022-07-11"^^xsd:date ;
	dcterms:rights "Open Parliament Licence v3.0"@en ;
    dcterms:description "A model describing"@en ;
	foaf:depiction <https://ukparliament.github.io/ontologies/parliamentary-paper/parliamentary-paper.svg> ;
	foaf:maker
		[ foaf:name "Jayne Bosworth" ],
		[ foaf:name "Robert Brook"; foaf:homepage <https://robert-brook.com/> ],
		[ foaf:name "Ned Morrell" ],
		[ foaf:name "Michael Smethurst"; foaf:homepage <http://smethur.st/> ],
		[ foaf:name "Anya Somerville" ].


#######  Classes ##### 	

ppaper:ParliamentaryPaperWork rdf:type owl:Class ;
	rdfs:label "Parliamentary paper work"@en ;
	rdfs:comment "A parliamentary paper made available to Parliament as realised in an expression made available to a House."@en ;
	rdfs:isDefinedBy <http://parliament.uk/ontologies/parliamentary-paper/> .
	
ppaper:ParliamentaryPaper rdf:type owl:Class ;
	rdfs:label "Parliamentary paper"@en ;
	rdfs:comment "The expression of a parliamentary paper work as made available to a House."@en ;
	rdfs:isDefinedBy <http://parliament.uk/ontologies/parliamentary-paper/> .
	
ppaper:PaperBundle rdf:type owl:Class ;
	rdfs:label "Paper bundle"@en ;
	rdfs:comment "A bundle of related parliamentary papers, for example: a bundle containing a statutory instrument paper and its related explanatory memorandum."@en ;
	rdfs:isDefinedBy <http://parliament.uk/ontologies/parliamentary-paper/> .
	
ppaper:PaperType rdf:type owl:Class ;
	rdfs:label "Paper type"@en ;
	rdfs:comment "The type of a paper, for example: a bill, a statutory instrument, a petition, a written statement or a set of annual accounts."@en ;
	rdfs:isDefinedBy <http://parliament.uk/ontologies/parliamentary-paper/> .
	
ppaper:PaperSeriesItem rdf:type owl:Class ;
	rdfs:label "Paper series item"@en ;
	rdfs:comment "A parliamentary paper as it exists as part of a paper series. A parliamentary paper forming part of a series may result in the paper being 'numbered' as part of that series."@en ;
	rdfs:isDefinedBy <http://parliament.uk/ontologies/parliamentary-paper/> .
	
ppaper:PaperSeries rdf:type owl:Class ;
	rdfs:label "Paper series"@en ;
	rdfs:comment "A series of parliamentary papers, for example: the Treaty Series."@en ;
	rdfs:isDefinedBy <http://parliament.uk/ontologies/parliamentary-paper/> .
	
ppaper:Session rdf:type owl:Class ;
	rdfs:label "Session"@en ;
	rdfs:comment "A period during which Parliament is able to conduct business on days of its choosing. A session is within a Parliament period. The first session of a Parliament begins on the same day as the Parliament period and ends on a day named in a subsequent prorogation proclamation. Subsequent sessions within the Parliament period begin and end on dates named in subsequent prorogation proclamations. The final session of a Parliament ends either with prorogation followed by dissolution or with dissolution. Session periods are the same for both Houses."@en ;
	rdfs:isDefinedBy <http://parliament.uk/ontologies/parliamentary-paper/> .
	
				

#######  Object properties ##### 
	
ppaper:expressionOf rdf:type owl:ObjectProperty ;
	rdfs:label "Expression of"@en ;
	rdfs:comment "Relates a parliamentary paper to the work the paper is an expression of. A parliamentary paper is an expression of one work. A parliamentary paper work may be expressed by one or more parliamentary papers."@en ;
	rdfs:domain ppaper:ParliamentaryPaper ;
	rdfs:range ppaper:ParliamentaryPaperWork ;
	rdfs:isDefinedBy <http://parliament.uk/ontologies/parliamentary-paper/> .
	
ppaper:formsPartOf rdf:type owl:ObjectProperty ;
	rdfs:label "Forms part of"@en ;
	rdfs:comment "Relates a parliamentary paper to the paper bundle it forms part of. A parliamentary paper may belong to one or more paper bundles, or none."@en ;
	rdfs:domain ppaper:ParliamentaryPaper ;
	rdfs:range ppaper:PaperBundle ;
	rdfs:isDefinedBy <http://parliament.uk/ontologies/parliamentary-paper/> .

ppaper:hasType rdf:type owl:ObjectProperty ;
	rdfs:label "Has type"@en ;
	rdfs:comment "Relates a parliamentary paper to its type. A parliamentary paper may have one or more types."@en ;
	rdfs:domain ppaper:ParliamentaryPaper ;
	rdfs:range ppaper:PaperType ;
	rdfs:isDefinedBy <http://parliament.uk/ontologies/parliamentary-paper/> .

ppaper:paperTypeParent rdf:type owl:ObjectProperty ;
	rdfs:label "Paper type parent"@en ;
	rdfs:comment "Relates a paper type to its parent paper type. A paper type may have one or more parent paper types, or none.  A paper type may have one or more child paper types, or none."@en ;
	rdfs:domain ppaper:PaperType ;
	rdfs:range ppaper:PaperType ;
	rdfs:isDefinedBy <http://parliament.uk/ontologies/parliamentary-paper/> .

ppaper:positionsParliamentaryPaper rdf:type owl:ObjectProperty ;
	rdfs:label "Positions parliamentary paper"@en ;
	rdfs:comment "Relates the existence of a parliamentary paper in a series to that parliamentary paper. A paper series item refers to one parliamentary paper."@en ;
	rdfs:domain ppaper:PaperSeriesItem ;
	rdfs:range ppaper:ParliamentaryPaper ;
	rdfs:isDefinedBy <http://parliament.uk/ontologies/parliamentary-paper/> .

ppaper:inSeries rdf:type owl:ObjectProperty ;
	rdfs:label "In series"@en ;
	rdfs:comment "Relates the existence of a parliamentary paper in a series to the series it forms part of. A paper series item forms part of one paper series."@en ;
	rdfs:domain ppaper:PaperSeriesItem ;
	rdfs:range ppaper:PaperSeries ;
	rdfs:isDefinedBy <http://parliament.uk/ontologies/parliamentary-paper/> .

ppaper:paperSeriesParent rdf:type owl:ObjectProperty ;
	rdfs:label "Paper series parent"@en ;
	rdfs:comment "Relates a paper series to its parent paper series. A paper series may have one parent paper series, or none. A paper series may have one or more child paper series, or none. For example: the Treaty Series of in force treaties forms part of the overarching series grouping all treaties."@en ;
	rdfs:domain ppaper:PaperSeries ;
	rdfs:range ppaper:PaperSeries ;
	rdfs:isDefinedBy <http://parliament.uk/ontologies/parliamentary-paper/> .

ppaper:paperSeriesFollows rdf:type owl:ObjectProperty ;
	rdfs:label "Paper series follows"@en ;
	rdfs:comment "Relates a paper series to its predecessor series. A paper series may follow one series, or none."@en ;
	rdfs:domain ppaper:PaperSeries ;
	rdfs:range ppaper:PaperSeries ;
	rdfs:isDefinedBy <http://parliament.uk/ontologies/parliamentary-paper/> .

ppaper:belongsTo rdf:type owl:ObjectProperty ;
	rdfs:label "Belongs to"@en ;
	rdfs:comment "Relates a paper series to the session that series belongs to. A paper series may belong to one session, or none."@en ;
	rdfs:domain ppaper:PaperSeries ;
	rdfs:range ppaper:Session ;
	rdfs:isDefinedBy <http://parliament.uk/ontologies/parliamentary-paper/> .

	
	
#######  Data properties ##### 

ppaper:paperSeriesPrefix rdf:type owl:DatatypeProperty ;
	rdfs:label "Paper series prefix"@en ;
	rdfs:comment "Relates a paper series to the prefix forming part of the 'number' of a parliamentary paper being part of that series."@en ;
	rdfs:domain ppaper:PaperSeries ;
	rdfs:range rdfs:Literal ;
	rdfs:isDefinedBy <http://parliament.uk/ontologies/parliamentary-paper/> .
	
ppaper:confersPrivilege rdf:type owl:DatatypeProperty ;
	rdfs:label "Confers privilege"@en ;
	rdfs:comment "Used to record if membership of a series confers parliamentary privilige."@en ;
	rdfs:domain ppaper:PaperSeries ;
	rdfs:range xsd:boolean ;
	rdfs:isDefinedBy <http://parliament.uk/ontologies/parliamentary-paper/> .


