@prefix pfba: <http://parliament.uk/ontologies/formal-body-affiliation/> . 
@prefix xsd: <http://www.w3.org/2001/XMLSchema#> . 
@prefix rdf: <http://www.w3.org/1999/02/22-rdf-syntax-ns#> .
@prefix dcterms: <http://purl.org/dc/terms/> .
@prefix owl:     <http://www.w3.org/2002/07/owl#> .
@prefix rdfs:    <http://www.w3.org/2000/01/rdf-schema#> .
@prefix foaf:	<http://xmlns.com/foaf/0.1/> .

<http://parliament.uk/ontologies/formal-body-affiliation/> 
    rdf:type owl:Ontology ;
    dcterms:title "Formal body affiliation ontology"@en ;
    dcterms:created "2017-06-22"^^xsd:date ;
	dcterms:rights "Open Parliament Licence v3.0"@en ;
    dcterms:description "A model describing specialisations of group affiliations and positions specific to formal bodies, for example: ex-officio membership of a committee, or chairing of a committee."@en ;
	foaf:depiction <https://ukparliament.github.io/ontologies/formal-body-affiliation/formal-body-affiliation.png> ;
	foaf:maker
		[ foaf:name "James Bowman" ],
		[ foaf:name "Gordon Clarke" ],
		[ foaf:name "Robert Brook"; foaf:homepage <https://robert-brook.com/> ],
		[ foaf:name "Edward McCarthy" ],
		[ foaf:name "Silver Oliver" ],
		[ foaf:name "Michael Smethurst"; foaf:homepage <http://smethur.st/> ],
	    [ foaf:name "Anya Somerville" ].


#######  Classes ##### 	

pfba:FormalBodyMembership rdf:type owl:Class ;
	rdfs:label "Formal body membership"@en ;
	rdfs:comment "Specialises group inclusion to membership of a formal body; membership being taken from the backbenches nominated in a House, subject experts not being Members of a House, or other appointed members."@en ;
	rdfs:isDefinedBy <http://parliament.uk/ontologies/formal-body-affiliation/> .
	
pfba:CooptedMembership rdf:type owl:Class ;
	rdfs:subClassOf pfba:FormalBodyMembership ;
	rdfs:label "Co-opted membership"@en ;
	rdfs:comment "Co-opted membership results from a formal body adding a member at the discretion of existing members. A co-opted member may be a Member of a House: for example, in the House of Lords a peer who is a subject matter expert. Co-opted members may be people who are not Members of a House, referred to as lay members in the House of Commons and external members in the House of Lords: for example, the Executive Committee may co-opt the Director of the Parliamentary Digital Service or Parliamentary Security Director into its membership."@en ;
	rdfs:isDefinedBy <http://parliament.uk/ontologies/formal-body-affiliation/> .
	
pfba:AlternateMembership rdf:type owl:Class ;
	rdfs:subClassOf pfba:FormalBodyMembership ;
	rdfs:label "Alternate membership"@en ;
	rdfs:comment "Alternate members substitute for other members when those members are unable to attend: for example, the Lords Procedure Committee is supplemented by an alternate for each party grouping, an alternate for the Crossbenchers and an alternate for the Convenor. Alternate members receive papers to the formal body, even when not substituting for a member. When substituting for a member, alternate members are entitled to attend meetings and to vote."@en ;
	rdfs:isDefinedBy <http://parliament.uk/ontologies/formal-body-affiliation/> .
	
pfba:ExOfficioMembership rdf:type owl:Class ;
	rdfs:subClassOf pfba:FormalBodyMembership ;
	rdfs:label "Ex-officio membership"@en ;
	rdfs:comment "Ex-officio membership is membership granted by the holding of a position external to the formal body. A frontbencher may hold an ex-officio membership of a committee: for example, Government and Opposition Whips having membership of the Administration Committee; Ministers having membership of the Committee of Public Accounts and the Environmental Audit Committee, though by convention not attending meetings of either committee; or Leaders of the House chairing the Select Committee on Modernisation of the House of Commons between 1997 and 2010."@en ;
	rdfs:isDefinedBy <http://parliament.uk/ontologies/formal-body-affiliation/> .
	
pfba:FormalBodyPosition rdf:type owl:Class ;
	rdfs:label "Formal body position"@en ;
	rdfs:comment "Specialises position to formal bodies."@en ;
	rdfs:isDefinedBy <http://parliament.uk/ontologies/formal-body-affiliation/> .
	
pfba:Chair rdf:type owl:Class ;
	rdfs:subClassOf pfba:FormalBodyPosition ;
	rdfs:label "Chair"@en ;
	rdfs:comment "The position of chair of a formal body. A formal body may have one or more incumbents in the chair position at the same time, or none. "@en ;
	rdfs:isDefinedBy <http://parliament.uk/ontologies/formal-body-affiliation/> .
	
pfba:PrincipalClerk rdf:type owl:Class ;
	rdfs:subClassOf pfba:FormalBodyPosition ;
	rdfs:label "Principal clerk"@en ;
	rdfs:comment "The position of principal clerk of a formal body. A formal body may have one or more incumbents in the position of principal clerk at the same time, or none."@en ;
	rdfs:isDefinedBy <http://parliament.uk/ontologies/formal-body-affiliation/> .
	
pfba:InternalExpert rdf:type owl:Class ;
	rdfs:subClassOf pfba:FormalBodyPosition ;
	rdfs:label "Internal expert"@en ;
	rdfs:comment "A subject matter expert appointed by a formal body. A committee appoints an internal expert as a committee specialist."@en ;
	rdfs:isDefinedBy <http://parliament.uk/ontologies/formal-body-affiliation/> .
	
pfba:ExternalExpert rdf:type owl:Class ;
	rdfs:subClassOf pfba:FormalBodyPosition ;
	rdfs:label "External expert"@en ;
	rdfs:comment "A subject matter expert contracted by a formal body for the duration of an inquiry."@en ;
	rdfs:isDefinedBy <http://parliament.uk/ontologies/formal-body-affiliation/> .