@prefix ppsa: <http://parliament.uk/ontologies/procedure-step-annotation/> . 
@prefix xsd: <http://www.w3.org/2001/XMLSchema#> . 
@prefix rdf: <http://www.w3.org/1999/02/22-rdf-syntax-ns#> .
@prefix dcterms: <http://purl.org/dc/terms/> .
@prefix owl:     <http://www.w3.org/2002/07/owl#> .
@prefix rdfs:    <http://www.w3.org/2000/01/rdf-schema#> .
@prefix foaf:	<http://xmlns.com/foaf/0.1/> .

<http://parliament.uk/ontologies/procedure-step-annotation/> 
    rdf:type owl:Ontology ;
    dcterms:title "Procedure step ontology"@en ;
    dcterms:created "2019-04-16"^^xsd:date ;
	dcterms:rights "Open Parliament Licence v3.0"@en ;
    dcterms:description "A model describing annotations added to procedure steps by the Indexing and Data Management Section of the House of Commons Library. Annotations are used to describe how a procedure step is actualised."@en ;
	foaf:depiction <https://ukparliament.github.io/ontologies/procedure-step-annotation/procedure-step-annotation.png> ;
	foaf:maker
		[ foaf:name "Robert Brook"; foaf:homepage <https://robert-brook.com/> ],
		[ foaf:name "Michael Smethurst"; foaf:homepage <http://smethur.st/> ],
	    [ foaf:name "Anya Somerville" ] .


#######  Classes ##### 	

ppsa:Step rdf:type owl:Class ;
	rdfs:label "Step"@en ;
	rdfs:comment "A step is either a business step, a logic gate step or a decision step. Steps are joined by routes to form procedures. For example, within the SI procedures there exists a step named 'English Votes for English Laws (EVEL) consideration'. Steps may occur in more than one procedure. For example, all statutory instrument procedures include the EVEL consideration step."@en ;
	rdfs:isDefinedBy <http://parliament.uk/ontologies/procedure-step-annotation/> .
	
ppsa:Publication rdf:type owl:Class ;
	rdfs:label "Publication"@en ;
	rdfs:comment "A publication."@en ;
	rdfs:isDefinedBy <http://parliament.uk/ontologies/procedure-step-annotation/> .
	

	

	
##### Object properties ####


ppsa:actualiseWith rdf:type owl:ObjectProperty ;
	rdfs:label "Actualise with"@en ;
	rdfs:comment "Relates a step to a step where steps may be actualised together."@en ;
	rdfs:domain ppsa:Step ;
	rdfs:range ppsa:Step ;
	rdfs:isDefinedBy <http://parliament.uk/ontologies/procedure-step-annotation/> .

ppsa:source rdf:type owl:ObjectProperty ;
	rdfs:label "Source"@en ;
	rdfs:comment "Relates a step to the publication which is the source of information for that step."@en ;
	rdfs:domain ppsa:Step ;
	rdfs:range ppsa:Publication ;
	rdfs:isDefinedBy <http://parliament.uk/ontologies/procedure-step-annotation/> .
	

				
	
##### Data properties ####	
	
ppsa:linkNote rdf:type owl:DatatypeProperty ;
	rdfs:label "Link note"@en ;
	rdfs:comment "A note that describes where a business item, actualising a step, should link to in a publication."@en ;
	rdfs:domain ppsa:Step ;
	rdfs:range rdf:langString ;
	rdfs:isDefinedBy <http://parliament.uk/ontologies/procedure-step-annotation/> .
	
ppsa:dateNote rdf:type owl:DatatypeProperty ;
	rdfs:label "Date note"@en ;
	rdfs:comment "A note that describes the date to use when actualising a step."@en ;
	rdfs:domain ppsa:Step ;
	rdfs:range rdf:langString ;
	rdfs:isDefinedBy <http://parliament.uk/ontologies/procedure-step-annotation/> .
						