@prefix plg: <http://parliament.uk/ontologies/legislation/> . 
@prefix xsd: <http://www.w3.org/2001/XMLSchema#> . 
@prefix rdf: <http://www.w3.org/1999/02/22-rdf-syntax-ns#> .
@prefix dcterms: <http://purl.org/dc/terms/> .
@prefix owl:     <http://www.w3.org/2002/07/owl#> .
@prefix rdfs:    <http://www.w3.org/2000/01/rdf-schema#> .
@prefix foaf:	<http://xmlns.com/foaf/0.1/> .

<http://parliament.uk/ontologies/legislation/> 
    rdf:type owl:Ontology ;
    dcterms:title "Legislation ontology"@en ;
    dcterms:created "2018-03-21"^^xsd:date ;
	dcterms:rights "Open Parliament Licence v3.0"@en ;
    dcterms:description "A model describing the forms of draft and made legislation considered by Parliament, powers delegated by primary legislation and accompanying duties toward Parliament."@en ;
	foaf:depiction <https://ukparliament.github.io/ontologies/legislation/legislation.png> ;
	foaf:maker
		[ foaf:name "David Beamish" ],
		[ foaf:name "Robert Brook"; foaf:homepage <https://robert-brook.com/> ],
		[ foaf:name "Nerys Davies" ],
		[ foaf:name "Jack Dent" ],
		[ foaf:name "Samu Lang" ],
		[ foaf:name "Lucinda Maer" ],
		[ foaf:name "Silver Oliver" ],
		[ foaf:name "John Sheridan" ],
		[ foaf:name "Michael Smethurst"; foaf:homepage <http://smethur.st/> ],
	    [ foaf:name "Anya Somerville" ],
	    [ foaf:name "Jayne Sunley" ],
	    [ foaf:name "Matthew Waddington" ],
		[ foaf:name "Jane White" ].


#######  Classes #####

plg:EnablingThing rdf:type owl:Class ;
	rdfs:label "Enabling thing"@en ;
	rdfs:comment "A thing that enables the exercise of a power."@en ;
	rdfs:isDefinedBy <http://parliament.uk/ontologies/legislation/> .
	
plg:ActOfParliament rdf:type owl:Class ;
	rdfs:subClassOf plg:EnablingThing ;
	rdfs:label "Act of Parliament"@en ;
	rdfs:comment "An Act of Parliament creates, amends or repeals legislation. An Act is a Bill having been passed by Parliament and been given Royal Assent. Acts of Parliament which are in force comprise statute law also known as the statute book."@en ;
	rdfs:isDefinedBy <http://parliament.uk/ontologies/legislation/> .

plg:EnablingPower rdf:type owl:Class ;
	rdfs:label "Enabling power"@en ;
	rdfs:comment "A power delegated by one or more items of primary legislation, enabling the exercise of regulations as described in the Act."@en ;
	rdfs:isDefinedBy <http://parliament.uk/ontologies/legislation/> .
	
plg:EnabledThing rdf:type owl:Class ;
	rdfs:label "Enabled thing"@en ;
	rdfs:comment "A thing which is intended to exercise a power set out in statute."@en ;
	rdfs:isDefinedBy <http://parliament.uk/ontologies/legislation/> .

plg:PublishedDraftUnderEUWA rdf:type owl:Class ;
	rdfs:subClassOf plg:EnabledThing ;
	rdfs:label "Published draft under the European Union (Withdrawal) Act 2018"@en ;
	rdfs:comment "A draft published under the duties laid out in paragraph 14 of schedule 8 of the European Union (Withdrawal) Act 2018. A Minister has a duty to publish such a draft 28 joint sitting days before the laying of any instrument which intends to amend or revoke subordinate legislation under section 2(2) of the European Communities Act 1972, including subordinate legislation implementing EU directives."@en ;
	rdfs:isDefinedBy <http://parliament.uk/ontologies/legislation/> .

plg:ProposedNegativeStatutoryInstrument rdf:type owl:Class ;
	rdfs:subClassOf plg:EnabledThing ;
	rdfs:label "Proposed negative statutory instrument"@en ;
	rdfs:comment "A regulation - made under a power or powers set out in clauses 7, 8 or 9 of the European Union (Withdrawal) Act 2018 - which government ministers propose be laid under the negative procedure. Sifting committees of either House may recommend that any subsequent statutory instrument or instruments be laid under the affirmative procedure."@en ;
	rdfs:isDefinedBy <http://parliament.uk/ontologies/legislation/> .

plg:DraftAndMadeStatutoryInstrumentSubjectToParliamentaryProcedure rdf:type owl:Class ;
	rdfs:subClassOf plg:EnabledThing ;
	rdfs:label "Draft and made statutory instrument subject to parliamentary procedure"@en ;
	rdfs:comment "The National Archives classify made instruments as legislation and draft instruments as draft legislation. Parliament considers both made and draft instruments as part of the legislative process, distinct from a FRBR work as used by The National Archives. Parliament includes draft instruments in its description of statutory instruments which are modelled here together."@en ;
	rdfs:isDefinedBy <http://parliament.uk/ontologies/legislation/> .

plg:DraftStatutoryInstrument rdf:type owl:Class ;
	rdfs:label "Draft statutory instrument"@en ;
	rdfs:comment "Draft statutory instruments are laid before Parliament, and may be objected to. A draft instrument is made into secondary legislation when signed by a government minister. Draft statutory instruments are published by The National Archives and classified by them as a FRBR work."@en ;
	rdfs:isDefinedBy <http://parliament.uk/ontologies/legislation/> .

plg:MadeStatutoryInstrument rdf:type owl:Class ;
	rdfs:label "Made statutory instrument"@en ;
	rdfs:comment "Made statutory instruments may progress from draft, or be laid without draft before Parliament as made. Parliament may consider particular instruments as made with imposing a duty to lay. For example: commencement orders. Made statutory instruments may be objected to within Parliament. A made instrument has been signed into secondary legislation by a government minister. Made statutory instruments are published by The National Archives and classified by them as a FRBR work."@en ;
	rdfs:isDefinedBy <http://parliament.uk/ontologies/legislation/> .
	
plg:StatutoryInstrumentSeriesItem rdf:type owl:Class ;
	rdfs:label "Statutory instrument series item"@en ;
	rdfs:comment "A statutory instrument series item links a draft or made statutory instrument subject to parliamentary procedure to a statutory instrument series. A statutory instrument can be included by means of an item in more than one series excepting these cases: Northern Ireland series instruments do not form part of any other series; legal series instruments do not form part of any other series; National Assembly for Wales series SIs and Scottish series instruments can be included in the commencement order series but no other. Commencement order series items may also form part of either the Welsh or Scottish series. Where an instrument appears as an item in more than one series, the citation order is formed by (1) the commencement order series and item identifier followed by (2) any other series and item identifier. Where the instrument is made by the Welsh Ministers, the 'W. / Cy.' number follows the SI number."@en ;
	rdfs:isDefinedBy <http://parliament.uk/ontologies/legislation/> .
	
plg:StatutoryInstrumentSeries rdf:type owl:Class ;
	rdfs:label "Statutory instrument series"@en ;
	rdfs:comment "A statutory instrument may appear in one or more series, or in none. Series include: Welsh Instruments, corresponding to Wales Statutory Instruments; Northern Ireland Orders in Council; Commencement Orders; Appointed Day Orders; Legal Statutory Instruments; and Scottish Statutory Instruments, being United Kingdom instruments that have particular application to Scotland."@en ;
	rdfs:isDefinedBy <http://parliament.uk/ontologies/legislation/> .
	
plg:Duty rdf:type owl:Class ;
	rdfs:label "Duty"@en ;
	rdfs:comment "An obligation that must be discharged in relation to the exercise of an enabling power."@en ;
	rdfs:isDefinedBy <http://parliament.uk/ontologies/legislation/> .
	
	

##### Object properties ####

plg:confers rdf:type owl:ObjectProperty ;
	rdfs:label "Confers"@en ;
	rdfs:comment "Relates an enabling thing to an enabling power. An enabling thing may confer more than one enabling power. Secondary legislation may confer powers to enable further legislation, being sub-delegation into tertiary law. Such law may be made without statutory instrument and is not itself subject to parliamentary procedure."@en ;
	rdfs:domain plg:EnablingThing ;
	rdfs:range plg:EnablingPower ;
	rdfs:isDefinedBy <http://parliament.uk/ontologies/legislation/> .
	
plg:imposes rdf:type owl:ObjectProperty ;
	rdfs:label "Imposes"@en ;
	rdfs:comment "Relates an enabling thing to a duty imposed in the exercise of an associated enabling power."@en ;
	rdfs:domain plg:EnablingPower ;
	rdfs:range plg:Duty ;
	rdfs:isDefinedBy <http://parliament.uk/ontologies/legislation/> .
	
plg:exercises rdf:type owl:ObjectProperty ;
	rdfs:label "Exercises"@en ;
	rdfs:comment "Relates an enabled thing to an enabling power. An enabled thing is enabled by one or more enabling powers and an enabling power may enable more than one enabled thing."@en ;
	rdfs:domain plg:EnabledThing ;
	rdfs:range plg:EnablingPower ;
	rdfs:isDefinedBy <http://parliament.uk/ontologies/legislation/> .

plg:requires rdf:type owl:ObjectProperty ;
	rdfs:label "Requires"@en ;
	rdfs:comment "Relates an enabling power to a duty. The exercise of an enabling power may require one or more duties, or none. A duty may be associated with the exercise of one or more enabling powers."@en ;
	rdfs:domain plg:EnablingPower ;
	rdfs:range plg:Duty ;
	rdfs:isDefinedBy <http://parliament.uk/ontologies/legislation/> .

plg:enabledBy rdf:type owl:ObjectProperty ;
	rdfs:label "Enabled by"@en ;
	rdfs:comment "Relates an enabled thing to the thing which enables it. An enabled thing may be enabled by one or more enabling things. An enabling thing may enable one or more enabled things, or none."@en ;
	rdfs:domain plg:EnabledThing ;
	rdfs:range plg:EnablingThing ;
	rdfs:isDefinedBy <http://parliament.uk/ontologies/legislation/> .
	
plg:precededBy rdf:type owl:ObjectProperty ;
	rdfs:label "Preceded by"@en ;
	rdfs:comment "Relates an enabled thing to the enabled thing which preceded it. An enabled thing may be preceded by one or more enabled things, or by none. An enabled thing may precede one or more enabled things, or none."@en ;
	rdfs:domain plg:EnabledThing ;
	rdfs:range plg:EnabledThing ;
	rdfs:isDefinedBy <http://parliament.uk/ontologies/legislation/> .
	
plg:embodiedAsDraftStatutoryInstrument rdf:type owl:ObjectProperty ;
	rdfs:label "Embodied as draft statutory instrument"@en ;
	rdfs:comment "Relates a draft or made statutory instrument subject to parliamentary procedure to draft legislation published by The National Archives and identified by them as a FRBR work. A draft or made statutory instrument subject to parliamentary procedure is embodied as a single draft statutory instrument, or none. A draft statutory instrument is related to one draft or made statutory instrument subject to parliamentary procedure, or to none."@en ;
	rdfs:domain plg:DraftAndMadeStatutoryInstrumentSubjectToParliamentaryProcedure ;
	rdfs:range plg:DraftStatutoryInstrument ;
	rdfs:isDefinedBy <http://parliament.uk/ontologies/legislation/> .
	
plg:embodiedAsMadeStatutoryInstrument rdf:type owl:ObjectProperty ;
	rdfs:label "Embodied as made statutory instrument"@en ;
	rdfs:comment "Relates a draft or made statutory instrument subject to parliamentary procedure to made legislation published by The National Archives and identified by them as a FRBR work. A draft or made statutory instrument subject to parliamentary procedure will be embodied as a single made statutory instrument, or none. A made statutory instrument is related to one draft or made statutory instrument subject to parliamentary procedure, or to none."@en ;
	rdfs:domain plg:DraftAndMadeStatutoryInstrumentSubjectToParliamentaryProcedure ;
	rdfs:range plg:MadeStatutoryInstrument ;
	rdfs:isDefinedBy <http://parliament.uk/ontologies/legislation/> .
	
plg:asSeriesItem rdf:type owl:ObjectProperty ;
	rdfs:label "As series item"@en ;
	rdfs:comment "Relates a made statutory instrument to a statutory instrument series item. A made statutory instrument may belong to more than one series by means of a series item. A series item is formed of a single made statutory instrument."@en ;
	rdfs:domain plg:MadeStatutoryInstrument ;
	rdfs:range plg:StatutoryInstrumentSeriesItem ;
	rdfs:isDefinedBy <http://parliament.uk/ontologies/legislation/> .
	
plg:inSeries rdf:type owl:ObjectProperty ;
	rdfs:label "In series"@en ;
	rdfs:comment "Relates a statutory instrument series item to a statutory instrument series. A series may have one or more items, or none. A series item places an instrument in a single series."@en ;
	rdfs:domain plg:StatutoryInstrumentSeriesItem ;
	rdfs:range plg:StatutoryInstrumentSeries ;
	rdfs:isDefinedBy <http://parliament.uk/ontologies/legislation/> .
	
					
	
##### Data properties ####	

plg:siPrefix rdf:type owl:DatatypeProperty ;
	rdfs:label "SI prefix"@en ;
	rdfs:comment "The prefix part of a statutory instrument number, for example, 'SI' in 'SI 1986/925'."@en ;
	rdfs:domain plg:MadeStatutoryInstrument ;
	rdfs:range rdfs:Literal ;
	rdfs:isDefinedBy <http://parliament.uk/ontologies/legislation/> .
	
plg:siYear rdf:type owl:DatatypeProperty ;
	rdfs:label "SI year"@en ;
	rdfs:comment "The year part of a statutory instrument number, for example, '1986' in 'SI 1986/925'. The SI year is the year the instrument was laid before Parliament, except when laid in draft in one calendar year, made in a following year and having its SI year updated."@en ;
	rdfs:domain plg:MadeStatutoryInstrument ;
	rdfs:range rdfs:Literal ;
	rdfs:isDefinedBy <http://parliament.uk/ontologies/legislation/> .
	
plg:siIdentiferInYear rdf:type owl:DatatypeProperty ;
	rdfs:label "SI identifer in year"@en ;
	rdfs:comment "The identifier in year part of a statutory instrument number, for example, '925' in 'SI 1986/925'."@en ;
	rdfs:domain plg:MadeStatutoryInstrument ;
	rdfs:range rdfs:Literal ;
	rdfs:isDefinedBy <http://parliament.uk/ontologies/legislation/> .
	
plg:madeDate rdf:type owl:DatatypeProperty ;
	rdfs:label "Made date"@en ;
	rdfs:comment "The date on which a statutory instrument is made by a government minister."@en ;
	rdfs:domain plg:MadeStatutoryInstrument ;
	rdfs:range xsd:date ;
	rdfs:isDefinedBy <http://parliament.uk/ontologies/legislation/> .
	
plg:comingIntoForceDate rdf:type owl:DatatypeProperty ;
	rdfs:label "Coming into force date"@en ;
	rdfs:comment "The date on which a statutory instrument comes into force. Schedules within an instrument may come into force on different dates. Coming into force details would be given in a coming into force note where no single coming into force date is given."@en ;
	rdfs:domain plg:DraftAndMadeStatutoryInstrumentSubjectToParliamentaryProcedure ;
	rdfs:range xsd:date ;
	rdfs:isDefinedBy <http://parliament.uk/ontologies/legislation/> .
	
plg:comingIntoForceNote rdf:type owl:DatatypeProperty ;
	rdfs:label "Coming into force note"@en ;
	rdfs:comment "A coming into force note sets out details of the commencement of provisions or effects forming part or parts of an instrument, or the instrument as a whole."@en ;
	rdfs:domain plg:DraftAndMadeStatutoryInstrumentSubjectToParliamentaryProcedure ;
	rdfs:range rdf:langString ;
	rdfs:isDefinedBy <http://parliament.uk/ontologies/legislation/> .

plg:isbn rdf:type owl:DatatypeProperty ;
	rdfs:label "ISBN"@en ;
	rdfs:comment "An identifier conforming to the ISBN standard."@en ;
	rdfs:domain plg:DraftAndMadeStatutoryInstrumentSubjectToParliamentaryProcedure ;
	rdfs:range rdfs:Literal ;
	rdfs:isDefinedBy <http://parliament.uk/ontologies/legislation/> .
	
plg:siSeriesItemIdentifier rdf:type owl:DatatypeProperty ;
	rdfs:label "SI series item identifier"@en ;
	rdfs:comment "The identifier of an item within a series, for example, '121' in ' SI 2018/647 (W. 121)'."@en ;
	rdfs:domain plg:StatutoryInstrumentSeriesItem ;
	rdfs:range rdfs:Literal ;
	rdfs:isDefinedBy <http://parliament.uk/ontologies/legislation/> .

plg:chapterNumber rdf:type owl:DatatypeProperty ;
	rdfs:label "Chapter number"@en ;
	rdfs:comment "The identifier in year part of an Act of Parliament number, for example, '12' in '1986 c. 12'."@en ;
	rdfs:domain plg:ActOfParliament ;
	rdfs:range rdfs:Literal ;
	rdfs:isDefinedBy <http://parliament.uk/ontologies/legislation/> .

plg:actYear rdf:type owl:DatatypeProperty ;
	rdfs:label "Act year"@en ;
	rdfs:comment "The year part of an Act of Parliament number, for example, '1986' in '1986 c. 12'. The Act year is the year in which Royal Assent was given."@en ;
	rdfs:domain plg:ActOfParliament ;
	rdfs:range rdfs:Literal ;
	rdfs:isDefinedBy <http://parliament.uk/ontologies/legislation/> .

plg:royalAssentOn rdf:type owl:DatatypeProperty ;
	rdfs:label "Royal Assent on"@en ;
	rdfs:comment "The date on which Royal Assent was given, as recorded by legislation.gov.uk. This may differ from the date recorded by Parliament if Royal Assent is given after midnight on a sitting day."@en ;
	rdfs:domain plg:ActOfParliament ;
	rdfs:range xsd:date ;
	rdfs:isDefinedBy <http://parliament.uk/ontologies/legislation/> .