@prefix phme: <http://parliament.uk/ontologies/house-membership-enabling/> . 
@prefix xsd: <http://www.w3.org/2001/XMLSchema#> . 
@prefix rdf: <http://www.w3.org/1999/02/22-rdf-syntax-ns#> .
@prefix dcterms: <http://purl.org/dc/terms/> .
@prefix owl:     <http://www.w3.org/2002/07/owl#> .
@prefix rdfs:    <http://www.w3.org/2000/01/rdf-schema#> .
@prefix foaf:	<http://xmlns.com/foaf/0.1/> .

<http://parliament.uk/ontologies/house-membership/> 
    rdf:type owl:Ontology ;
    dcterms:title "House membership enabling ontology"@en ;
    dcterms:created "2022-05-18"^^xsd:date ;
	dcterms:rights "Open Parliament Licence v3.0"@en ;
    dcterms:description "A model attaching House seats and seat incumbencies to the things they are enabled by."@en ;
	foaf:depiction <https://ukparliament.github.io/ontologies/house-membership-enabling/house-membership-enabling.svg> ;
	foaf:maker
		[ foaf:name "Robert Brook"; foaf:homepage <https://robert-brook.com/> ],
		[ foaf:name "Michael Smethurst"; foaf:homepage <http://smethur.st/> ] .


#######  Classes ##### 	

phme:HouseSeat rdf:type owl:Class ;
	rdfs:label "House seat"@en ;
	rdfs:comment "A seat as a position in a House - rather than a physical seat or constituency - which may be allocated to a Member, for example: a seat in the House of Commons associated with a constituency - or a seat in the House of Lords allocated to the Archbishop of Canterbury, inherited by a hereditary peer or granted to a life peer."@en ;
	rdfs:isDefinedBy <http://parliament.uk/ontologies/house-membership-enabling/> .
	
phme:HouseSeatEnablingThing rdf:type owl:Class ;
	rdfs:label "House seat enabling thing"@en ;
	rdfs:comment ""@en ;
	rdfs:isDefinedBy <http://parliament.uk/ontologies/house-membership-enabling/> .
	
phme:SeatIncumbency rdf:type owl:Class ;
	rdfs:label "Seat incumbency"@en ;
	rdfs:comment "The occupation of a seat in a House by a person, for a period of time.  A person may have more than one incumbency over time. Only one person can be incumbent in a house seat at one time. A person having a seat incumbency which has a start date in the past and an end date in the future - or which has no end date - is a current Member. A person having a seat incumbency with an end date in the past - and no current incumbency - is an ex-Member."@en ;
	rdfs:isDefinedBy <http://parliament.uk/ontologies/house-membership-enabling/> .
	
phme:SeatIncumbencyEnablingThing rdf:type owl:Class ;
	rdfs:label "Seat incumbency enabling thing"@en ;
	rdfs:comment ""@en ;
	rdfs:isDefinedBy <http://parliament.uk/ontologies/house-membership-enabling/> .


	
##### Object properties ####

phme:houseSeatEnabledBy rdf:type owl:ObjectProperty ;
	rdfs:label "House seat enabled by"@en ;
	rdfs:comment "Relates a House seat to the thing which enables the existence of that seat."@en ;
	rdfs:domain phm:HouseSeat ;
	rdfs:range phm:HouseSeatEnablingThing ;
	rdfs:isDefinedBy <http://parliament.uk/ontologies/house-membership-enabling/> .
	
phme:seatIncumbencyEnabledBy rdf:type owl:ObjectProperty ;
	rdfs:label "Seat incumbency enabled by"@en ;
	rdfs:comment "Relates a seat incumbency to the thing which enables the existence of that incumbency."@en ;
	rdfs:domain phm:SeatIncumbency ;
	rdfs:range phm:SeatIncumbencyEnablingThing ;
	rdfs:isDefinedBy <http://parliament.uk/ontologies/house-membership-enabling/> .