@prefix pl: <http://parliament.uk/ontologies/laying/> . 
@prefix xsd: <http://www.w3.org/2001/XMLSchema#> . 
@prefix rdf: <http://www.w3.org/1999/02/22-rdf-syntax-ns#> .
@prefix dcterms: <http://purl.org/dc/terms/> .
@prefix owl:     <http://www.w3.org/2002/07/owl#> .
@prefix rdfs:    <http://www.w3.org/2000/01/rdf-schema#> .
@prefix foaf:	<http://xmlns.com/foaf/0.1/> .

<http://parliament.uk/ontologies/laying/> 
    rdf:type owl:Ontology ;
    dcterms:title "Laying ontology"@en ;
    dcterms:created "2018-02-06"^^xsd:date ;
	dcterms:rights "Open Parliament Licence v3.0"@en ;
    dcterms:description "A model describing the laying of papers before a House and the authority a paper is laid under."@en;
	foaf:depiction <https://ukparliament.github.io/ontologies/laying/laying.svg> ;
	foaf:maker 
		[ foaf:name "Jayne Bosworth" ],
		[ foaf:name "Robert Brook"; foaf:homepage <https://robert-brook.com/> ],
		[ foaf:name "Jack Dent" ],
		[ foaf:name "Mike Hennessy" ],
		[ foaf:name "Matt Korris" ],
		[ foaf:name "Stephen McGinness" ],
		[ foaf:name "Ned Morrell" ],
		[ foaf:name "Michael Smethurst"; foaf:homepage <http://smethur.st/> ],
		[ foaf:name "Anya Somerville" ].


#######  Classes #####
	
pl:MakingAvailable rdf:type owl:Class ;
	rdfs:label "Making available"@en ;
	rdfs:comment "The act of making a thing available to a House or to a House by means of its Library."@en ;
	rdfs:isDefinedBy <http://parliament.uk/ontologies/laying/> .
	
pl:Laying rdf:type owl:Class ;
	rdfs:subClassOf pl:MakingAvailable ;
	rdfs:label "Laying"@en ;
	rdfs:comment "The act of making available a paper into a House. Papers may be laid before both Houses on the same day."@en ;
	rdfs:isDefinedBy <http://parliament.uk/ontologies/laying/> .

pl:LayingAuthority rdf:type owl:Class ;
	rdfs:label "Laying authority"@en ;
	rdfs:comment ""@en ;
	rdfs:isDefinedBy <http://parliament.uk/ontologies/laying/> .

pl:LayingAuthorityType rdf:type owl:Class ;
	rdfs:label "Laying authority type"@en ;
	rdfs:comment "The type of an authority under which a paper is laid before a House. Legislation may impose a duty on a body to lay papers before a House, these are laid 'by Act'. Command papers are laid in a House by the government and are laid 'by Command'."@en ;
	rdfs:isDefinedBy <http://parliament.uk/ontologies/laying/> .
	
pl:LaidPaper rdf:type owl:Class ;
	rdfs:subClassOf pl:ParliamentaryPaper ;
	rdfs:subClassOf pl:MadeAvailableThing ;
	rdfs:label "Laid paper"@en ;
	rdfs:comment "A paper having been laid before a House."@en ;
	rdfs:isDefinedBy <http://parliament.uk/ontologies/laying/> .
	
pl:ParliamentaryPaper rdf:type owl:Class ;
	rdfs:label "Parliamentary paper"@en ;
	rdfs:comment "Papers laid into or published under the authority of Parliament."@en ;
	rdfs:isDefinedBy <http://parliament.uk/ontologies/laying/> .

pl:MadeAvailableThing rdf:type owl:Class ;
	rdfs:label "Made available thing"@en ;
	rdfs:comment "A thing made available to a House or to a House by means of its Library."@en ;
	rdfs:isDefinedBy <http://parliament.uk/ontologies/laying/> .
	
	

#######  Object properties ##### 
	
pl:hasLayingAuthority rdf:type owl:ObjectProperty ;
	rdfs:label "Has laying authority"@en ;
	rdfs:comment "Relates an act of laying a paper to a laying authority."@en ;
	rdfs:domain pl:Laying ;
	rdfs:range pl:LayingAuthority ;
	rdfs:isDefinedBy <http://parliament.uk/ontologies/laying/> .
	
pl:hasLayingAuthorityType rdf:type owl:ObjectProperty ;
	rdfs:label "Has laying authority type"@en ;
	rdfs:comment "Relates a laying authority to its type."@en ;
	rdfs:domain pl:LayingAuthority ;
	rdfs:range pl:LayingAuthorityType ;
	rdfs:isDefinedBy <http://parliament.uk/ontologies/laying/> .
	
pl:parentLayingAuthorityType rdf:type owl:ObjectProperty ;
	rdfs:label "Parent laying authority type"@en ;
	rdfs:comment "Relates a laying authority type to its parent."@en ;
	rdfs:domain pl:LayingAuthorityType ;
	rdfs:range pl:LayingAuthorityType ;
	rdfs:isDefinedBy <http://parliament.uk/ontologies/laying/> .
	
pl:lays rdf:type owl:ObjectProperty ;
	rdfs:label "Lays"@en ;
	rdfs:comment "Relates an act of laying a paper to the paper having been laid."@en ;
	rdfs:domain pl:Laying ;
	rdfs:range pl:LaidPaper ;
	rdfs:isDefinedBy <http://parliament.uk/ontologies/laying/> .
				

#######  Data properties ##### 

pl:isAuditorCertified rdf:type owl:DatatypeProperty ;
	rdfs:label "Is auditor certified"@en ;
	rdfs:comment "Used to record whether a laid paper has been certified by an auditor."@en ;
	rdfs:domain pl:LaidPaper ;
	rdfs:range xsd:boolean ;
	rdfs:isDefinedBy <http://parliament.uk/ontologies/laying/> .