@prefix putil: <http://parliament.uk/ontologies/utility/> . 
@prefix xsd: <http://www.w3.org/2001/XMLSchema#> . 
@prefix rdf: <http://www.w3.org/1999/02/22-rdf-syntax-ns#> .
@prefix dcterms: <http://purl.org/dc/terms/> .
@prefix owl:     <http://www.w3.org/2002/07/owl#> .
@prefix rdfs:    <http://www.w3.org/2000/01/rdf-schema#> .
@prefix foaf:	<http://xmlns.com/foaf/0.1/> .

<http://parliament.uk/ontologies/utility/> 
    rdf:type owl:Ontology ;
    dcterms:title "Utility ontology"@en ;
    dcterms:created "2016-10-05"^^xsd:date ;
	dcterms:rights "Open Parliament Licence v3.0"@en ;
    dcterms:description "Provides a set of common properties for reuse by other models."@en ;
	foaf:depiction <https://ukparliament.github.io/ontologies/utility/utility.svg> ;
	foaf:maker
		[ foaf:name "Robert Brook"; foaf:homepage <https://robert-brook.com/> ],
		[ foaf:name "Silver Oliver" ],
		[ foaf:name "Michael Smethurst"; foaf:homepage <http://smethur.st/> ],
	    [ foaf:name "Anya Somerville" ].


#######  Classes ##### 	


putil:Thing rdf:type owl:Class ;
	rdfs:label "Thing"@en ;
	rdfs:comment "A thing. Anything. At all. Provides a set of properties for reuse by any other model."@en ;
	rdfs:isDefinedBy <http://parliament.uk/ontologies/utility/> .
	
putil:TemporalThing rdf:type owl:Class ;
	rdfs:subClassOf putil:Thing ;
	rdfs:label "Temporal thing"@en ;
	rdfs:comment "An interval between two points in time, having a name."@en ;
	rdfs:isDefinedBy <http://parliament.uk/ontologies/utility/> .

putil:Identifier rdf:type owl:Class ;
	rdfs:label "Identifier"@en ;
	rdfs:comment "An identifier from an external system. Might be another Parliament system or an external system such as Wikidata."@en ;
	rdfs:isDefinedBy <http://parliament.uk/ontologies/utility/> .
	
putil:IdentifierSource rdf:type owl:Class ;
	rdfs:label "Identifier source"@en ;
	rdfs:comment "An identifier source. The system or website from which the identifier originates."@en ;
	rdfs:isDefinedBy <http://parliament.uk/ontologies/utility/> .

putil:WebLink rdf:type owl:Class ;
	rdfs:label "Web link"@en ;
	rdfs:comment "A web link with a source, type and URL."@en ;
	rdfs:isDefinedBy <http://parliament.uk/ontologies/utility/> .			
	
putil:WebLinkSource rdf:type owl:Class ;
	rdfs:label "Web link source"@en ;
	rdfs:comment "The publisher of the URL identified by the web link e.g. The Daily Mail, personal website, Facebook, Wikipedia."@en ;
	rdfs:isDefinedBy <http://parliament.uk/ontologies/utility/> .	
	
putil:WebLinkType rdf:type owl:Class ;
	rdfs:label "Web link type"@en ;
	rdfs:comment "A link type e.g. personal homepage, obituary."@en ;
	rdfs:isDefinedBy <http://parliament.uk/ontologies/utility/> .
	
putil:Label rdf:type owl:Class ;
	rdfs:label "Label"@en ;
	rdfs:comment "Allows a thing to have different labels at different time periods. e.g. a Government Department, Select Committee, Bill or inquiry might change its name during its lifetime. Reuses preferredLabel, abbreviationLabel, sortLabel, startDate and endDate from Thing."@en ;
	rdfs:isDefinedBy <http://parliament.uk/ontologies/utility/> .	

#######  Object properties ##### 

putil:hasIdentifier rdf:type owl:ObjectProperty ;
	rdfs:label "Has identifier"@en ;
	rdfs:comment "Relates a thing to an identifier."@en ;
	rdfs:domain putil:Thing ;
	rdfs:range putil:Identifier ;
	rdfs:isDefinedBy <http://parliament.uk/ontologies/utility/> .

putil:hasIdentifierSource rdf:type owl:ObjectProperty ;
	rdfs:label "Has identifier source"@en ;
	rdfs:comment "Relates an identifier to its source."@en ;
	rdfs:domain putil:Identifier ;
	rdfs:range putil:IdentifierSource ;
	rdfs:isDefinedBy <http://parliament.uk/ontologies/utility/> .
	
putil:hasWebLink rdf:type owl:ObjectProperty ;
	rdfs:label "Has web link"@en ;
	rdfs:comment "Relates a thing to a web link. e.g. Person to a twitter account."@en ;
	rdfs:domain putil:Thing ;
	rdfs:range putil:WebLink ;
	rdfs:isDefinedBy <http://parliament.uk/ontologies/utility/> .
	
putil:hasWebLinkSource rdf:type owl:ObjectProperty ;
	rdfs:label "Has web link source"@en ;
	rdfs:comment "Relates a web link to a link source."@en ;
	rdfs:domain putil:WebLink ;
	rdfs:range putil:WebLinkSource ;
	rdfs:isDefinedBy <http://parliament.uk/ontologies/utility/> .	
	
putil:hasWebLinkType rdf:type owl:ObjectProperty ;
	rdfs:label "Has web link type"@en ;
	rdfs:comment "Relates a link to a weblink type."@en ;
	rdfs:domain putil:WebLink ;
	rdfs:range putil:WebLinkType ;
	rdfs:isDefinedBy <http://parliament.uk/ontologies/utility/> .		
	
putil:hasLabel rdf:type owl:ObjectProperty ;
	rdfs:label "Has label"@en ;
	rdfs:comment "Relates a thing to a label during a time period."@en ;
	rdfs:domain putil:Thing ;
	rdfs:range putil:Label ;
	rdfs:isDefinedBy <http://parliament.uk/ontologies/utility/> .		
	
putil:precededBy rdf:type owl:ObjectProperty ;
	rdfs:label "Preceded by"@en ;
	rdfs:comment "Relates a thing to its predecessor. Usually the thing and its preceding thing will be of the same class."@en ;
	rdfs:domain putil:Thing ;
	rdfs:range putil:Thing ;
	rdfs:isDefinedBy <http://parliament.uk/ontologies/utility/> .				
		

#######  Data properties #####

