@prefix pso: <http://parliament.uk/ontologies/standing-order/> . 
@prefix xsd: <http://www.w3.org/2001/XMLSchema#> . 
@prefix rdf: <http://www.w3.org/1999/02/22-rdf-syntax-ns#> .
@prefix dcterms: <http://purl.org/dc/terms/> .
@prefix owl:     <http://www.w3.org/2002/07/owl#> .
@prefix rdfs:    <http://www.w3.org/2000/01/rdf-schema#> .
@prefix foaf:	<http://xmlns.com/foaf/0.1/> .

<http://parliament.uk/ontologies/standing-order/> 
    rdf:type owl:Ontology ;
    dcterms:title "Standing Order ontology"@en ;
    dcterms:created "2020-12-07"^^xsd:date ;
	dcterms:rights "Open Parliament Licence v3.0"@en ;
    dcterms:description "A model describing Standing Orders for both Houses of Parliament, establishing persistent identification of orders and fragments of orders."@en;
	foaf:depiction <https://ukparliament.github.io/ontologies/standing-order/standing-order.png> ;
	foaf:maker
		[ foaf:name "Robert Brook"; foaf:homepage <https://robert-brook.com/> ],
		[ foaf:name "Thomas Fleming"; foaf:homepage <https://tgfleming.wordpress.com/> ],
		[ foaf:name "Niels D. Goet"; foaf:homepage <https://ngoet.com/> ],
		[ foaf:name "Michael Smethurst"; foaf:homepage <http://smethur.st/> ],
		[ foaf:name "Anya Somerville" ],
	    [ foaf:name "Radoslaw Zubek"; foaf:homepage <https://radoslawzubek.com/> ].


#######  Classes #####

pso:House rdf:type owl:Class ;
	rdfs:label "House"@en ;
	rdfs:comment "A parliamentary House, for example: the House of Lords."@en ;
	rdfs:isDefinedBy <http://parliament.uk/ontologies/standing-order/> .

pso:BusinessExtent rdf:type owl:Class ;
	rdfs:label "Business extent"@en ;
	rdfs:comment "Sets out the extent of business described by a Standing Order as public business or private business."@en ;
	rdfs:isDefinedBy <http://parliament.uk/ontologies/standing-order/> .
	
pso:RevisionSet rdf:type owl:Class ;
	rdfs:label "Revision set"@en ;
	rdfs:comment "A set of orders as they exist at the time of revision of one or more orders."@en ;
	rdfs:isDefinedBy <http://parliament.uk/ontologies/standing-order/> .
	
pso:OrderVersion rdf:type owl:Class ;
	rdfs:label "Order version"@en ;
	rdfs:comment "A version of an order contained by a revision set."@en ;
	rdfs:isDefinedBy <http://parliament.uk/ontologies/standing-order/> .
	
pso:Order rdf:type owl:Class ;
	rdfs:label "Order"@en ;
	rdfs:comment "An order is an FRBR-style work level item, wrapping different manifestations - described as versions - over time. It represents a platonic entity and associated intent."@en ;
	rdfs:isDefinedBy <http://parliament.uk/ontologies/standing-order/> .

pso:FragmentVersion rdf:type owl:Class ;
	rdfs:label "Fragment version"@en ;
	rdfs:comment "A version of a fragment of a Standing Order, contained by a revision set."@en ;
	rdfs:isDefinedBy <http://parliament.uk/ontologies/standing-order/> .

pso:Fragment rdf:type owl:Class ;
	rdfs:label "Fragment"@en ;
	rdfs:comment "A fragment is an FRBR-style work level item, wrapping different manifestations - described as fragment versions - over time. It represents a platonic entity and associated intent."@en ;
	rdfs:isDefinedBy <http://parliament.uk/ontologies/standing-order/> .

pso:Revision rdf:type owl:Class ;
	rdfs:label "Revision"@en ;
	rdfs:comment "A revision is a change to the text of a Standing Order fragment."@en ;
	rdfs:isDefinedBy <http://parliament.uk/ontologies/standing-order/> .


#######  Object properties ##### 

pso:issuedBy rdf:type owl:ObjectProperty ;
	rdfs:label "Issued by"@en ;
	rdfs:comment "Relates a revision set to the House it is issued by."@en ;
	rdfs:domain pso:RevisionSet ;
	rdfs:range pso:House ;
	rdfs:isDefinedBy <http://parliament.uk/ontologies/standing-order/> .
	
pso:revisionSetCoversBusinessExtent rdf:type owl:ObjectProperty ;
	rdfs:label "Revision set covers business extent"@en ;
	rdfs:comment "Relates a revision set to the business extent which that set covers."@en ;
	rdfs:domain pso:RevisionSet ;
	rdfs:range pso:BusinessExtent ;
	rdfs:isDefinedBy <http://parliament.uk/ontologies/standing-order/> .

pso:orderVersionContainedBy rdf:type owl:ObjectProperty ;
	rdfs:label "Order version contained by"@en ;
	rdfs:comment "Relates an order version to the revision set it is contained by."@en ;
	rdfs:domain pso:OrderVersion ;
	rdfs:range pso:RevisionSet ;
	rdfs:isDefinedBy <http://parliament.uk/ontologies/standing-order/> .