@prefix ptr: <http://parliament.uk/ontologies/treaty/> . 
@prefix xsd: <http://www.w3.org/2001/XMLSchema#> . 
@prefix rdf: <http://www.w3.org/1999/02/22-rdf-syntax-ns#> .
@prefix dcterms: <http://purl.org/dc/terms/> .
@prefix owl:     <http://www.w3.org/2002/07/owl#> .
@prefix rdfs:    <http://www.w3.org/2000/01/rdf-schema#> .
@prefix foaf:	<http://xmlns.com/foaf/0.1/> .

<http://parliament.uk/ontologies/treaty/> 
    rdf:type owl:Ontology ;
    dcterms:title "Treaty ontology"@en ;
    dcterms:created "2019-01-16"^^xsd:date ;
	dcterms:rights "Open Parliament Licence v3.0"@en ;
    dcterms:description "An ontology describing the form of treaties considered by UK Parliament."@en ;
	foaf:depiction <https://ukparliament.github.io/ontologies/treaty/treaty.png> ;
	foaf:maker
		[ foaf:name "David Beamish" ],
		[ foaf:name "Robert Brook"; foaf:homepage <https://robert-brook.com/> ],
		[ foaf:name "Jack Dent" ],
		[ foaf:name "Arabella Lang" ],
		[ foaf:name "Michael Smethurst"; foaf:homepage <http://smethur.st/> ],
	    [ foaf:name "Anya Somerville" ],
		[ foaf:name "Jane White" ] .


#######  Classes ##### 	

ptr:Bill rdf:type owl:Class ;
	rdfs:label "Bill"@en ;
	rdfs:comment "A bill presented to Parliament."@en ;
	rdfs:isDefinedBy <http://parliament.uk/ontologies/treaty/> .
	
ptr:DraftAndMadeStatutoryInstrumentSubjectToParliamentaryProcedure rdf:type owl:Class ;
	rdfs:label "Draft and made statutory instrument subject to parliamentary procedure"@en ;
	rdfs:comment "The National Archives classify made instruments as legislation - and draft instruments as draft legislation. Parliament considers both made and draft instruments as part of the legislative process, distinct from a FRBR work as used by TNA. Parliament includes draft instruments in its description of statutory instruments, which are modelled here together."@en ;
	rdfs:isDefinedBy <http://parliament.uk/ontologies/treaty/> .
	
ptr:GovernmentOrganisation rdf:type owl:Class ;
	rdfs:label "Government organisation"@en ;
	rdfs:comment "A government department, agency or public body with responsibility for a sector of public administration."@en ;
	rdfs:isDefinedBy <http://parliament.uk/ontologies/treaty/> .

ptr:Treaty rdf:type owl:Class ;
	rdfs:label "Treaty"@en ;
	rdfs:comment "A treaty is a written agreement between states - or between states and international organisations - which is binding under international law."@en ;
	rdfs:isDefinedBy <http://parliament.uk/ontologies/treaty/> .

ptr:TreatyAsLaid rdf:type owl:Class ;
	rdfs:label "Treaty as laid"@en ;
	rdfs:comment "Treaties requiring ratification - including those treaties requiring ratification to which the United Kingdom is acceding - are subject to the Constitutional Reform and Governance Act 2010. The 2010 Act sets out that such treaties must be laid before Parliament prior to ratification and are then subject to a procedure described in part within the Act. All treaties are laid before Parliament following ratification, though this is not a requirement set out in the 2010 Act and does not trigger a parliamentary procedure."@en ;
	rdfs:isDefinedBy <http://parliament.uk/ontologies/treaty/> .
	
# edited to here
	
ptr:TreatySeriesItem rdf:type owl:Class ;
	rdfs:label "Treaty series item"@en ;
	rdfs:comment "A treaty is listed in a treaty series as a treaty series item. At any time, a treaty series item is always in a treaty series. A treaty may be placed in a new treaty series by means of a new treaty series item. A treaty is listed in one of the bilateral, multilateral or European Union treaty series if it has not come into force in the United Kingdom. A treaty subject to the Constitutional Reform and Governance Act 2010 is listed in one of these series when first laid before Parliament. If Parliament ((( does not object to ))) ratification of the treaty, the treaty becomes available to the government to ratify and then may come into force. When a treaty comes into force, it is listed in the Treaty Series. Use FCO definitions here"@en ;
	rdfs:isDefinedBy <http://parliament.uk/ontologies/treaty/> .
	
ptr:TreatySeries rdf:type owl:Class ;
	rdfs:label "Treaty series"@en ;
	rdfs:comment "A series of which a treaty is an item by means of a treaty series item. The United Kingdom Foreign and Commonwealth Office lists treaties in one of four series: the bilateral series, the multilateral series, the European Union series or the Treaty Series. One of the four treaty series is itself called the Treaty Series."@en ;
	rdfs:isDefinedBy <http://parliament.uk/ontologies/treaty/> .
	

	
##### Object properties ####

ptr:requiresPassageOfBill rdf:type owl:ObjectProperty ;
	rdfs:label "Requires passage of bill"@en ;
	rdfs:comment "Relates a treaty to the required passage of one or more bills in order to enable the satisfaction of treaty obligations."@en ;
	rdfs:domain ptr:Treaty ;
	rdfs:range ptr:Bill ;
	rdfs:isDefinedBy <http://parliament.uk/ontologies/treaty/> .
	
ptr:requiresPassageOfDraftAndMadeStatutoryInstrumentSubjectToParliamentaryProcedure rdf:type owl:ObjectProperty ;
	rdfs:label "Requires passage of a draft or made Statutory Instrument subject to parliamentary procedure"@en ;
	rdfs:comment "Relates a treaty to the required passage of one or more statutory instruments in order to enable the satisfaction of treaty obligations."@en ;
	rdfs:domain ptr:Treaty ;
	rdfs:range ptr:DraftAndMadeStatutoryInstrumentSubjectToParliamentaryProcedure ;
	rdfs:isDefinedBy <http://parliament.uk/ontologies/treaty/> .
	
ptr:laidAs rdf:type owl:ObjectProperty ;
	rdfs:label "Laid as"@en ;
	rdfs:comment "When first laid, a treaty which requires ratification is subject to procedure described in the Constitutional Reform and Governance Act 2010. If the treaty is not rejected by Parliament, it becomes available to the government for ratification. After a treaty is ratified, it is laid before Parliament again, without procedural effect. This property relates a treaty as an abstract work to the form in which it is laid. The 'Laid as' property relates a treaty to the form in which it is laid."@en ;
	rdfs:domain ptr:Treaty ;
	rdfs:range ptr:TreatyAsLaid ;
	rdfs:isDefinedBy <http://parliament.uk/ontologies/treaty/> .

ptr:asSeriesItem rdf:type owl:ObjectProperty ;
	rdfs:label "As series item"@en ;
	rdfs:comment "Relates a treaty as laid before Parliament to a treaty series item. A treaty series item maps a treaty to the treaty series it is listed in at the time of laying. Each treaty series item refers to one treaty as laid. A treaty as laid appears as one treaty series item."@en ;
	rdfs:domain ptr:TreatyAsLaid ;
	rdfs:range ptr:TreatySeriesItem ;
	rdfs:isDefinedBy <http://parliament.uk/ontologies/treaty/> .

ptr:inSeries rdf:type owl:ObjectProperty ;
	rdfs:label "In series"@en ;
	rdfs:comment "Relates a treaty series item to the treaty series it appears in. A treaty series item is listed in a single treaty series."@en ;
	rdfs:domain ptr:TreatySeriesItem ;
	rdfs:range ptr:TreatySeries ;
	rdfs:isDefinedBy <http://parliament.uk/ontologies/treaty/> .
	
ptr:hasLeadDepartment rdf:type owl:ObjectProperty ;
	rdfs:label "Has lead department"@en ;
	rdfs:comment "Relates a treaty to its lead government department. Treaties are laid into Parliament by the Foreign and Commonwealth Office and may have a different assigned lead department."@en ;
	rdfs:domain ptr:Treaty ;
	rdfs:range ptr:GovernmentOrganisation ;
	rdfs:isDefinedBy <http://parliament.uk/ontologies/treaty/> .


	
##### Data properties ####

ptr:commandPaperPrefix rdf:type owl:DatatypeProperty ;
	rdfs:label "Command paper prefix"@en ;
	rdfs:comment "A treaty as laid has a citation formed of a command paper prefix and command paper number. Each command paper has one command paper prefix. Each series of command papers has its own prefix. A series has command paper numbers between 1 and 9999, after which a new series is created."@en ;
	rdfs:domain ptr:TreatyAsLaid ;
	rdfs:range rdfs:Literal ;
	rdfs:isDefinedBy <http://parliament.uk/ontologies/treaty/> .

ptr:commandPaperNumber rdf:type owl:DatatypeProperty ;
	rdfs:label "Command paper number"@en ;
	rdfs:comment "A treaty as laid has a citation formed of a command paper prefix and command paper number. A series has command paper numbers between 1 and 9999, after which a new series is created."@en ;
	rdfs:domain ptr:TreatyAsLaid ;
	rdfs:range rdfs:Literal ;
	rdfs:isDefinedBy <http://parliament.uk/ontologies/treaty/> .

ptr:seriesItemCitation rdf:type owl:DatatypeProperty ;
	rdfs:label "Series item citation"@en ;
	rdfs:comment "An item in a treaty series has a citation, in addition to a Command Paper number: for example, China No. 1 (2017)."@en ;
	rdfs:domain ptr:TreatySeriesItem ;
	rdfs:range rdfs:Literal ;
	rdfs:isDefinedBy <http://parliament.uk/ontologies/treaty/> .
	
ptr:ukRatificationDate rdf:type owl:DatatypeProperty ;
	rdfs:label "UK ratification date"@en ;
	rdfs:comment "The date on which a treaty is recorded as coming into force. Parts of a treaty may come into force on different dates and under differing conditions. Where no single coming into force date is given, coming into force details are given in a coming into force note.."@en ;
	rdfs:domain ptr:Treaty ;
	rdfs:range xsd:date ;
	rdfs:isDefinedBy <http://parliament.uk/ontologies/treaty/> .
	
ptr:ukComingIntoForceDate rdf:type owl:DatatypeProperty ;
	rdfs:label "UK coming into force date"@en ;
	rdfs:comment "The date on which a treaty is recorded as coming into force. Parts of a treaty may come into force on different dates and under differing conditions. Where no single coming into force date is given, coming into force details are given in a coming into force note.."@en ;
	rdfs:domain ptr:Treaty ;
	rdfs:range xsd:date ;
	rdfs:isDefinedBy <http://parliament.uk/ontologies/treaty/> .	

ptr:ukComingIntoForceNote rdf:type owl:DatatypeProperty ;
	rdfs:label "UK coming into force note"@en ;
	rdfs:comment "A coming into force note sets out details of the commencement of provisions or effects forming part or parts of a treaty, or the treaty as a whole where it does not come into force on a single date."@en ;
	rdfs:domain ptr:Treaty ;
	rdfs:range rdf:langString ;
	rdfs:isDefinedBy <http://parliament.uk/ontologies/treaty/> .	