@prefix ptr: <http://parliament.uk/ontologies/treaty/> . 
@prefix xsd: <http://www.w3.org/2001/XMLSchema#> . 
@prefix rdf: <http://www.w3.org/1999/02/22-rdf-syntax-ns#> .
@prefix dcterms: <http://purl.org/dc/terms/> .
@prefix owl:     <http://www.w3.org/2002/07/owl#> .
@prefix rdfs:    <http://www.w3.org/2000/01/rdf-schema#> .
@prefix foaf:	<http://xmlns.com/foaf/0.1/> .

<http://parliament.uk/ontologies/treaty/> 
    rdf:type owl:Ontology ;
    dcterms:title "Treaty ontology"@en ;
    dcterms:created "2019-01-16"^^xsd:date ;
	dcterms:rights "Open Parliament Licence v3.0"@en ;
    dcterms:description "An ontology describing the form of treaties considered by UK Parliament."@en ;
	foaf:depiction <https://ukparliament.github.io/ontologies/treaty/treaty.png> ;
	foaf:maker
		[ foaf:name "David Beamish" ],
		[ foaf:name "Robert Brook"; foaf:homepage <https://robert-brook.com/> ],
		[ foaf:name "Jack Dent" ],
		[ foaf:name "Arabella Lang" ],
		[ foaf:name "Michael Smethurst"; foaf:homepage <http://smethur.st/> ],
	    [ foaf:name "Anya Somerville" ],
		[ foaf:name "Jane White" ] .


#######  Classes ##### 	

ptr:Bill rdf:type owl:Class ;
	rdfs:label "Bill"@en ;
	rdfs:comment "A bill presented to Parliament."@en ;
	rdfs:isDefinedBy <http://parliament.uk/ontologies/treaty/> .
	
ptr:DraftAndMadeStatutoryInstrumentSubjectToParliamentaryProcedure rdf:type owl:Class ;
	rdfs:label "Draft and made statutory instrument subject to parliamentary procedure"@en ;
	rdfs:comment "The National Archives classify made instruments as legislation and draft instruments as draft legislation. Parliament considers both made and draft instruments as part of the legislative process, distinct from a FRBR work as used by The National Archives. Parliament includes draft instruments in its description of statutory instruments which are modelled here together."@en ;
	rdfs:isDefinedBy <http://parliament.uk/ontologies/treaty/> .

ptr:Treaty rdf:type owl:Class ;
	rdfs:label "Treaty"@en ;
	rdfs:comment "A text recording agreement between two or more parties, including nation states and international organisations. Treaties between nation states are described by the Vienna Convention on the Law of Treaties. Treaties between nation states and international organisations and between international organisations themselves are described by the Vienna Convention on the Law of Treaties between States and International Organizations or between International Organizations."@en ;
	rdfs:isDefinedBy <http://parliament.uk/ontologies/treaty/> .

ptr:TreatyAsLaid rdf:type owl:Class ;
	rdfs:label "Treaty as laid"@en ;
	rdfs:comment "Treaties requiring ratification are subject to the Constitutional Reform and Governance Act 2010 and are laid before Parliament before ratification and afterwards on coming into force. Laying before ratification is subject to procedure described in part within the 2010 Act."@en ;
	rdfs:isDefinedBy <http://parliament.uk/ontologies/treaty/> .
	
ptr:TreatySeriesItem rdf:type owl:Class ;
	rdfs:label "Treaty series item"@en ;
	rdfs:comment "A treaty is listed in a treaty series as a treaty series item. At any time, a treaty series item is always in a treaty series. A treaty may be placed in a new treaty series by means of a new treaty series item. A treaty is listed in one of the bilateral, multilateral or European Union treaty series if it has not come into force in the United Kingdom. A treaty subject to the Constitutional Reform and Governance Act 2010 is listed in one of these series when first laid before Parliament. If Parliament permits ratification of the treaty, the treaty becomes available to the government to ratify and then may come into force. When a treaty comes into force, it is listed in the Treaty Series."@en ;
	rdfs:isDefinedBy <http://parliament.uk/ontologies/treaty/> .
	
ptr:TreatySeries rdf:type owl:Class ;
	rdfs:label "Treaty series"@en ;
	rdfs:comment "A series of which a treaty is an item by means of a treaty series item. The United Kingdom Foreign and Commonwealth Office lists treaties in one of four series: the bilateral series, the multilateral series, the European Union series or the Treaty Series. One of the four treaty series is itself called the Treaty Series."@en ;
	rdfs:isDefinedBy <http://parliament.uk/ontologies/treaty/> .
	
ptr:InForceStatus rdf:type owl:Class ;
	rdfs:label "In force status"@en ;
	rdfs:comment "The process by which a party to a treaty brings that treaty into force in their jurisdiction."@en ;
	rdfs:isDefinedBy <http://parliament.uk/ontologies/treaty/> .
	
ptr:GovernmentOrganisation rdf:type owl:Class ;
	rdfs:label "Government organisation"@en ;
	rdfs:comment "A government department, agency or public body with responsibility for a sector of public administration."@en ;
	rdfs:isDefinedBy <http://parliament.uk/ontologies/treaty/> .
	
ptr:Action rdf:type owl:Class ;
	rdfs:label "Action"@en ;
	rdfs:comment "An action taken by a party as part of the process of entering into a treaty."@en ;
	rdfs:isDefinedBy <http://parliament.uk/ontologies/treaty/> .

ptr:ActionType rdf:type owl:Class ;
	rdfs:label "Action type"@en ;
	rdfs:comment "The type of action taken by a party on a treaty. For example: signing, ratification, accession or withdrawal."@en ;
	rdfs:isDefinedBy <http://parliament.uk/ontologies/treaty/> .
		
ptr:Party rdf:type owl:Class ;
	rdfs:label "Party"@en ;
	rdfs:comment "An entity having the capacity to enter into treaty obligations. For example: a nation state, an intergovernmental organisation or internationally recognised authority."@en ;
	rdfs:isDefinedBy <http://parliament.uk/ontologies/treaty/> .
	

	
##### Object properties ####

ptr:requiresPassageOfBill rdf:type owl:ObjectProperty ;
	rdfs:label "Requires passage of bill"@en ;
	rdfs:comment "Relates a treaty to the required passage of one or more bills in order to enable the satisfaction of treaty obligations."@en ;
	rdfs:domain ptr:Treaty ;
	rdfs:range ptr:Bill ;
	rdfs:isDefinedBy <http://parliament.uk/ontologies/treaty/> .
	
ptr:requiresPassageOfDraftAndMadeStatutoryInstrumentSubjectToParliamentaryProcedure rdf:type owl:ObjectProperty ;
	rdfs:label "Requires passage of a draft or made Statutory Instrument subject to parliamentary procedure"@en ;
	rdfs:comment "Relates a treaty to the required passage of one or more statutory instruments in order to enable the satisfaction of treaty obligations."@en ;
	rdfs:domain ptr:Treaty ;
	rdfs:range ptr:DraftAndMadeStatutoryInstrumentSubjectToParliamentaryProcedure ;
	rdfs:isDefinedBy <http://parliament.uk/ontologies/treaty/> .
	
ptr:laidAs rdf:type owl:ObjectProperty ;
	rdfs:label "Laid as"@en ;
	rdfs:comment "When first laid, a treaty which requires ratification is subject to procedure described in the Constitutional Reform and Governance Act 2010. If the treaty is not rejected by Parliament, it becomes available to the government for ratification. After a treaty is ratified, it is laid before Parliament again, without procedural effect. This property relates a treaty as an abstract work to the form in which it is laid. The 'Laid as' property relates a treaty to the form in which it is laid."@en ;
	rdfs:domain ptr:Treaty ;
	rdfs:range ptr:TreatyAsLaid ;
	rdfs:isDefinedBy <http://parliament.uk/ontologies/treaty/> .

ptr:asSeriesItem rdf:type owl:ObjectProperty ;
	rdfs:label "As series item"@en ;
	rdfs:comment "Relates a treaty as laid before Parliament to a treaty series item. A treaty series item maps a treaty to the treaty series it is listed in at the time of laying. Each treaty series item refers to one treaty as laid. A treaty as laid appears as one treaty series item."@en ;
	rdfs:domain ptr:TreatyAsLaid ;
	rdfs:range ptr:TreatySeriesItem ;
	rdfs:isDefinedBy <http://parliament.uk/ontologies/treaty/> .

ptr:inSeries rdf:type owl:ObjectProperty ;
	rdfs:label "In series"@en ;
	rdfs:comment "Relates a treaty series item to the treaty series it appears in. A treaty series item is listed in a single treaty series."@en ;
	rdfs:domain ptr:TreatySeriesItem ;
	rdfs:range ptr:TreatySeries ;
	rdfs:isDefinedBy <http://parliament.uk/ontologies/treaty/> .
	
ptr:hasInForceStatus rdf:type owl:ObjectProperty ;
	rdfs:label "Has in force status"@en ;
	rdfs:comment "Relates a treaty to its in force status for a party."@en ;
	rdfs:domain ptr:Treaty ;
	rdfs:range ptr:InForceStatus ;
	rdfs:isDefinedBy <http://parliament.uk/ontologies/treaty/> .
	
ptr:inForceStatusFor rdf:type owl:ObjectProperty ;
	rdfs:label "In force status for"@en ;
	rdfs:comment "Relates the in force status of a treaty to a party."@en ;
	rdfs:domain ptr:InForceStatus ;
	rdfs:range ptr:Party ;
	rdfs:isDefinedBy <http://parliament.uk/ontologies/treaty/> .
	
ptr:hasLeadDepartment rdf:type owl:ObjectProperty ;
	rdfs:label "Has lead department"@en ;
	rdfs:comment "Relates a treaty to its lead government department. Treaties are laid into Parliament by the Foreign and Commonwealth Office and may have a different assigned lead department."@en ;
	rdfs:domain ptr:Treaty ;
	rdfs:range ptr:GovernmentOrganisation ;
	rdfs:isDefinedBy <http://parliament.uk/ontologies/treaty/> .
	
ptr:actsOn rdf:type owl:ObjectProperty ;
	rdfs:label "Acts on"@en ;
	rdfs:comment "Relates an action by a party to the treaty the action is being applied to. A treaty may have one or more actions over time taken by a single party. Each action applies to a single treaty and is by a single party."@en ;
	rdfs:domain ptr:Action ;
	rdfs:range ptr:Treaty ;
	rdfs:isDefinedBy <http://parliament.uk/ontologies/treaty/> .
	
ptr:completesAction rdf:type owl:ObjectProperty ;
	rdfs:label "Completes action"@en ;
	rdfs:comment "Relates a party to an action they complete on a treaty. A party may complete many actions on a treaty over time. An action on a treaty is completed by one party."@en ;
	rdfs:domain ptr:Party ;
	rdfs:range ptr:Action ;
	rdfs:isDefinedBy <http://parliament.uk/ontologies/treaty/> .
	
ptr:hasActionType rdf:type owl:ObjectProperty ;
	rdfs:label "Has action type"@en ;
	rdfs:comment "Relates an action taken by a party to the type of that action. Each action has one type. Many actions may have the same action type: for example, many parties might ratify a treaty at different times. "@en ;
	rdfs:domain ptr:Action ;
	rdfs:range ptr:ActionType ;
	rdfs:isDefinedBy <http://parliament.uk/ontologies/treaty/> .
	

								# edited to here
	

					
	
##### Data properties ####

ptr:commandPaperPrefix rdf:type owl:DatatypeProperty ;
	rdfs:label "Command paper prefix"@en ;
	rdfs:comment "A command paper prefix is applied until a command paper number reaches 9999, after which the command paper prefix is changed. Each command paper has one command paper prefix."@en ;
	rdfs:domain ptr:TreatyAsLaid ;
	rdfs:range rdfs:Literal ;
	rdfs:isDefinedBy <http://parliament.uk/ontologies/treaty/> .

ptr:commandPaperNumber rdf:type owl:DatatypeProperty ;
	rdfs:label "Command paper number"@en ;
	rdfs:comment "A command paper number follows its prefix and does not exceed 9999. Each command paper has one command paper number."@en ;
	rdfs:domain ptr:TreatyAsLaid ;
	rdfs:range rdfs:Literal ;
	rdfs:isDefinedBy <http://parliament.uk/ontologies/treaty/> .

ptr:seriesItemCitation rdf:type owl:DatatypeProperty ;
	rdfs:label "Series item citation"@en ;
	rdfs:comment "Each item in a treaty series has its own citation."@en ;
	rdfs:domain ptr:TreatySeriesItem ;
	rdfs:range rdfs:Literal ;
	rdfs:isDefinedBy <http://parliament.uk/ontologies/treaty/> .
	
ptr:comingIntoForceNote rdf:type owl:DatatypeProperty ;
	rdfs:label "Coming into force note"@en ;
	rdfs:comment ""@en ;
	rdfs:domain ptr:InForceStatus ;
	rdfs:range rdf:langString ;
	rdfs:isDefinedBy <http://parliament.uk/ontologies/treaty/> .	
	
ptr:actionDate rdf:type owl:DatatypeProperty ;
	rdfs:label "Action date"@en ;
	rdfs:comment "The date on which an action was completed or is due to be completed. An action may not have a recorded date."@en ;
	rdfs:domain ptr:Action ;
	rdfs:range xsd:date ;
	rdfs:isDefinedBy <http://parliament.uk/ontologies/treaty/> .