@prefix prec: <http://parliament.uk/ontologies/record/> . 
@prefix xsd: <http://www.w3.org/2001/XMLSchema#> . 
@prefix rdf: <http://www.w3.org/1999/02/22-rdf-syntax-ns#> .
@prefix dcterms: <http://purl.org/dc/terms/> .
@prefix owl:     <http://www.w3.org/2002/07/owl#> .
@prefix rdfs:    <http://www.w3.org/2000/01/rdf-schema#> .
@prefix foaf:	<http://xmlns.com/foaf/0.1/> .

<http://parliament.uk/ontologies/record/> 
    rdf:type owl:Ontology ;
    dcterms:title "Record ontology"@en ;
    dcterms:created "2018-07-09"^^xsd:date ;
	dcterms:rights "Open Parliament Licence v3.0"@en ;
    dcterms:description "A model informed by FRBR - describing works, collections of works, their expressions and manifestations."@en ;
	foaf:depiction <https://ukparliament.github.io/ontologies/record/record.png> ;
	foaf:maker
		[ foaf:name "Robert Brook"; foaf:homepage <https://robert-brook.com/> ],
		[ foaf:name "Silver Oliver" ],
		[ foaf:name "Michael Smethurst"; foaf:homepage <http://smethur.st/> ],
	    [ foaf:name "Anya Somerville" ] .


#######  Classes #####

prec:Work rdf:type owl:Class ;
	rdfs:label "Work"@en ;
	rdfs:comment "A distinct intellectual creation, similar to a work as defined in FRBR."@en ;
	rdfs:isDefinedBy <http://parliament.uk/ontologies/record/> .
	
prec:Publisher rdf:type owl:Class ;
	rdfs:label "Publisher"@en ;
	rdfs:comment "An entity responsible for making a resource available."@en ;
	rdfs:isDefinedBy <http://parliament.uk/ontologies/record/> .
	
prec:Place rdf:type owl:Class ;
	rdfs:label "Place"@en ;
	rdfs:comment "A place named in a geography."@en ;
	rdfs:isDefinedBy <http://parliament.uk/ontologies/record/> .
	
prec:EditorialForm rdf:type owl:Class ;
	rdfs:label "Editorial form"@en ;
	rdfs:comment "The editorial form of a work, for example: a report, an article, a transcript, or the minutes of a meeting."@en ;
	rdfs:isDefinedBy <http://parliament.uk/ontologies/record/> .
	
prec:Collection rdf:type owl:Class ;
	rdfs:label "Collection"@en ;
	rdfs:comment "A curated collection of works."@en ;
	rdfs:isDefinedBy <http://parliament.uk/ontologies/record/> .
	
prec:Series rdf:type owl:Class ;
	rdfs:subClassOf prec:Collection ;
	rdfs:label "Series"@en ;
	rdfs:comment "A specialised form of collection, allowing works to be placed in an order."@en ;
	rdfs:isDefinedBy <http://parliament.uk/ontologies/record/> .
	
prec:SeriesPosition rdf:type owl:Class ;
	rdfs:label "Series position"@en ;
	rdfs:comment "The position of a work within a series of works."@en ;
	rdfs:isDefinedBy <http://parliament.uk/ontologies/record/> .
	
prec:Focus rdf:type owl:Class ;
	rdfs:label "Focus"@en ;
	rdfs:comment "A focus area for a manifestation or collection of works. Allows us to point at any modelled thing as a focus area, for example: a committee or a bill."@en ;
	rdfs:isDefinedBy <http://parliament.uk/ontologies/record/> .
	
prec:Expression rdf:type owl:Class ;
	rdfs:label "Expression"@en ;
	rdfs:comment "A work may be realised - as an expression - having more than one format, for example: a podcast episode made available as an audio file and as a text transcript."@en ;
	rdfs:isDefinedBy <http://parliament.uk/ontologies/record/> .
	
prec:Format rdf:type owl:Class ;
	rdfs:label "Format"@en ;
	rdfs:comment "The format taken by the expression of a work, for example: the format of the expression of a podcast episode - as an audio file, or as a text transcript."@en ;
	rdfs:isDefinedBy <http://parliament.uk/ontologies/record/> .
	
prec:Manifestation rdf:type owl:Class ;
	rdfs:label "Manifestation"@en ;
	rdfs:comment "A manifestation of an expression of a work, allowing for multiple versions of an expression over time, for example: an edition of a book, or a remastered audio file of a podcast episode."@en ;
	rdfs:isDefinedBy <http://parliament.uk/ontologies/record/> .
	
prec:Contribution rdf:type owl:Class ;
	rdfs:label "Contribution"@en ;
	rdfs:comment "A contribution by an agent, for example: by a person or by a corporate author."@en ;
	rdfs:isDefinedBy <http://parliament.uk/ontologies/record/> .
	
prec:Revision rdf:type owl:Class ;
	rdfs:label "Revision"@en ;
	rdfs:comment "The type of an edit between two manifestations, for example: a major update or a minor update."@en ;
	rdfs:isDefinedBy <http://parliament.uk/ontologies/record/> .
	
prec:RevisionType rdf:type owl:Class ;
	rdfs:label "Revision type"@en ;
	rdfs:comment "The type of an edit between two manifestations, for example: a major update or a minor update."@en ;
	rdfs:isDefinedBy <http://parliament.uk/ontologies/record/> .
	
prec:File rdf:type owl:Class ;
	rdfs:label "File"@en ;
	rdfs:comment "A file associated with a manifestation of a work, for example: a spreadsheet, a PDF or a Word document."@en ;
	rdfs:isDefinedBy <http://parliament.uk/ontologies/record/> .
	
				

#######  Object properties ##### 

prec:hasPublisher rdf:type owl:ObjectProperty ;
	rdfs:label "Has publisher"@en ;
	rdfs:comment "Relates a work to a publisher or publishers."@en ;
	rdfs:domain prec:Work ;
	rdfs:range prec:Publisher ;
	rdfs:isDefinedBy <http://parliament.uk/ontologies/record/> .
	
prec:hasGeographicScope rdf:type owl:ObjectProperty ;
	rdfs:label "Has geographic scope"@en ;
	rdfs:comment "Denotes the geographic scope of a work, the scope being a geographic place."@en ;
	rdfs:domain prec:Work ;
	rdfs:range prec:Place ;
	rdfs:isDefinedBy <http://parliament.uk/ontologies/record/> .
	
prec:takesEditorialForm rdf:type owl:ObjectProperty ;
	rdfs:label "Takes editorial form"@en ;
	rdfs:comment "Relates a work to an editorial form."@en ;
	rdfs:domain prec:Work ;
	rdfs:range prec:EditorialForm ;
	rdfs:isDefinedBy <http://parliament.uk/ontologies/record/> .
	
prec:partOfCollection rdf:type owl:ObjectProperty ;
	rdfs:label "Part of collection"@en ;
	rdfs:comment "Includes a work within a collection, as a part of that collection."@en ;
	rdfs:domain prec:Work ;
	rdfs:range prec:Collection ;
	rdfs:isDefinedBy <http://parliament.uk/ontologies/record/> .
	
prec:collectionPartOfCollection rdf:type owl:ObjectProperty ;
	rdfs:label "Collection part of collection"@en ;
	rdfs:comment "Relates a collection to a wider collection it forms part of, for example: a collection of works on health policy generally formed of collections of works concerned with particular areas of health policy."@en ;
	rdfs:domain prec:Collection ;
	rdfs:range prec:Collection ;
	rdfs:isDefinedBy <http://parliament.uk/ontologies/record/> .
	
prec:inSeriesPosition rdf:type owl:ObjectProperty ;
	rdfs:label "In series position"@en ;
	rdfs:comment "Relates a work to the position that work has within a series."@en ;
	rdfs:domain prec:Work ;
	rdfs:range prec:SeriesPosition ;
	rdfs:isDefinedBy <http://parliament.uk/ontologies/record/> .

prec:inSeries rdf:type owl:ObjectProperty ;
	rdfs:label "In series"@en ;
	rdfs:comment "Relates the series position of a work to a series in which that work appears."@en ;
	rdfs:domain prec:SeriesPosition ;
	rdfs:range prec:Series ;
	rdfs:isDefinedBy <http://parliament.uk/ontologies/record/> .

prec:expressionOf rdf:type owl:ObjectProperty ;
	rdfs:label "Expression of"@en ;
	rdfs:comment "Relates an expression to the work as expressed. An expression is of a single work. A work has one or more expressions."@en ;
	rdfs:domain prec:Expression ;
	rdfs:range prec:Work ;
	rdfs:isDefinedBy <http://parliament.uk/ontologies/record/> .
	
prec:hasFormat rdf:type owl:ObjectProperty ;
	rdfs:label "Has format"@en ;
	rdfs:comment "Relates an expression to the format taken by that expression. Different expressions of the same work may have different formats."@en ;
	rdfs:domain prec:Expression ;
	rdfs:range prec:Format ;
	rdfs:isDefinedBy <http://parliament.uk/ontologies/record/> .
	
prec:manifestationOf rdf:type owl:ObjectProperty ;
	rdfs:label "Manifestation of"@en ;
	rdfs:comment "Relates a manifestation of an expression to that expression. An expression may have more than one manifestation. A manifestation has a single expression."@en ;
	rdfs:domain prec:Manifestation ;
	rdfs:range prec:Expression ;
	rdfs:isDefinedBy <http://parliament.uk/ontologies/record/> .
	
prec:manifestationHasFocus rdf:type owl:ObjectProperty ;
	rdfs:label "Manifestation has focus"@en ;
	rdfs:comment "Relates a manifestation to the focus area of that manifestation."@en ;
	rdfs:domain prec:Manifestation ;
	rdfs:range prec:Focus ;
	rdfs:isDefinedBy <http://parliament.uk/ontologies/record/> .
	
prec:collectionHasFocus rdf:type owl:ObjectProperty ;
	rdfs:label "Collection has focus"@en ;
	rdfs:comment "Relates a collection to the focus area of that collection."@en ;
	rdfs:domain prec:Collection ;
	rdfs:range prec:Focus ;
	rdfs:isDefinedBy <http://parliament.uk/ontologies/record/> .
	
prec:hasContribution rdf:type owl:ObjectProperty ;
	rdfs:label "hasContribution"@en ;
	rdfs:comment "Relates a manifestation to a contribution. Contributors to a work may differ across different manifestations of that work."@en ;
	rdfs:domain prec:Manifestation ;
	rdfs:range prec:Contribution ;
	rdfs:isDefinedBy <http://parliament.uk/ontologies/record/> .
	
prec:fromManifestation rdf:type owl:ObjectProperty ;
	rdfs:label "From manifestation"@en ;
	rdfs:comment "Relates a revision to the manifestation which was revised."@en ;
	rdfs:domain prec:Revision ;
	rdfs:range prec:Manifestation ;
	rdfs:isDefinedBy <http://parliament.uk/ontologies/record/> .
	
prec:toManifestation rdf:type owl:ObjectProperty ;
	rdfs:label "To manifestation"@en ;
	rdfs:comment "Relates a revision to the resulting revised manifestation."@en ;
	rdfs:domain prec:Revision ;
	rdfs:range prec:Manifestation ;
	rdfs:isDefinedBy <http://parliament.uk/ontologies/record/> .
	
prec:hasRevisionType rdf:type owl:ObjectProperty ;
	rdfs:label "Has revision type"@en ;
	rdfs:comment "Relates a revision to the revision type of that manifestation."@en ;
	rdfs:domain prec:Revision ;
	rdfs:range prec:RevisionType ;
	rdfs:isDefinedBy <http://parliament.uk/ontologies/record/> .
	
prec:hasAttachment rdf:type owl:ObjectProperty ;
	rdfs:label "Has attachment"@en ;
	rdfs:comment "Relates a manifestation to a file.."@en ;
	rdfs:domain prec:Manifestation ;
	rdfs:range prec:File ;
	rdfs:isDefinedBy <http://parliament.uk/ontologies/record/> .
	

				
	
##### Data properties ####	
	
prec:scope rdf:type owl:DatatypeProperty ;
	rdfs:label "Scope"@en ;
	rdfs:comment "The scope of a work, for example: the scope of a POST briefing."@en ;
	rdfs:domain prec:Work ;
	rdfs:range rdf:langString ;
	rdfs:isDefinedBy <http://parliament.uk/ontologies/record/> .

prec:referenceNumber rdf:type owl:DatatypeProperty ;
	rdfs:label "Reference number"@en ;
	rdfs:comment "The reference number of a work."@en ;
	rdfs:domain prec:Work ;
	rdfs:range rdfs:Literal ;
	rdfs:isDefinedBy <http://parliament.uk/ontologies/record/> .
	
prec:minimumReadingAge rdf:type owl:DatatypeProperty ;
	rdfs:label "Minimum reading age"@en ;
	rdfs:comment "The minimum reading age for a manifestation of a work."@en ;
	rdfs:domain prec:Manifestation ;
	rdfs:range xsd:integer ;
	rdfs:isDefinedBy <http://parliament.uk/ontologies/record/> .
	
prec:publishedAt rdf:type owl:DatatypeProperty ;
	rdfs:label "Published at"@en ;
	rdfs:comment "The date and time of the publication of a manifestation."@en ;
	rdfs:domain prec:Manifestation ;
	rdfs:range xsd:dateTime ;
	rdfs:isDefinedBy <http://parliament.uk/ontologies/record/> .
	
prec:mediaType rdf:type owl:DatatypeProperty ;
	rdfs:label "Media type"@en ;
	rdfs:comment "The media type of a file."@en ;
	rdfs:domain prec:File ;
	rdfs:range rdfs:Literal ;
	rdfs:isDefinedBy <http://parliament.uk/ontologies/record/> .
	
prec:hasRevisionDescription rdf:type owl:DatatypeProperty ;
	rdfs:label "Has revision description"@en ;
	rdfs:comment "The description of a revision made to a manifestation."@en ;
	rdfs:domain prec:Revision ;
	rdfs:range rdf:langString ;
	rdfs:isDefinedBy <http://parliament.uk/ontologies/record/> .