@prefix ppub: <http://parliament.uk/ontologies/publisher/> . 
@prefix xsd: <http://www.w3.org/2001/XMLSchema#> . 
@prefix rdf: <http://www.w3.org/1999/02/22-rdf-syntax-ns#> .
@prefix dcterms: <http://purl.org/dc/terms/> .
@prefix owl:     <http://www.w3.org/2002/07/owl#> .
@prefix rdfs:    <http://www.w3.org/2000/01/rdf-schema#> .

<http://parliament.uk/ontologies/publisher/> 
    rdf:type owl:Ontology ;
    dcterms:title "Publisher ontology"@en ;
    dcterms:created "2018-06-28"^^xsd:date ;
	dcterms:rights "Open Parliament Licence v3.0"@en ;
    dcterms:description "A model describing the publishing of material by offices within Parliament, for example: the House of Commons Library."@en ;
	foaf:depiction <https://ukparliament.github.io/ontologies/publisher/publisher.png> ;
	foaf:maker
		[ foaf:name "Robert Brook"; foaf:homepage <https://robert-brook.com/> ],
		[ foaf:name "Silver Oliver" ],
		[ foaf:name "Michael Smethurst"; foaf:homepage <http://smethur.st/> ],
	    [ foaf:name "Anya Somerville" ] .


#######  Classes ##### 	

ppub:Agent rdf:type owl:Class ;
	rdfs:label "Agent"@en ;
	rdfs:comment "Agents include people and groups, including those outside the Parliamentary Service, participating in parliamentary procedure and contributing to the wider work of Parliament."@en ;
	rdfs:isDefinedBy <http://parliament.uk/ontologies/publisher/> .
	
ppub:Group rdf:type owl:Class ;
	rdfs:subClassOf ppub:Agent ;
	rdfs:label "Group"@en ;
	rdfs:comment "A group of people. Groups may contain other groups or be empty."@en ;
	rdfs:isDefinedBy <http://parliament.uk/ontologies/publisher/> .
	
ppub:Publisher rdf:type owl:Class ;
	rdfs:subClassOf ppub:Agent ;
	rdfs:label "Publisher"@en ;
	rdfs:comment "An entity responsible for making a resource available."@en ;
	rdfs:isDefinedBy <http://parliament.uk/ontologies/publisher/> .
	
ppub:EditorialBoard rdf:type owl:Class ;
	rdfs:subClassOf ppub:Group ;
	rdfs:label "Editorial board"@en ;
	rdfs:comment "A group overseeing a publisher, for example: the board of POST, made up of Members of Parliament, considering and approving areas of research."@en ;
	rdfs:isDefinedBy <http://parliament.uk/ontologies/publisher/> .
	
ppub:House rdf:type owl:Class ;
	rdfs:subClassOf ppub:Group ;
	rdfs:label "House"@en ;
	rdfs:comment "A parliamentary House, for example: the House of Lords."@en ;
	rdfs:isDefinedBy <http://parliament.uk/ontologies/publisher/> .
	
ppub:ResearchService rdf:type owl:Class ;
	rdfs:subClassOf ppub:Publisher ;
	rdfs:label "Research service"@en ;
	rdfs:comment "A group of researchers, for example: in the Library of the House of Commons, in the Library of the House of Lords or the Parliamentary Office of Science and Technology."@en ;
	rdfs:isDefinedBy <http://parliament.uk/ontologies/publisher/> .
	
ppub:ResearchSection rdf:type owl:Class ;
	rdfs:subClassOf ppub:Publisher ;
	rdfs:label "Research section"@en ;
	rdfs:comment "A group of researchers within the Library of the House of Commons having a particular focus, for example: the Parliament and Constitution Centre."@en ;
	rdfs:isDefinedBy <http://parliament.uk/ontologies/publisher/> .
	
ppub:Concept rdf:type owl:Class ;
	rdfs:label "Concept"@en ;
	rdfs:comment "A SKOS Concept, for example: a library subject term."@en ;
	rdfs:isDefinedBy <http://parliament.uk/ontologies/publisher/> .
	

##### Object properties ####

ppub:hasEditorialBoard rdf:type owl:ObjectProperty ;
	rdfs:label "Has editorial board"@en ;
	rdfs:comment "Relates a publisher to its editorial board."@en ;
	rdfs:domain ppub:Publisher ;
	rdfs:range ppub:EditorialBoard ;
	rdfs:isDefinedBy <http://parliament.uk/ontologies/publisher/> .
	
ppub:hasResearchService rdf:type owl:ObjectProperty ;
	rdfs:label "Has research service"@en ;
	rdfs:comment "Relates a House to a research service. A research service may belong to one House or both, for example: the Parliamentary Office of Science and Technology, a bicameral office."@en ;
	rdfs:domain ppub:House ;
	rdfs:range ppub:ResearchService ;
	rdfs:isDefinedBy <http://parliament.uk/ontologies/publisher/> .
	
ppub:hasResearchSection rdf:type owl:ObjectProperty ;
	rdfs:label "Has section"@en ;
	rdfs:comment "Relates a research service to a research section within that service."@en ;
	rdfs:domain ppub:ResearchService ;
	rdfs:range ppub:ResearchSection ;
	rdfs:isDefinedBy <http://parliament.uk/ontologies/publisher/> .
	
ppub:focus rdf:type owl:ObjectProperty ;
	rdfs:label "Focus"@en ;
	rdfs:comment "Relates a publisher to one or more policy areas, policy areas being represented as SKOS concepts."@en ;
	rdfs:domain ppub:Publisher ;
	rdfs:range ppub:Concept ;
	rdfs:isDefinedBy <http://parliament.uk/ontologies/publisher/> .