@prefix pcon: <http://parliament.uk/ontologies/contribution/> . 
@prefix xsd: <http://www.w3.org/2001/XMLSchema#> . 
@prefix rdf: <http://www.w3.org/1999/02/22-rdf-syntax-ns#> .
@prefix dcterms: <http://purl.org/dc/terms/> .
@prefix owl:     <http://www.w3.org/2002/07/owl#> .
@prefix rdfs:    <http://www.w3.org/2000/01/rdf-schema#> .
@prefix foaf:	<http://xmlns.com/foaf/0.1/> .

<http://parliament.uk/ontologies/contribution/> 
    rdf:type owl:Ontology ;
    dcterms:title "Contribution ontology"@en ;
    dcterms:created "2018-06-28"^^xsd:date ;
	dcterms:rights "Open Parliament Licence v3.0"@en ;
    dcterms:description "A model describing contributions made by people or groups."@en ;
	foaf:depiction <https://ukparliament.github.io/ontologies/contribution/contribution.png> ;
	foaf:maker
		[ foaf:name "Robert Brook"; foaf:homepage <https://robert-brook.com/> ],
		[ foaf:name "Michael Smethurst"; foaf:homepage <http://smethur.st/> ],
	    [ foaf:name "Anya Somerville" ] .


#######  Classes #####

pcon:Agent rdf:type owl:Class ;
	rdfs:label "Agent"@en ;
	rdfs:comment "An agent. The superset of all people and all groups of people."@en ;
	rdfs:isDefinedBy <http://parliament.uk/ontologies/contribution/> .
	
pcon:Contribution rdf:type owl:Class ;
	rdfs:label "Contribution"@en ;
	rdfs:comment "A contribution by an individual or organisation to a document or committee inquiry etc."@en ;
	rdfs:isDefinedBy <http://parliament.uk/ontologies/contribution/> .
	
pcon:ContributionRole rdf:type owl:Class ;
	rdfs:label "ContributionRole"@en ;
	rdfs:comment "The type of contribution made. Might be as an author or reviewer or inquiry witness etc."@en ;
	rdfs:isDefinedBy <http://parliament.uk/ontologies/contribution/> .
	
pcon:Incumbency rdf:type owl:Class ;
	rdfs:label "Incumbency"@en ;
	rdfs:comment "A position held by a person for a period of time. e.g. Philip Hammond occupying the position of Foreign Secretary between two dates."@en ;
	rdfs:isDefinedBy <http://parliament.uk/ontologies/contribution/> .
	
				

#######  Object properties ##### 

pcon:makesContribution rdf:type owl:ObjectProperty ;
	rdfs:label "makesContribution"@en ;
	rdfs:comment "Relates a person or group to a contribution they've made."@en ;
	rdfs:domain pcon:Agent ;
	rdfs:range pcon:Contribution ;
	rdfs:isDefinedBy <http://parliament.uk/ontologies/contribution/> .
	
pcon:hasContributionRole rdf:type owl:ObjectProperty ;
	rdfs:label "hasContributionRole"@en ;
	rdfs:comment "Relates a contribution to the type of contribution made."@en ;
	rdfs:domain pcon:Contribution ;
	rdfs:range pcon:ContributionRole ;
	rdfs:isDefinedBy <http://parliament.uk/ontologies/contribution/> .
	
pcon:inCapacity rdf:type owl:ObjectProperty ;
	rdfs:label "inCapacity"@en ;
	rdfs:comment "Relates a contribution to an incumbency of the person making the contribution e.g. a person making a contribution in their capacity of holding a CEO position of an organisation."@en ;
	rdfs:domain pcon:Contribution ;
	rdfs:range pcon:Incumbency ;
	rdfs:isDefinedBy <http://parliament.uk/ontologies/contribution/> .
	
	
	
#######  Data properties ##### 

pcon:isPublic rdf:type owl:DatatypeProperty ;
	rdfs:label "Is public"@en ;
	rdfs:comment "Relates a contribution to whether not that contribution is made public. The is public flag will by necessity not be public."@en ;
	rdfs:domain pcon:Contribution ;
	rdfs:range xsd:boolean ;
	rdfs:isDefinedBy <http://parliament.uk/ontologies/contribution/> .

pcon:displayOrder rdf:type owl:DatatypeProperty ;
	rdfs:label "Display order"@en ;
	rdfs:comment "Relates a contribution type to its display order."@en ;
	rdfs:domain pcon:ContributionType ;
	rdfs:range xsd:integer ;
	rdfs:isDefinedBy <http://parliament.uk/ontologies/contribution/> .