@prefix pwqa: <http://parliament.uk/ontologies/written-question-and-answer/> . 
@prefix xsd: <http://www.w3.org/2001/XMLSchema#> . 
@prefix rdf: <http://www.w3.org/1999/02/22-rdf-syntax-ns#> .
@prefix dcterms: <http://purl.org/dc/terms/> .
@prefix owl:     <http://www.w3.org/2002/07/owl#> .
@prefix rdfs:    <http://www.w3.org/2000/01/rdf-schema#> .

<http://parliament.uk/ontologies/written-question-and-answer/> 
    rdf:type owl:Ontology ;
    dcterms:title "Written question and answer ontology"@en ;
    dcterms:created "10/10/2016"^^xsd:date ;
	dcterms:rights "Open Parliament Licence v3.0"@en ;
    dcterms:description "Written question and answer ontology for UK Parliament. This model only deals with questions that have been successfully tabled."@en .


#######  Classes ##### 	

pwqa:Member rdf:type owl:Class ;
	rdfs:label "Member"@en ;
	rdfs:comment "A current or former member of a house."@en ;
	rdf:isDefinedBy <http://parliament.uk/ontologies/written-question-and-answer/> .
	
pwqa:WrittenQuestion rdf:type owl:Class ;
	rdfs:label "WrittenQuestion"@en ;
	rdfs:comment "A type of Parliamentary question to which a written answer is expected. Written questions allow members to ask for information on the work, policy and activities of answering bodies. Usually this is to a minister in a government department but sometimes questions can be asked of non-departmental bodies. e.g. Church Commissioners."@en ;
	rdf:isDefinedBy <http://parliament.uk/ontologies/written-question-and-answer/> .
	
pwqa:WrittenAnswer rdf:type owl:Class ;
    rdfs:subClassOf pwqa:PursuableThing ;
	rdfs:label "WrittenAnswer"@en ;
	rdfs:comment "An answer to a written question, provided by an answering body."@en ;
	rdf:isDefinedBy <http://parliament.uk/ontologies/written-question-and-answer/> .
	
pwqa:AnsweringBody rdf:type owl:Class ;
	rdfs:label "AnsweringBody"@en ;
	rdfs:comment "A body to whom members can table written questions. May be a government department but sometimes other bodies either Parliamentary or external to Parliament. e.g. House of Commons Commission, Church Commissioners."@en ;
	rdf:isDefinedBy <http://parliament.uk/ontologies/written-question-and-answer/> .
	
pwqa:AllocatedAnsweringBody rdf:type owl:Class ;
	rdfs:label "AllocatedAnsweringBody"@en ;
	rdfs:comment "The answering body allocated to a question, either at tabling or in the event of the question being transferred. Note that the allocated answering body can change over time when one answering body transfers responsibility to another answering body. So allocated answering bodies are time bound. This would use startAt and endAt properties from the Core ontology."@en ;
	rdf:isDefinedBy <http://parliament.uk/ontologies/written-question-and-answer/> .
	
pwqa:Transferral rdf:type owl:Class ;
	rdfs:label "Transferral"@en ;
	rdfs:comment "The act of one answering body transferring responsibility for answering a question to another answering body."@en ;
	rdf:isDefinedBy <http://parliament.uk/ontologies/written-question-and-answer/> .
	
pwqa:PursuableThing rdf:type owl:Class ;
	rdfs:label "PursuableThing"@en ;
	rdfs:comment "A piece of Parliamentary business cited in a question. The question is asked as a follow up to the pursuable thing. e.g. in pursuant to a written or oral answer, a ministerial statement."@en ;
	rdf:isDefinedBy <http://parliament.uk/ontologies/written-question-and-answer/> .
	
pwqa:QuestionStatus rdf:type owl:Class ;
	rdfs:label "QuestionStatus"@en ;
	rdfs:comment "The current status of a question. May be active, withdrawn or no longer expecting an answer. Active in this case covers questions awaiting an answer and questions that have already been answered."@en ;
	rdf:isDefinedBy <http://parliament.uk/ontologies/written-question-and-answer/> .
	
pwqa:AnswerType rdf:type owl:Class ;
	rdfs:label "AnswerType"@en ;
	rdfs:comment "The type of a given answer e.g. holding answer, current answer or corrected answer. If a question is asked toward the end of a session, and Parliament is prorogued before it can be answered, a prorogation answer may be provided. The answer will state that there was not time to answer the question before prorogation."@en ;
	rdf:isDefinedBy <http://parliament.uk/ontologies/written-question-and-answer/> .
	
pwqa:DelegatedAnswer rdf:type owl:Class ;
	rdfs:label "DelegatedAnswer"@en ;
	rdfs:comment "Part of a written answer provided by an arm's length body rather than an answering body e.g. a government department might ask the UK Statistics Authority to provide part or all of an written answer."@en ;
	rdf:isDefinedBy <http://parliament.uk/ontologies/written-question-and-answer/> .
	
pwqa:ArmsLengthBody rdf:type owl:Class ;
	rdfs:label "ArmsLengthBody"@en ;
	rdfs:comment "An organisation operating at arm's length from the government e.g. UK Statistics Authority."@en ;
	rdf:isDefinedBy <http://parliament.uk/ontologies/written-question-and-answer/> .
	
pwqa:LibraryDeposit rdf:type owl:Class ;
	rdfs:label "LibraryDeposit"@en ;
	rdfs:comment "A paper or set of papers placed by a minister or the speaker in the library of either House. Usually deposits are made into both libraries but sometimes only one."@en ;
	rdf:isDefinedBy <http://parliament.uk/ontologies/written-question-and-answer/> .
	
pwqa:Document rdf:type owl:Class ;
	rdfs:label "Document"@en ;
	rdfs:comment "A document."@en ;
	rdf:isDefinedBy <http://parliament.uk/ontologies/written-question-and-answer/> .


#######  Object properties ##### 

pwqa:allocation rdf:type owl:ObjectProperty ;
	rdfs:label "allocation"@en ;
	rdfs:comment "Allows a question to be assigned to one or more answering bodies. A question intended for multiple answering bodies is sometimes referred to as a round robin question. Note that this is a major change from existing data models where the same question, when asked of different answering bodies, have been considered to be different questions."@en ;
	rdfs:domain pwqa:WrittenQuestion ;
	rdfs:range pwqa:AllocatedAnsweringBody ;
	rdf:isDefinedBy <http://parliament.uk/ontologies/written-question-and-answer/> .

pwqa:allocatedTo rdf:type owl:ObjectProperty ;
	rdfs:label "allocatedTo"@en ;
	rdfs:comment "Allows an allocation at a point in time to an answering body."@en ;
	rdfs:domain pwqa:AllocatedAnsweringBody ;
	rdfs:range pwqa:AnsweringBody ;
	rdf:isDefinedBy <http://parliament.uk/ontologies/written-question-and-answer/> .

pwqa:transferredFrom rdf:type owl:ObjectProperty ;
	rdfs:label "transferredFrom"@en ;
	rdfs:comment "Allows a transferral to specify the answering body to which the written question was formerly allocated."@en ;
	rdfs:domain pwqa:Transferral ;
	rdfs:range pwqa:AllocatedAnsweringBody ;
	rdf:isDefinedBy <http://parliament.uk/ontologies/written-question-and-answer/> .

pwqa:transferredTo rdf:type owl:ObjectProperty ;
	rdfs:label "transferredTo"@en ;
	rdfs:comment "Allows a transferral to specify the answering body to which the written question is subsequently allocated."@en ;
	rdfs:domain pwqa:Transferral ;
	rdfs:range pwqa:AllocatedAnsweringBody ;
	rdf:isDefinedBy <http://parliament.uk/ontologies/written-question-and-answer/> .

pwqa:answerTo rdf:type owl:ObjectProperty ;
	rdfs:label "answerTo"@en ;
	rdfs:comment "Allows a written answer to be associated with one or more written questions. This replicates more precisely the current functionality around grouped questions. In other words, a group of questions in receipt of the same answer. There is some debate as to whether the same text given in answer to questions from multiple members can be considered one, or the same, answer. This also allows a single question to have many answers. Sometimes multiple answers from a single answering body (e.g. holding answer, current answer, correction). Sometimes different answers from different answering bodies to the same question e.g. answers to a round robin question. Note that this is a major change to current data models, where a single question can have one and only one answer, and a single answer can be to one and only one question."@en ;
	rdfs:domain pwqa:WrittenAnswer ;
	rdfs:range pwqa:WrittenQuestion ;
	rdf:isDefinedBy <http://parliament.uk/ontologies/written-question-and-answer/> .
	
pwqa:answeringBody rdf:type owl:ObjectProperty ;
	rdfs:label "answeringBody"@en ;
	rdfs:comment "Relates a written answer to the answering body that provided it. A single answer can only be provided by one answering body."@en ;
	rdfs:domain pwqa:WrittenAnswer ;
	rdfs:range pwqa:AnsweringBody ;
	rdf:isDefinedBy <http://parliament.uk/ontologies/written-question-and-answer/> .
	
pwqa:hasQuestionStatus rdf:type owl:ObjectProperty ;
	rdfs:label "hasQuestionStatus"@en ;
	rdfs:comment "Relates a written question to its current question status."@en ;
	rdfs:domain pwqa:WrittenQuestion ;
	rdfs:range pwqa:QuestionStatus ;
	rdf:isDefinedBy <http://parliament.uk/ontologies/written-question-and-answer/> .
	
pwqa:tables rdf:type owl:ObjectProperty ;
	rdfs:label "tables"@en ;
	rdfs:comment "Relates a member to a question they have tabled."@en ;
	rdfs:domain pwqa:Member ;
	rdfs:range pwqa:WrittenQuestion ;
	rdf:isDefinedBy <http://parliament.uk/ontologies/written-question-and-answer/> .
	
pwqa:inPursuantTo rdf:type owl:ObjectProperty ;
	rdfs:label "inPursuantTo"@en ;
	rdfs:comment "Relates a written question to a piece of Parliamentary business cited by the question."@en ;
	rdfs:domain pwqa:WrittenQuestion ;
	rdfs:range pwqa:PursuableThing ;
	rdf:isDefinedBy <http://parliament.uk/ontologies/written-question-and-answer/> .
	
pwqa:answeringMember rdf:type owl:ObjectProperty ;
	rdfs:label "answeringMember"@en ;
	rdfs:comment "Relates a written answer to the member who provided it. In practice this will be a minister in a government department or a person occupying a government position in a non-departmental answering body."@en ;
	rdfs:domain pwqa:WrittenAnswer ;
	rdfs:range pwqa:Member ;
	rdf:isDefinedBy <http://parliament.uk/ontologies/written-question-and-answer/> .
	
pwqa:hasAnswerType rdf:type owl:ObjectProperty ;
	rdfs:label "hasAnswerType"@en ;
	rdfs:comment "Relates a written answer to its type i.e. a holding answer, current answer or correction."@en ;
	rdfs:domain pwqa:WrittenAnswer ;
	rdfs:range pwqa:AnswerType ;
	rdf:isDefinedBy <http://parliament.uk/ontologies/written-question-and-answer/> .
	
pwqa:previousAnswer rdf:type owl:ObjectProperty ;
	rdfs:label "previousAnswer"@en ;
	rdfs:comment "Relates a written answer to a previous answer that answers the question in whole or in part. e.g. I refer the honourable X to the answer given..."@en ;
	rdfs:domain pwqa:WrittenAnswer ;
	rdfs:range pwqa:AnswerType ;
	rdf:isDefinedBy <http://parliament.uk/ontologies/written-question-and-answer/> .
	
pwqa:delegatedAnswer rdf:type owl:ObjectProperty ;
	rdfs:label "delegatedAnswer"@en ;
	rdfs:comment "Relates a written answer to a delegated answer provided by an arms length body. The delegated answer may provide part or all of the full answer."@en ;
	rdfs:domain pwqa:WrittenAnswer ;
	rdfs:range pwqa:DelegatedAnswer ;
	rdf:isDefinedBy <http://parliament.uk/ontologies/written-question-and-answer/> .
	
pwqa:delegatedTo rdf:type owl:ObjectProperty ;
	rdfs:label "delegatedTo"@en ;
	rdfs:comment "Relates a delegated answer to the arm's length body that provided it."@en ;
	rdfs:domain pwqa:DelegatedAnswer ;
	rdfs:range pwqa:ArmsLengthBody ;
	rdf:isDefinedBy <http://parliament.uk/ontologies/written-question-and-answer/> .
	
pwqa:refersToLibraryDeposit rdf:type owl:ObjectProperty ;
	rdfs:label "refersToLibraryDeposit"@en ;
	rdfs:comment "Relates a delegated answer a library deposit i.e. the answer to a question may undertake to deposit papers in the libraries of either House."@en ;
	rdfs:domain pwqa:WrittenAnswer ;
	rdfs:range pwqa:LibraryDeposit ;
	rdf:isDefinedBy <http://parliament.uk/ontologies/written-question-and-answer/> .
	
pwqa:refersToDocument rdf:type owl:ObjectProperty ;
	rdfs:label "refersToLibraryDeposit"@en ;
	rdfs:comment "Relates a written answer to a document provided as an attachment to the answer text. The document might form part or all of the answer."@en ;
	rdfs:domain pwqa:WrittenQuestion ;
	rdfs:range xsd:dateTime ;
	rdf:isDefinedBy <http://parliament.uk/ontologies/written-question-and-answer/> .
	
pwqa:refersToDocument rdf:type owl:ObjectProperty ;
	rdfs:label "refersToLibraryDeposit"@en ;
	rdfs:comment "Relates a written answer to a document. The document might form part or all of the answer."@en ;
	rdfs:domain pwqa:WrittenQuestion ;
	rdfs:range xsd:dateTime ;
	rdf:isDefinedBy <http://parliament.uk/ontologies/written-question-and-answer/> .
		

#######  Data properties ##### 


pwqa:tabledAt rdf:type owl:DatatypeProperty ;
	rdfs:label "tabledAt"@en ;
	rdfs:comment "Relates a written question to the date time it was tabled at."@en ;
	rdfs:domain pwqa:WrittenQuestion ;
	rdfs:range xsd:dateTime ;
	rdf:isDefinedBy <http://parliament.uk/ontologies/written-question-and-answer/> .
	
pwqa:namedDateForAnswer rdf:type owl:DatatypeProperty ;
	rdfs:label "namedDateForAnswer"@en ;
	rdfs:comment "Relates a written question to a named day. The member tabling the question has requested that it be answered by the named day. Note that named day questions can only be tabled in the House of Commons. Most written questions are 'ordinary'. By convention a member can expect such questions to be answered within 7 days of tabling. Named day questions are used to elicit a faster response."@en ;
	rdfs:domain pwqa:WrittenQuestion ;
	rdfs:range xsd:date ;
	rdf:isDefinedBy <http://parliament.uk/ontologies/written-question-and-answer/> .
	
pwqa:heading rdf:type owl:DatatypeProperty ;
	rdfs:label "heading"@en ;
	rdfs:comment "Relates a written question to its heading text. This is supplied by the Indexing and Data Management Section in the House of Commons Library."@en ;
	rdfs:domain pwqa:WrittenQuestion ;
	rdfs:range rdf:langString ;
	rdf:isDefinedBy <http://parliament.uk/ontologies/written-question-and-answer/> .	
	
pwqa:templateText rdf:type owl:DatatypeProperty ;
	rdfs:label "templateText"@en ;
	rdfs:comment "Relates a written question to the template text that prefaces it. This is usually of the form, 'To ask the minister for etc.' and varies depending on the answering body."@en ;
	rdfs:domain pwqa:WrittenQuestion ;
	rdfs:range rdf:langString ;
	rdf:isDefinedBy <http://parliament.uk/ontologies/written-question-and-answer/> .	
	
pwqa:questionText rdf:type owl:DatatypeProperty ;
	rdfs:label "questionText"@en ;
	rdfs:comment "Relates a written question to the actual text of the question as asked by the member."@en ;
	rdfs:domain pwqa:WrittenQuestion ;
	rdfs:range rdf:langString ;
	rdf:isDefinedBy <http://parliament.uk/ontologies/written-question-and-answer/> .	