@prefix pbill: <http://parliament.uk/ontologies/bill/> . 
@prefix xsd: <http://www.w3.org/2001/XMLSchema#> . 
@prefix rdf: <http://www.w3.org/1999/02/22-rdf-syntax-ns#> .
@prefix dcterms: <http://purl.org/dc/terms/> .
@prefix owl:     <http://www.w3.org/2002/07/owl#> .
@prefix rdfs:    <http://www.w3.org/2000/01/rdf-schema#> .
@prefix skos: <http://www.w3.org/2004/02/skos/core#> .
@prefix foaf:	<http://xmlns.com/foaf/0.1/> .

<http://parliament.uk/ontologies/bill/> 
    rdf:type owl:Ontology ;
    dcterms:title "Bill ontology"@en ;
    dcterms:created "2019-06-10"^^xsd:date ;
	dcterms:rights "Open Parliament Licence v3.0"@en ;
    dcterms:description "A model describing the form of bills before Parliament."@en ;
	foaf:depiction <https://ukparliament.github.io/ontologies/agency/agency.svg> ;
	foaf:maker
	    [ foaf:name "Jayne Bosworth" ],
		[ foaf:name "Robert Brook"; foaf:homepage <https://robert-brook.com/> ],
		[ foaf:name "Graeme Cowie" ],
		[ foaf:name "Richard Kelly" ],
		[ foaf:name "Ned Morrell" ],
		[ foaf:name "Claire Searle" ],
		[ foaf:name "Michael Smethurst"; foaf:homepage <https://smethur.st/> ],
	    [ foaf:name "Anya Somerville" ].


#######  Classes ####
	
pbill:PaperExpression rdf:type owl:Class ;
	rdfs:label "Paper expression"@en ;
	rdfs:comment "A paper made available to a House, being an expression of a paper work."@en ;
	rdfs:isDefinedBy <http://parliament.uk/ontologies/bill/> .

pbill:PaperWork rdf:type owl:Class ;
	rdfs:label "Paper work"@en ;
	rdfs:comment "A paper as a single intellectual work, as defined in the Functional Requirements for Bibliographic Records specification."@en ;
	rdfs:isDefinedBy <http://parliament.uk/ontologies/bill/> .

pbill:BillExpression rdf:type owl:Class ;
	rdfs:subClassOf pbill:PaperExpression ;
	rdfs:label "Bill expression"@en ;
	rdfs:comment "An expression of a bill work at a point in time. A new expression of the bill work is created by any amendment being made to the bill, or when a bill passes from the first House to the second House."@en ;
	rdfs:isDefinedBy <http://parliament.uk/ontologies/bill/> .

pbill:BillWork rdf:type owl:Class ;
	rdfs:subClassOf pbill:PaperWork ;
	rdfs:label "Bill work"@en ;
	rdfs:comment "A proposal for a new Act of Parliament."@en ;
	rdfs:isDefinedBy <http://parliament.uk/ontologies/bill/> .

pbill:PublicBillWork rdf:type owl:Class ;
	rdfs:subClassOf pbill:BillWork ;
	rdfs:label "Public Bill work"@en ;
	rdfs:comment "A proposal for a new Act of Parliament with general application across the whole population, without that application being limited to particular groups, people or places. A Public Bill is either a Government Bill or a Private Members' Bill."@en ;
	rdfs:isDefinedBy <http://parliament.uk/ontologies/bill/> .
	
pbill:HybridBillWork rdf:type owl:Class ;
	rdfs:subClassOf pbill:PublicBillWork ;
	rdfs:label "Hybrid Bill work"@en ;
	rdfs:comment "A hybrid bill is a public bill, having general application across the whole population, whilst also having been examined by the Examiners of Petitions for Private Bills and found to differently affect the interests of particular groups, people or places. Hybrid bills are presented as public bills. If examined and found to be hybrid, they follow a procedure including parts of the private bill procedure."@en ;
	rdfs:isDefinedBy <http://parliament.uk/ontologies/bill/> .
	
pbill:PrivateBillWork rdf:type owl:Class ;
	rdfs:subClassOf pbill:BillWork ;
	rdfs:label "Private Bill work"@en ;
	rdfs:comment "A proposal for a new Act of Parliament affecting the interests of particular groups, people or places."@en ;
	rdfs:isDefinedBy <http://parliament.uk/ontologies/bill/> .

pbill:DraftBill rdf:type owl:Class ;
	rdfs:label "Draft Bill"@en ;
	rdfs:comment "A draft form of a Government bill issued before being introduced as a Public Bill to Parliament. A draft bill is available to be examined either by a Commons or Lords select committee, or by a joint committee of both Houses of Parliament created for that purpose."@en ;
	rdfs:isDefinedBy <http://parliament.uk/ontologies/bill/> .
	
pbill:ActOfParliament rdf:type owl:Class ;
	rdfs:label "Act of Parliament"@en ;
	rdfs:comment "An Act of Parliament creates, amends or repeals legislation. An Act is a Bill which has been passed by Parliament and given Royal Assent."@en ;
	rdfs:isDefinedBy <http://parliament.uk/ontologies/bill/> .

pbill:ParliamentActProcedureInvocation rdf:type owl:Class ;
	rdfs:label "Parliament Act procedure invocation"@en ;
	rdfs:comment "Where a Public Bill is passed by the House of Commons and rejected by the House of Lords in the same session, the Commons may introduce an identical bill - or a bill deemed to be the same bill as the former bill having alterations certified by the Speaker of the House of Commons as being necessary - in the following session, under procedure set out in the Parliament Act 1911. If the House of Lords reject the second bill, that bill may be put forward for Royal Assent if the Speaker of the Commons certifies that the bill meets the conditions set out in section 2 of the 1911 Act."@en ;
	rdfs:isDefinedBy <http://parliament.uk/ontologies/bill/> .
	
pbill:DepartmentalSponsorship rdf:type owl:Class ;
	rdfs:label "Departmental sponsorship"@en ;
	rdfs:comment "The sponsorship of a Public Bill by a Government department. If the machinery of Government changes during the passage of a bill, the sponsorship of that bill may pass to another Government department."@en ;
	rdfs:isDefinedBy <http://parliament.uk/ontologies/bill/> .
	
pbill:MinisterialDepartment rdf:type owl:Class ;
	rdfs:label "Ministerial department"@en ;
	rdfs:comment "A ministerial department is an executive body of government, headed by a government minister having responsibility for described areas of public administration."@en ;
	rdfs:isDefinedBy <http://parliament.uk/ontologies/bill/> .

pbill:MemberSponsorship rdf:type owl:Class ;
	rdfs:label "Member sponsorship"@en ;
	rdfs:comment "The sponsorship of a Public Bill by a Member. Sponsorship of a Public Bill may pass to another Member, for example: if a Member is elevated to the House of Lords."@en ;
	rdfs:isDefinedBy <http://parliament.uk/ontologies/bill/> .

pbill:Incumbency rdf:type owl:Class ;
	rdfs:label "Incumbency"@en ;
	rdfs:comment "The holding of a position by a person, including the time period for which this was the case. For example, Philip Hammond holding the position of Foreign Secretary between two dates."@en ;
	rdfs:isDefinedBy <http://parliament.uk/ontologies/bill/> .
	
pbill:House rdf:type owl:Class ;
	rdfs:label "House"@en ;
	rdfs:comment "A parliamentary House, for example: the House of Lords."@en ;
	rdfs:isDefinedBy <http://parliament.uk/ontologies/house-bill/> .
	


#######  Object properties ##### 
	
pbill:expressionOf rdf:type owl:ObjectProperty ;
	rdfs:label "Expression of"@en ;
	rdfs:comment "Relates a bill expression to the bill work it is an expression of. A bill expression is an expression of one bill work. A bill work is expressed as one or more expressions."@en ;
	rdfs:domain pbill:BillExpression ;
	rdfs:range pbill:BillWork ;
	rdfs:isDefinedBy <http://parliament.uk/ontologies/bill/> .

pbill:precededBy rdf:type owl:ObjectProperty ;
	rdfs:label "Preceded by"@en ;
	rdfs:comment "Relates a Public Bill to the Draft Bill which preceded it. A Public Bill may be preceded by one Draft Bill, or none. A Draft Bill may be followed by one Public Bill, or none."@en ;
	rdfs:domain pbill:PublicBillWork ;
	rdfs:range pbill:DraftBill ;
	rdfs:isDefinedBy <http://parliament.uk/ontologies/bill/> .
	
pbill:enactedAs rdf:type owl:ObjectProperty ;
	rdfs:label "Enacted as"@en ;
	rdfs:comment "Relates a bill work to the Act of Parliament the bill is enacted as after receiving Royal Assent. A bill is enacted as one Act, or none. An Act is the enactment of one bill."@en ;
	rdfs:domain pbill:BillWork ;
	rdfs:range pbill:ActOfParliament ;
	rdfs:isDefinedBy <http://parliament.uk/ontologies/bill/> .

pbill:parliamentActInvokedFrom rdf:type owl:ObjectProperty ;
	rdfs:label "Parliament Act invoked from"@en ;
	rdfs:comment "Relates an invocation of the Parliament Act 1911 and the Parliament Act 1949 to a Public Bill in the preceding session. An invocation of the Parliament Act 1911 is from one Public Bill."@en ;
	rdfs:domain pbill:ParliamentActProcedureInvocation ;
	rdfs:range pbill:PublicBillWork ;
	rdfs:isDefinedBy <http://parliament.uk/ontologies/bill/> .

pbill:parliamentActInvokedTo rdf:type owl:ObjectProperty ;
	rdfs:label "Parliament Act invoked to"@en ;
	rdfs:comment "Relates an invocation of the Parliament Act 1911 and the Parliament Act 1949 to a Public Bill in the following session. An invocation of the Parliament Act 1911 is to one Public Bill."@en ;
	rdfs:domain pbill:ParliamentActProcedureInvocation ;
	rdfs:range pbill:PublicBillWork ;
	rdfs:isDefinedBy <http://parliament.uk/ontologies/bill/> .
	
pbill:departmentalSponsorshipOfPublicBill rdf:type owl:ObjectProperty ;
	rdfs:label "Departmental sponsorship of Public Bill"@en ;
	rdfs:comment "Relates a sponsorship by a Government department to a Public Bill at a point in time. A government bill has one or more departmental sponsorships over time. A Private Members' Bill has no departmental sponsorships."@en ;
	rdfs:domain pbill:DepartmentalSponsorship ;
	rdfs:range pbill:PublicBillWork ;
	rdfs:isDefinedBy <http://parliament.uk/ontologies/bill/> .
	
pbill:memberSponsorshipOfPublicBill rdf:type owl:ObjectProperty ;
	rdfs:label "Member sponsorship of Public Bill"@en ;
	rdfs:comment "Relates a sponsorship of a Public Bill by a Member at a point in time to the bill being sponsored. A Public Bill may have one or more Member sponsorships over time."@en ;
	rdfs:domain pbill:MemberSponsorship ;
	rdfs:range pbill:PublicBillWork ;
	rdfs:isDefinedBy <http://parliament.uk/ontologies/bill/> .
	
pbill:sponsorshipByGovernmentDepartment rdf:type owl:ObjectProperty ;
	rdfs:label "Sponsorship by government department"@en ;
	rdfs:comment "Relates a departmental sponsorship to the Ministerial Department sponsoring a Public Bill at a point in time. A departmental sponsorship is by one Ministerial Department."@en ;
	rdfs:domain pbill:DepartmentalSponsorship ;
	rdfs:range pbill:MinisterialDepartment ;
	rdfs:isDefinedBy <http://parliament.uk/ontologies/bill/> .
	
pbill:sponsorshipByIncumbency rdf:type owl:ObjectProperty ;
	rdfs:label "Sponsorship by incumbency"@en ;
	rdfs:comment "Relates a Member sponsorship to the incumbency of a Member sponsoring a Public Bill at a point in time. For a Private Members’ Bill, the incumbency is a seat incumbency. For a Government Bill, the incumbency is an incumbency in a Government position. A sponsorship by incumbency is by one incumbency."@en ;
	rdfs:domain pbill:MemberSponsorship ;
	rdfs:range pbill:Incumbency ;
	rdfs:isDefinedBy <http://parliament.uk/ontologies/bill/> .
	
pbill:inHouse rdf:type owl:ObjectProperty ;
	rdfs:label "In House"@en ;
	rdfs:comment "Relates a Member sponsorship to the House that sponsorship is in. A Member sponsorship is in one House."@en ;
	rdfs:domain pbill:MemberSponsorship ;
	rdfs:range pbill:House ;
	rdfs:isDefinedBy <http://parliament.uk/ontologies/bill/> .



#######  Data properties #####
	
pbill:longTitle rdf:type owl:DatatypeProperty ;
	rdfs:label "Long title"@en ;
	rdfs:comment "The long title of a Bill is the wording at the start of a Bill that begins 'A Bill to ...', followed by text describing the purposes of the Bill."@en ;
	rdfs:domain pbill:BillExpression ;
	rdfs:range rdf:langString ;
	rdfs:isDefinedBy <http://parliament.uk/ontologies/bill/> .
