@prefix pbill: <http://parliament.uk/ontologies/bill/> . 
@prefix xsd: <http://www.w3.org/2001/XMLSchema#> . 
@prefix rdf: <http://www.w3.org/1999/02/22-rdf-syntax-ns#> .
@prefix dcterms: <http://purl.org/dc/terms/> .
@prefix owl:     <http://www.w3.org/2002/07/owl#> .
@prefix rdfs:    <http://www.w3.org/2000/01/rdf-schema#> .
@prefix skos: <http://www.w3.org/2004/02/skos/core#> .
@prefix foaf:	<http://xmlns.com/foaf/0.1/> .

<http://parliament.uk/ontologies/bill/> 
    rdf:type owl:Ontology ;
    dcterms:title "Bill ontology"@en ;
    dcterms:created "2019-06-10"^^xsd:date ;
	dcterms:rights "Open Parliament Licence v3.0"@en ;
    dcterms:description "A model describing the form of bills before Parliament."@en ;
	foaf:depiction <https://ukparliament.github.io/ontologies/agency/agency.svg> ;
	foaf:maker
	    [ foaf:name "Jayne Bosworth" ],
		[ foaf:name "Robert Brook"; foaf:homepage <https://robert-brook.com/> ],
		[ foaf:name "Graeme Cowie" ],
		[ foaf:name "Richard Kelly" ],
		[ foaf:name "Ned Morrell" ],
		[ foaf:name "Claire Searle" ],
		[ foaf:name "Michael Smethurst"; foaf:homepage <https://smethur.st/> ],
	    [ foaf:name "Anya Somerville" ].


#######  Classes #####

pbill:BillExpression rdf:type owl:Class ;
	rdfs:label "Bill expression"@en ;
	rdfs:comment ""@en ;
	rdfs:isDefinedBy <http://parliament.uk/ontologies/bill/> .

pbill:BillWork rdf:type owl:Class ;
	rdfs:label "Bill work"@en ;
	rdfs:comment "A proposal for a new Act of Parliament."@en ;
	rdfs:isDefinedBy <http://parliament.uk/ontologies/bill/> .

pbill:PublicBillWork rdf:type owl:Class ;
	rdfs:subClassOf pbill:BillWork ;
	rdfs:label "Public Bill work"@en ;
	rdfs:comment "A proposal for a new Act of Parliament with general application across the whole population, without that application being limited to particular groups, people or places. A Public Bill is either a Government Bill or a Private Members' Bill."@en ;
	rdfs:isDefinedBy <http://parliament.uk/ontologies/bill/> .
	
pbill:HybridBillWork rdf:type owl:Class ;
	rdfs:subClassOf pbill:PublicBillWork ;
	rdfs:label "Hybrid Bill work"@en ;
	rdfs:comment "A hybrid bill is a public bill having general application across the whole population, whilst also having been examined and found to differently affect the interests of particular groups, people or places. Hybrid bills are presented as public bills. If examined and found to be hybrid, they follow a procedure including parts of the private bill procedure."@en ;
	rdfs:isDefinedBy <http://parliament.uk/ontologies/bill/> .
	
pbill:PrivateBillWork rdf:type owl:Class ;
	rdfs:subClassOf pbill:BillWork ;
	rdfs:label "Private Bill work"@en ;
	rdfs:comment "A proposal for a new Act of Parliament differently affecting the interests of particular groups, people or places."@en ;
	rdfs:isDefinedBy <http://parliament.uk/ontologies/bill/> .

pbill:DraftBill rdf:type owl:Class ;
	rdfs:label "Draft Bill"@en ;
	rdfs:comment "A draft form of a Government bill issued before being introduced as a Public Bill to Parliament. A draft bill is available to be examined either by a Commons or Lords select committee, or by a joint committee of both Houses of Parliament created for that purpose. This process of examining the draft bill is known as 'pre-legislative scrutiny'"@en ;
	rdfs:isDefinedBy <http://parliament.uk/ontologies/bill/> .
	
pbill:ActOfParliament rdf:type owl:Class ;
	rdfs:label "Act of Parliament"@en ;
	rdfs:comment "An Act of Parliament creates, amends or repeals legislation. An Act is a Bill having been passed by Parliament and been given Royal Assent. Acts of Parliament which are in force comprise statute law."@en ;
	rdfs:isDefinedBy <http://parliament.uk/ontologies/bill/> .

pbill:CarryOver rdf:type owl:Class ;
	rdfs:label "Carry over"@en ;
	rdfs:comment "The act of carrying a bill over from a session to the following session. A bill being carried over results in the creation of a new bill in the new session, the text of the new bill being the text of the original bill as amended in the previous session. Public Bills which have not been passed by the end of the session in which they were introduced will otherwise fall. A bill being before the House of Commons, it is necessary for that House to pass a carry over motion in order for the bill to be carried over into the following session. Private Members' Bills cannot be carried over."@en ;
	rdfs:isDefinedBy <http://parliament.uk/ontologies/bill/> .

pbill:ParliamentActProcedureInvocation rdf:type owl:Class ;
	rdfs:label "Parliament Act procedure invocation"@en ;
	rdfs:comment "The Parliament Acts of 1911 and 1949 limit the power of the House of Lords in relation to the House of Commons. The Acts removed the rights of the Lords to pass bills on public tax and spending, to veto or to indefinitely delay the progress of Public Bills. Where a bill is passed by the House of Commons and rejected by the House of Lords in the same session, the Government may introduce a similar bill in the following session. If the House of Commons invokes the Parliament Act, the House of Lords has one month to agree to the bill, otherwise the Commons may pass the bill unilaterally. The similarity of a bill being introduced in a following session is not made explicit until the Speaker certifies the bill as being subject to the Parliament Act."@en ;
	rdfs:isDefinedBy <http://parliament.uk/ontologies/bill/> .
	
pbill:DepartmentalSponsorship rdf:type owl:Class ;
	rdfs:label "Departmental sponsorship"@en ;
	rdfs:comment "The sponsorship of a Public Bill by a Government organisation. If the machinery of Government changes during the passage of a bill, it is possible for the sponsorship of that bill to pass to a different Government organisation."@en ;
	rdfs:isDefinedBy <http://parliament.uk/ontologies/bill/> .
	
pbill:GovernmentOrganisation rdf:type owl:Class ;
	rdfs:label "Government Organisation"@en ;
	rdfs:comment "Government departments, agencies and public bodies which have responsibility for a specific sector of public administration."@en ;
	rdfs:isDefinedBy <http://parliament.uk/ontologies/bill/> .

pbill:MemberSponsorship rdf:type owl:Class ;
	rdfs:label "Member sponsorship"@en ;
	rdfs:comment "The sponsorship of a Public Bill by a Member. It is possible for the sponsorship of a Public Bill to pass to a different Member, for example: if a Member is elevated to the House of Lords."@en ;
	rdfs:isDefinedBy <http://parliament.uk/ontologies/bill/> .
	
pbill:MemberLeadership rdf:type owl:Class ;
	rdfs:label "Member leadership"@en ;
	rdfs:comment "The leadership of a Public Bill by a Member. It is possible for the leadership of a Public Bill to pass to a different Member, for example: if a Member is elevated to the House of Lords."@en ;
	rdfs:isDefinedBy <http://parliament.uk/ontologies/bill/> .

pbill:Incumbency rdf:type owl:Class ;
	rdfs:label "Incumbency"@en ;
	rdfs:comment "The holding of a position by a person, including the time period for which this was the case. For example, Philip Hammond holding the position of Foreign Secretary between two dates."@en ;
	rdfs:isDefinedBy <http://parliament.uk/ontologies/bill/> .
	
pbill:LawCommissionBillWork rdf:type owl:Class ;
	rdfs:subClassOf pbill:PublicBillWork ;
	rdfs:label "Law Commission bill work"@en ;
	rdfs:comment ""@en ;
	rdfs:isDefinedBy <http://parliament.uk/ontologies/bill/> .
	
pbill:ConsolidationBillWork rdf:type owl:Class ;
	rdfs:subClassOf pbill:PublicBillWork ;
	rdfs:label "Consolidation bill work"@en ;
	rdfs:comment ""@en ;
	rdfs:isDefinedBy <http://parliament.uk/ontologies/bill/> .



#######  Object properties ##### 
	
pbill:ExpressionOf rdf:type owl:ObjectProperty ;
	rdfs:label "Expression of"@en ;
	rdfs:comment ""@en ;
	rdfs:domain pbill:BillExpression ;
	rdfs:range pbill:BillWork ;
	rdfs:isDefinedBy <http://parliament.uk/ontologies/bill/> .

pbill:precededBy rdf:type owl:ObjectProperty ;
	rdfs:label "Preceded by"@en ;
	rdfs:comment "Relates a Public Bill to the Draft Bill which preceded it. A Public Bill may be preceded by one Draft Bill, or none. A Draft Bill may be followed by one Public Bill, or none."@en ;
	rdfs:domain pbill:PublicBillWork ;
	rdfs:range pbill:DraftBill ;
	rdfs:isDefinedBy <http://parliament.uk/ontologies/bill/> .
	
pbill:enactedAs rdf:type owl:ObjectProperty ;
	rdfs:label "Enacted as"@en ;
	rdfs:comment "Relates a bill to the Act of Parliament the bill is enacted as after receiving Royal Assent."@en ;
	rdfs:domain pbill:BillWork ;
	rdfs:range pbill:ActOfParliament ;
	rdfs:isDefinedBy <http://parliament.uk/ontologies/bill/> .
	
pbill:carriedOverFrom rdf:type owl:ObjectProperty ;
	rdfs:label "Carried over from"@en ;
	rdfs:comment "Relates the act of being carried over to the bill in the preceding session."@en ;
	rdfs:domain pbill:CarryOver ;
	rdfs:range pbill:BillWork ;
	rdfs:isDefinedBy <http://parliament.uk/ontologies/bill/> .
	
pbill:carriedOverTo rdf:type owl:ObjectProperty ;
	rdfs:label "Carried over to"@en ;
	rdfs:comment "Relates the act of being carried over to the bill in the new session."@en ;
	rdfs:domain pbill:CarryOver ;
	rdfs:range pbill:BillWork ;
	rdfs:isDefinedBy <http://parliament.uk/ontologies/bill/> .
	
pbill:parliamentActInvokedFrom rdf:type owl:ObjectProperty ;
	rdfs:label "Parliament Act invoked from"@en ;
	rdfs:comment "Relates an invocation of the Parliament Act to a Public Bill in the preceding session."@en ;
	rdfs:domain pbill:ParliamentActProcedureInvocation ;
	rdfs:range pbill:PublicBillWork ;
	rdfs:isDefinedBy <http://parliament.uk/ontologies/bill/> .

pbill:parliamentActInvokedTo rdf:type owl:ObjectProperty ;
	rdfs:label "Parliament Act invoked to"@en ;
	rdfs:comment "Relates an invocation of the Parliament Act to a Public Bill in the new session."@en ;
	rdfs:domain pbill:ParliamentActProcedureInvocation ;
	rdfs:range pbill:PublicBillWork ;
	rdfs:isDefinedBy <http://parliament.uk/ontologies/bill/> .
	
pbill:hasDepartmentalSponsorship rdf:type owl:ObjectProperty ;
	rdfs:label "Has departmental sponsorship"@en ;
	rdfs:comment "Relates a Public Bill to a sponsorship by a Government department at a point in time. A Public Bill may have one or more departmental sponsorships over time, or none in the case of a Private Members' Bill."@en ;
	rdfs:domain pbill:PublicBillWork ;
	rdfs:range pbill:DepartmentalSponsorship ;
	rdfs:isDefinedBy <http://parliament.uk/ontologies/bill/> .
	
pbill:hasMemberSponsorship rdf:type owl:ObjectProperty ;
	rdfs:label "Has Member sponsorship"@en ;
	rdfs:comment "Relates a Public Bill to a sponsorship by a Member at a point in time. A Public Bill may have one or more Member sponsorships over time, or none in the case of a Government Bill."@en ;
	rdfs:domain pbill:PublicBillWork ;
	rdfs:range pbill:MemberSponsorship ;
	rdfs:isDefinedBy <http://parliament.uk/ontologies/bill/> .
	
pbill:hasMemberLeadership rdf:type owl:ObjectProperty ;
	rdfs:label "Has Member leadership"@en ;
	rdfs:comment "Relates a Public Bill to a leadership by a Member at a point in time. A Public Bill may have one or more leading Members, or none in the case of a Private Members' Bill."@en ;
	rdfs:domain pbill:PublicBillWork ;
	rdfs:range pbill:MemberLeadership ;
	rdfs:isDefinedBy <http://parliament.uk/ontologies/bill/> .
	
pbill:sponsorshipByGovernmentOrganisation rdf:type owl:ObjectProperty ;
	rdfs:label "Sponsorship by government organisation"@en ;
	rdfs:comment "Relates a departmental sponsorship to the Government organisation sponsoring a Public Bill at a point in time."@en ;
	rdfs:domain pbill:DepartmentalSponsorship ;
	rdfs:range pbill:GovernmentOrganisation ;
	rdfs:isDefinedBy <http://parliament.uk/ontologies/bill/> .
	
pbill:sponsorshipByIncumbency rdf:type owl:ObjectProperty ;
	rdfs:label "Sponsorship by incumbency"@en ;
	rdfs:comment "Relates a Member sponsorship to the House seat incumbency of a Member sponsoring a Public Bill at a point in time."@en ;
	rdfs:domain pbill:MemberSponsorship ;
	rdfs:range pbill:Incumbency ;
	rdfs:isDefinedBy <http://parliament.uk/ontologies/bill/> .
	
pbill:leadershipByIncumbency rdf:type owl:ObjectProperty ;
	rdfs:label "Leadership by incumbency"@en ;
	rdfs:comment "Relates a Member leadership to the incumbency of a Member in a Government position leading a Public Bill at a point in time."@en ;
	rdfs:domain pbill:MemberLeadership ;
	rdfs:range pbill:Incumbency ;
	rdfs:isDefinedBy <http://parliament.uk/ontologies/bill/> .



#######  Data properties ##### 

pma:prefix rdf:type owl:DatatypeProperty ;
	rdfs:label "Prefix"@en ;
	rdfs:comment ""@en ;
	rdfs:domain pma:BillExpression ;
	rdfs:range rdfs:Literal ;
	rdfs:isDefinedBy <http://parliament.uk/ontologies/making-available/> .
	
pma:number rdf:type owl:DatatypeProperty ;
	rdfs:label "Number"@en ;
	rdfs:comment ""@en ;
	rdfs:domain pma:BillExpression ;
	rdfs:range xsd:integer ;
	rdfs:isDefinedBy <http://parliament.uk/ontologies/making-available/> .
	
pma:longTitle rdf:type owl:DatatypeProperty ;
	rdfs:label "Long title"@en ;
	rdfs:comment ""@en ;
	rdfs:domain pma:BillWork ;
	rdfs:range rdf:langString ;
	rdfs:isDefinedBy <http://parliament.uk/ontologies/making-available/> .
