@prefix pe: <http://parliament.uk/ontologies/election/> . 
@prefix xsd: <http://www.w3.org/2001/XMLSchema#> . 
@prefix rdf: <http://www.w3.org/1999/02/22-rdf-syntax-ns#> .
@prefix dcterms: <http://purl.org/dc/terms/> .
@prefix owl:     <http://www.w3.org/2002/07/owl#> .
@prefix rdfs:    <http://www.w3.org/2000/01/rdf-schema#> .
@prefix foaf:	<http://xmlns.com/foaf/0.1/> .

<http://parliament.uk/ontologies/election/> 
    rdf:type owl:Ontology ;
    dcterms:title "Election ontology"@en ;
    dcterms:created "2016-10-06"^^xsd:date ;
	dcterms:rights "Open Parliament Licence v3.0"@en ;
    dcterms:description "A model describing incumbencies resulting from general elections, by-elections for seats in the House of Commons, by-elections for excepted hereditary peers in the House of Lords and elections for positions including that of the Speaker of the House of Commons. The model describes the result of an election regardless of the process by which that election has been conducted, and covers election returns by the 'first past the post' system and those which follow other methods. Where applicable, the model is aligned with the Cabinet Office Election Result Data Standard."@en ;
	foaf:depiction  <https://ukparliament.github.io/ontologies/election/election.svg> ;
	foaf:maker
		[ foaf:name "Robert Brook"; foaf:homepage <https://robert-brook.com/> ],
		[ foaf:name "Oli Hawkins"; foaf:homepage <https://olihawkins.com/> ],
		[ foaf:name "Ned Morrell" ],
		[ foaf:name "Sym Roe"; foaf:homepage <http://symroe.co.uk/> ],
		[ foaf:name "Michael Smethurst"; foaf:homepage <http://smethur.st/> ],
	    [ foaf:name "Anya Somerville" ].
	


#######  Classes #####

pe:Election rdf:type owl:Class ;
	rdfs:label "Election"@en ;
	rdfs:comment "An election to elect a candidate or candidates to a seat or position."@en ;
	rdfs:isDefinedBy <http://parliament.uk/ontologies/election/> .
	
pe:ParliamentPeriod rdf:type owl:Class ;
	rdfs:label "Parliament period"@en ;
	rdfs:comment "The time period of a single Parliament between the date of its first assembly after a general election and its dissolution. A Parliament period contains contiguous session and prorogation periods. During a parliament period Parliament is either in session or prorogued. The start date of a Parliament may be changed by subsequent proclamations. A Parliament ends at the next dissolution. While the Fixed-term Parliaments Act 2011 was in force, the date of dissolution was determined by that Act or was named in a proclamation following a vote in Parliament for an early general election. The next Parliament began on the date named in the proclamation issued following a dissolution. Before the Fixed-term Parliaments Act 2011 came into force and after that Act was repealed by the Dissolution and Calling of Parliament Act 2022, the date of dissolution is fixed by proclamation. The dissolution proclamation also names the date for Parliament to reassemble. Parliament periods are the same across both Houses. Parliaments are numbered ordinally from the first Parliament of the United Kingdom, sitting in 1801."@en ;
	rdfs:isDefinedBy <http://parliament.uk/ontologies/election/> .
	
pe:GeneralElection rdf:type owl:Class ;
	rdfs:label "General election"@en ;
	rdfs:comment "A set of elections to seats in the House of Commons held in all constituencies concurrently."@en ;
	rdfs:isDefinedBy <http://parliament.uk/ontologies/election/> .

pe:Population rdf:type owl:Class ;
	rdfs:label "Population"@en ;
	rdfs:comment "A set of people."@en ;
	rdfs:isDefinedBy <http://parliament.uk/ontologies/election/> .
	
pe:PopulationSize rdf:type owl:Class ;
	rdfs:label "Population size"@en ;
	rdfs:comment "The recording of the size of a population on a date."@en ;
	rdfs:isDefinedBy <http://parliament.uk/ontologies/election/> .

pe:Electorate rdf:type owl:Class ;
	rdfs:subClassOf pe:Population ;
	rdfs:label "Electorate"@en ;
	rdfs:comment "A group of people who are eligible to vote in an election called at a particular time, for example: the group of people entitled to vote in a constituency election, or members of the House of Commons voting for their Speaker."@en ;
	rdfs:isDefinedBy <http://parliament.uk/ontologies/election/> .
	
pe:ConstituencyGroup rdf:type owl:Class ;
	rdfs:subClassOf pe:Population ;
	rdfs:label "Constituency group"@en ;
	rdfs:comment "A group of people represented by an election winner."@en ;
	rdfs:isDefinedBy <http://parliament.uk/ontologies/election/> .

pe:ConstituencyArea rdf:type owl:Class ;
	rdfs:label "Constituency area"@en ;
	rdfs:comment "An area within which members of a constituency group reside. Constituency areas bounding constituency groups represented in the House of Commons are set out by the Boundary Commissions and approved by Parliament."@en ;
	rdfs:isDefinedBy <http://parliament.uk/ontologies/election/> .
	
pe:Candidacy rdf:type owl:Class ;
	rdfs:label "Candidacy"@en ;
	rdfs:comment "A candidacy of a person standing in an election, for example: Phillip Hammond standing as the Conservative Party candidate in Runnymede and Weybridge, at the 2015 General Election."@en ;
	rdfs:isDefinedBy <http://parliament.uk/ontologies/election/> .

pe:CandidacyResult rdf:type owl:Class ;
	rdfs:label "Candidacy result"@en ;
	rdfs:comment "The result of a candidacy in an election, for example: Phillip Hammond's win as the Conservative Party candidate in Runnymede and Weybridge, at the 2015 General Election."@en ;
	rdfs:isDefinedBy <http://parliament.uk/ontologies/election/> .
	
pe:WinningCandidacyResult rdf:type owl:Class ;
	rdfs:subClassOf pe:CandidacyResult ;
	rdfs:label "Winning candidacy result"@en ;
	rdfs:comment "Used to record the winning candidacy in an election."@en ;
	rdfs:isDefinedBy <http://parliament.uk/ontologies/election/> .

pe:Certification rdf:type owl:Class ;
	rdfs:label "Certification"@en ;
	rdfs:comment "A certification of a candidate by a political party to stand in an election on behalf of that party. A candidate may be certified by more than one party, for example: by both The Labour Party and The Co-operative Party."@en ;
	rdfs:isDefinedBy <http://parliament.uk/ontologies/election/> .

pe:PoliticalParty rdf:type owl:Class ;
	rdfs:label "Political party"@en ;
	rdfs:comment "An organisation registered with the Electoral Commission as a political party."@en ;
	rdfs:isDefinedBy <http://parliament.uk/ontologies/election/> .
	
pe:Person rdf:type owl:Class ;
	rdfs:label "Person"@en ;
	rdfs:comment "A person."@en ;
	rdfs:isDefinedBy <http://parliament.uk/ontologies/election/> .
		
			

#######  Object properties ##### 

pe:intoParliamentPeriod rdf:type owl:ObjectProperty ;
	rdfs:label "Into Parliament period"@en ;
	rdfs:comment "Relates an election to the House of Commons to the Parliament period within which any resulting incumbency takes place. An election to the House of Commons is related to one Parliament period."@en ;
	rdfs:domain pe:Election ;
	rdfs:range pe:ParliamentPeriod ;
	rdfs:isDefinedBy <http://parliament.uk/ontologies/election/> .

pe:isPartOfGeneralElection rdf:type owl:ObjectProperty ;
	rdfs:label "Is part of general election"@en ;
	rdfs:comment "Relates a constituency election held as part of a general election to that general election. A constituency election is related to one general election, or none."@en ;
	rdfs:domain pe:Election ;
	rdfs:range pe:GeneralElection ;
	rdfs:isDefinedBy <http://parliament.uk/ontologies/election/> .
	
pe:eligibleToVoteIn rdf:type owl:ObjectProperty ;
	rdfs:label "Eligible to vote in"@en ;
	rdfs:comment "Relates a group of people - who at the time of an election are eligible to vote in that election - to that election. An election has one electorate. An electorate is eligible to take part in one or more elections."@en ;
	rdfs:domain pe:Electorate ;
	rdfs:range pe:Election ;
	rdfs:isDefinedBy <http://parliament.uk/ontologies/election/> .
	
pe:hasElectorate rdf:type owl:ObjectProperty ;
	rdfs:label "Has electorate"@en ;
	rdfs:comment "Relates a constituency group to a group of people who at the time of an election to the House of Commons are eligible to vote in the election for that constituency. Electorates in an election to the House of Commons are related to a constituency group; electorates for excepted hereditary peerage seats and for positions within Parliament are not. A constituency group has one electorate. An electorate forms part or all of one constituency group."@en ;
	rdfs:domain pe:ConstituencyGroup ;
	rdfs:range pe:Electorate  ;
	rdfs:isDefinedBy <http://parliament.uk/ontologies/election/> .
	
pe:boundedBy rdf:type owl:ObjectProperty ;
	rdfs:label "Bounded by"@en ;
	rdfs:comment "Relates a constituency group to a geographic area. Constituency groups represented in the House of Commons are within a constituency area. Some historical constituency groups had no defined geographical extent, for example: Oxford University. A boundary set change will result in the creation of both a new constituency area and a new constituency group. A constituency group is bounded by one constituency area, or none. A constituency area bounds one constituency group."@en ;
	rdfs:domain pe:ConstituencyGroup ;
	rdfs:range pe:ConstituencyArea ;
	rdfs:isDefinedBy <http://parliament.uk/ontologies/election/> .
	
pe:inElection rdf:type owl:ObjectProperty ;
	rdfs:label "In election"@en ;
	rdfs:comment "Relates a candidacy to the election that candidacy is in. A candidacy is in one election."@en ;
	rdfs:domain pe:Candidacy ;
	rdfs:range pe:Election  ;
	rdfs:isDefinedBy <http://parliament.uk/ontologies/election/> .
	
pe:hasCertification rdf:type owl:ObjectProperty ;
	rdfs:label "Has certification"@en ;
	rdfs:comment "Relates a candidacy to a certification by a political party of that candidacy. A candidacy has one or more certifications, or none. A certification is of one candidacy."@en ;
	rdfs:domain pe:Candidacy ;
	rdfs:range pe:Certification  ;
	rdfs:isDefinedBy <http://parliament.uk/ontologies/election/> .
	
pe:adjunctTo rdf:type owl:ObjectProperty ;
	rdfs:label "Adjunct to"@en ;
	rdfs:comment "Relates a certification to another certification to which it is adjunct, for example: relating a Co-operative Party certification to a Labour Party certification."@en ;
	rdfs:domain pe:Certification ;
	rdfs:range pe:Certification  ;
	rdfs:isDefinedBy <http://parliament.uk/ontologies/election/> .
	
pe:issuedBy rdf:type owl:ObjectProperty ;
	rdfs:label "Issued by"@en ;
	rdfs:comment "Relates a certification of a candidacy to the party issuing that certification. A certification is issued by one political party."@en ;
	rdfs:domain pe:Certification ;
	rdfs:range pe:PoliticalParty  ;
	rdfs:isDefinedBy <http://parliament.uk/ontologies/election/> .
	
pe:hasPoliticalParty rdf:type owl:ObjectProperty ;
	rdfs:label "Has political party"@en ;
	rdfs:comment "Relates a candidacy to a political party."@en ;
	rdfs:domain pe:Candidacy ;
	rdfs:range pe:PoliticalParty  ;
	rdfs:isDefinedBy <http://parliament.uk/ontologies/election/> .
	
pe:hasCandidate rdf:type owl:ObjectProperty ;
	rdfs:label "Has candidate"@en ;
	rdfs:comment "Relates a candidacy to a person being a candidate. A candidacy is of one person."@en ;
	rdfs:domain pe:Candidacy ;
	rdfs:range pe:Person  ;
	rdfs:isDefinedBy <http://parliament.uk/ontologies/election/> .
	
pe:hasCandidacyResult rdf:type owl:ObjectProperty ;
	rdfs:label "Has candidacy result"@en ;
	rdfs:comment "Relates a candidacy in an election to the result of that candidacy. A candidacy has one candidacy result. A candidacy result is for one candidacy."@en ;
	rdfs:domain pe:Candidacy ;
	rdfs:range pe:CandidacyResult  ;
	rdfs:isDefinedBy <http://parliament.uk/ontologies/election/> .
	
pe:ofPopulation rdf:type owl:ObjectProperty ;
	rdfs:label "Of population"@en ;
	rdfs:comment "Relates a population size as recorded on a date to that population. A population size is related to one population."@en ;
	rdfs:domain pe:PopulationSize ;
	rdfs:range pe:Population  ;
	rdfs:isDefinedBy <http://parliament.uk/ontologies/election/> .
	
	

#######  Data properties #####

pe:candidateName rdf:type owl:DatatypeProperty ;
	rdfs:label "Candidate name"@en ;
	rdfs:comment "The name of the candidate as it appears on the ballot."@en ;
	rdfs:domain pe:Candidacy ;
	rdfs:range rdf:langString ;
	rdfs:isDefinedBy <http://parliament.uk/ontologies/election/> .

pe:voteCount rdf:type owl:DatatypeProperty ;
	rdfs:label "Vote count"@en ;
	rdfs:comment "The number of accepted votes recorded for a candidacy."@en ;
	rdfs:domain pe:CandidacyResult ;
	rdfs:range xsd:integer ;
	rdfs:isDefinedBy <http://parliament.uk/ontologies/election/> .

pe:voteShare rdf:type owl:DatatypeProperty ;
	rdfs:label "Vote share"@en ;
	rdfs:comment "The share of a vote won in an election by a candidate as a fraction of the total accepted votes."@en ;
	rdfs:domain pe:CandidacyResult ;
	rdfs:range xsd:decimal ;
	rdfs:isDefinedBy <http://parliament.uk/ontologies/election/> .

pe:resultPosition rdf:type owl:DatatypeProperty ;
	rdfs:label "Result position"@en ;
	rdfs:comment "The ordinal position of the result of a candidacy in an election, for example: 1st or 2nd, recorded as 1 or 2."@en ;
	rdfs:domain pe:CandidacyResult ;
	rdfs:range xsd:integer ;
	rdfs:isDefinedBy <http://parliament.uk/ontologies/election/> .
	
											# edited to here
	
pe:recordedSize rdf:type owl:DatatypeProperty ;
	rdfs:label "Recorded size"@en ;
	rdfs:comment "The size of a population, for example: an electorate or constituency group."@en ;
	rdfs:domain pe:PopulationSize ;
	rdfs:range xsd:integer ;
	rdfs:isDefinedBy <http://parliament.uk/ontologies/election/> .
	
pe:recordedDate rdf:type owl:DatatypeProperty ;
	rdfs:label "Recorded date"@en ;
	rdfs:comment "The date on which a population size was recorded."@en ;
	rdfs:domain pe:PopulationSize ;
	rdfs:range xsd:date ;
	rdfs:isDefinedBy <http://parliament.uk/ontologies/election/> .	
	
pe:partyGained rdf:type owl:DatatypeProperty ;
	rdfs:label "Party gained"@en ;
	rdfs:comment "Whether the party certification of the winning candidate at an election differs from the party certification of the winning candidate at the preceding election."@en ;
	rdfs:domain pe:WinningCandidacyResult ;
	rdfs:range xsd:boolean ;
	rdfs:isDefinedBy <http://parliament.uk/ontologies/election/> .
	
pe:totalVotesCast rdf:type owl:DatatypeProperty ;
	rdfs:label "Total votes cast"@en ;
	rdfs:comment "The total number of votes cast across all candidacies in an election, including spoiled ballots. Turnout is defined by the House of Commons Library as the total number of votes cast and not spoiled, divided by the size of the electorate. This definition conforms to the generally accepted academic usage. Turnout is generally defined by Returning Officers as the total number of votes cast divided by the size of the electorate."@en ;
	rdfs:domain pe:Election ;
	rdfs:range xsd:integer ;
	rdfs:isDefinedBy <http://parliament.uk/ontologies/election/> .
		
pe:ballotsSpoiled rdf:type owl:DatatypeProperty ;
	rdfs:label "Ballots spoiled"@en ;
	rdfs:comment "The number of spoiled ballots cast by an electorate in an election, for example: ballots on which votes are given for more candidates than the voter is entitled to vote for, ballots on which anything is written or marked by which the voter can be identified, or ballots which are unmarked or void for uncertainty."@en ;
	rdfs:domain pe:Election ;
	rdfs:range xsd:integer ;
	rdfs:isDefinedBy <http://parliament.uk/ontologies/election/> .
	
pe:round rdf:type owl:DatatypeProperty ;
	rdfs:label "Round"@en ;
	rdfs:comment "The number of the round in an election having more than one round of voting."@en ;
	rdfs:domain pe:Election ;
	rdfs:range xsd:integer ;
	rdfs:isDefinedBy <http://parliament.uk/ontologies/election/> .
	
pe:declarationTime rdf:type owl:DatatypeProperty ;
	rdfs:label "Declaration time"@en ;
	rdfs:comment "The date and time at which results were declared for an election, for example: the declaration of the results in a constituency election, by the Returning Officer."@en ;
	rdfs:domain pe:Election ;
	rdfs:range xsd:dateTime ;
	rdfs:isDefinedBy <http://parliament.uk/ontologies/election/> .