@prefix pe: <http://parliament.uk/ontologies/election/> . 
@prefix xsd: <http://www.w3.org/2001/XMLSchema#> . 
@prefix rdf: <http://www.w3.org/1999/02/22-rdf-syntax-ns#> .
@prefix dcterms: <http://purl.org/dc/terms/> .
@prefix owl:     <http://www.w3.org/2002/07/owl#> .
@prefix rdfs:    <http://www.w3.org/2000/01/rdf-schema#> .
@prefix foaf:	<http://xmlns.com/foaf/0.1/> .

<http://parliament.uk/ontologies/election/> 
    rdf:type owl:Ontology ;
    dcterms:title "Election ontology"@en ;
    dcterms:created "2016-10-06"^^xsd:date ;
	dcterms:rights "Open Parliament Licence v3.0"@en ;
    dcterms:description "Election ontology for UK Parliament. This model describes the incumbencies resulting from general elections and by-elections for seats in the House of Commons, by-elections for excepted hereditary peers in the House of Lords and elections for positions including that of the Speaker of the House of Commons. The model describes the result of an election process rather than the process by which the election has been conducted: election returns by the “first past the post” system and those which follow other methods are included. The model is aligned with the Cabinet Office Election Result Data Standard, where applicable."@en ;
	foaf:depiction <election.png> .


#######  Classes ##### 	


pe:Election rdf:type owl:Class ;
	rdfs:label "Election"@en ;
	rdfs:comment "An election to elect a candidate or candidates to a seat or position."@en ;
	rdfs:isDefinedBy <http://parliament.uk/ontologies/election/> .
	
pe:ParliamentPeriod rdf:type owl:Class ;
	rdfs:label "Parliament period"@en ;
	rdfs:comment "The time period of a single Parliament between the date of its first assembly after a general election and its dissolution. A Parliament period contains contiguous session and prorogation periods: during a parliament period Parliament is either in session or prorogued. Until 2015, the dissolution proclamation named the date for Parliament to reassemble. After 2015, a Parliament begins on the date named in the proclamation issued after a dissolution. The start date of a Parliament may be changed by subsequent proclamations. A Parliament ends at the next dissolution. Until 2015 the date of dissolution was indeterminate and fixed by proclamation. After 2015 the date of dissolution is determined by the Fixed Term Parliament Act 2011, or is named in a proclamation after Parliament has voted for an early general election. Parliament periods are the same across both Houses. Parliaments are numbered ordinally from the first Parliament of the United Kingdom, sitting in 1801."@en ;
	rdfs:isDefinedBy <http://parliament.uk/ontologies/election/> .
	
pe:GeneralElection rdf:type owl:Class ;
	rdfs:label "General election"@en ;
	rdfs:comment "A set of elections to seats in the House of Commons held in all UK constituencies concurrently."@en ;
	rdfs:isDefinedBy <http://parliament.uk/ontologies/election/> .

pe:Population rdf:type owl:Class ;
	rdfs:label "Population"@en ;
	rdfs:comment "A set of people."@en ;
	rdfs:isDefinedBy <http://parliament.uk/ontologies/election/> .

pe:Electorate rdf:type owl:Class ;
	rdfs:subClassOf pe:Population ;
	rdfs:label "Electorate"@en ;
	rdfs:comment "A group of people who are eligible to vote in an election called at a particular time, for example: the group of people entitled to vote in a constituency election, or members of the House of Commons voting for their Speaker."@en ;
	rdfs:isDefinedBy <http://parliament.uk/ontologies/election/> .
	
pe:ConstituencyGroup rdf:type owl:Class ;
	rdfs:subClassOf pe:Population ;
	rdfs:label "Constituency group"@en ;
	rdfs:comment "A group of people represented by a person who has won an election, including people other than those eligible to vote at the time of election."@en ;
	rdfs:isDefinedBy <http://parliament.uk/ontologies/election/> .	
	
pe:ConstituencyAreaType rdf:type owl:Class ;
	rdfs:label "Constituency area type"@en ;
	rdfs:comment "The type of constituency area, for example: a borough or a county."@en ;
	rdfs:isDefinedBy <http://parliament.uk/ontologies/election/> .	

pe:ConstituencyArea rdf:type owl:Class ;
	rdfs:label "Constituency area"@en ;
	rdfs:comment "A geographic bounding of a constituency group."@en ;
	rdfs:isDefinedBy <http://parliament.uk/ontologies/election/> .
	
pe:Candidacy rdf:type owl:Class ;
	rdfs:label "Candidacy"@en ;
	rdfs:comment "A person standing as a candidate in an election, for example: Phillip Hammond standing as the Conservative Party candidate in Runnymede and Weybridge, at the 2015 General Election."@en ;
	rdfs:isDefinedBy <http://parliament.uk/ontologies/election/> .

pe:CandidacyResult rdf:type owl:Class ;
	rdfs:label "Candidacy result"@en ;
	rdfs:comment "The result of a person’s candidacy in an election."@en ;
	rdfs:isDefinedBy <http://parliament.uk/ontologies/election/> .
	
pe:WinningCandidacyResult rdf:type owl:Class ;
	rdfs:subClassOf pe:CandidacyResult ;
	rdfs:label "Winning candidacy result"@en ;
	rdfs:comment "Identifies a winning candidacy in an election."@en ;
	rdfs:isDefinedBy <http://parliament.uk/ontologies/election/> .

pe:Certification rdf:type owl:Class ;
	rdfs:label "Certification"@en ;
	rdfs:comment "A certification of a candidate by a political party, registered by the Electoral Commission, to stand in an election on behalf of that party. A candidate may be certified by more than one party, for example: by both The Labour Party and The Co-operative Party."@en ;
	rdfs:isDefinedBy <http://parliament.uk/ontologies/election/> .

pe:PoliticalParty rdf:type owl:Class ;
	rdfs:label "Political party"@en ;
	rdfs:comment "A group registered with the Electoral Commission as a political party."@en ;
	rdfs:isDefinedBy <http://parliament.uk/ontologies/election/> .
	
pe:Person rdf:type owl:Class ;
	rdfs:label "Person"@en ;
	rdfs:comment "A person."@en ;
	rdfs:isDefinedBy <http://parliament.uk/ontologies/election/> .

pe:ElectoralIncumbency rdf:type owl:Class ;
	rdfs:label "Electoral incumbency"@en ;
	rdfs:comment "An incumbency in a position or parliamentary seat decided by the result of an election."@en ;
	rdfs:isDefinedBy <http://parliament.uk/ontologies/election/> .
		
			

#######  Object properties ##### 

pe:intoParliamentPeriod rdf:type owl:ObjectProperty ;
	rdfs:label "Into Parliament period"@en ;
	rdfs:comment "Relates an election to the Parliament period within which any resulting incumbency will take place."@en ;
	rdfs:domain pe:Election ;
	rdfs:range pe:ParliamentPeriod ;
	rdfs:isDefinedBy <http://parliament.uk/ontologies/election/> .

pe:hasConstituencyAreaType rdf:type owl:ObjectProperty ;
	rdfs:label "Has constituency area type"@en ;
	rdfs:comment "Relates a constituency area to a constituency area type."@en ;
	rdfs:domain pe:ConstituencyArea ;
	rdfs:range pe:ConstituencyAreaType ;
	rdfs:isDefinedBy <http://parliament.uk/ontologies/election/> .

pe:isPartOfGeneralElection rdf:type owl:ObjectProperty ;
	rdfs:label "Is part of general election"@en ;
	rdfs:comment "Relates a constituency election to the general election of which it forms part."@en ;
	rdfs:domain pe:Election ;
	rdfs:range pe:GeneralElection ;
	rdfs:isDefinedBy <http://parliament.uk/ontologies/election/> .
	
pe:eligibleToVoteIn rdf:type owl:ObjectProperty ;
	rdfs:label "Eligible to vote in"@en ;
	rdfs:comment "Relates a group of people - who at the time of an election are eligible to vote - to that election."@en ;
	rdfs:domain pe:Electorate ;
	rdfs:range pe:Election ;
	rdfs:isDefinedBy <http://parliament.uk/ontologies/election/> .
	
pe:hasElectorate rdf:type owl:ObjectProperty ;
	rdfs:label "Has electorate"@en ;
	rdfs:comment "Relates a geographic area to a group of people who at the time of an election are eligible to vote in the election for that area."@en ;
	rdfs:domain pe:ConstituencyArea ;
	rdfs:range pe:Electorate  ;
	rdfs:isDefinedBy <http://parliament.uk/ontologies/election/> .
	
pe:hasConstituencyGroup rdf:type owl:ObjectProperty ;
	rdfs:label "Has constituency group"@en ;
	rdfs:comment "Relates a geographic area to its population."@en ;
	rdfs:domain pe:ConstituencyArea ;
	rdfs:range pe:ConstituencyGroup ;
	rdfs:isDefinedBy <http://parliament.uk/ontologies/election/> .
	
pe:hasCandidacy rdf:type owl:ObjectProperty ;
	rdfs:label "Has candidacy"@en ;
	rdfs:comment "Relates an election to a candidacy within that election."@en ;
	rdfs:domain pe:Election ;
	rdfs:range pe:Candidacy  ;
	rdfs:isDefinedBy <http://parliament.uk/ontologies/election/> .
	
pe:hasCertification rdf:type owl:ObjectProperty ;
	rdfs:label "Has certification"@en ;
	rdfs:comment "Relates a candidacy to a certification of the candidate by a political party."@en ;
	rdfs:domain pe:Candidacy ;
	rdfs:range pe:Certification  ;
	rdfs:isDefinedBy <http://parliament.uk/ontologies/election/> .
	
pe:adjunctTo rdf:type owl:ObjectProperty ;
	rdfs:label "Adjunct to"@en ;
	rdfs:comment "Relates an adjunct certification to a certification, for example: relating a Co-operative Party certification to a Labour Party certification."@en ;
	rdfs:domain pe:Certification ;
	rdfs:range pe:Certification  ;
	rdfs:isDefinedBy <http://parliament.uk/ontologies/election/> .
	
pe:toParty rdf:type owl:ObjectProperty ;
	rdfs:label "To party"@en ;
	rdfs:comment "Relates a certification of a candidate to the party issuing the certification."@en ;
	rdfs:domain pe:Certification ;
	rdfs:range pe:PoliticalParty  ;
	rdfs:isDefinedBy <http://parliament.uk/ontologies/election/> .
	
pe:hasCandidate rdf:type owl:ObjectProperty ;
	rdfs:label "Has candidate"@en ;
	rdfs:comment "Relates a candidacy to a person being a candidate."@en ;
	rdfs:domain pe:Candidacy ;
	rdfs:range pe:Person  ;
	rdfs:isDefinedBy <http://parliament.uk/ontologies/election/> .
	
pe:hasCandidacyResult rdf:type owl:ObjectProperty ;
	rdfs:label "Has candidacy result"@en ;
	rdfs:comment "Relates a candidacy to the result of that candidacy in an election."@en ;
	rdfs:domain pe:Candidacy ;
	rdfs:range pe:CandidacyResult  ;
	rdfs:isDefinedBy <http://parliament.uk/ontologies/election/> .
	
pe:establishesIncumbency rdf:type owl:ObjectProperty ;
	rdfs:label "Establishes incumbency"@en ;
	rdfs:comment "Relates a winning candidacy result to an electoral incumbency."@en ;
	rdfs:domain pe:WinningCandidacyResult  ;
	rdfs:range pe:ElectoralIncumbency  ;
	rdfs:isDefinedBy <http://parliament.uk/ontologies/election/> .				

#######  Data properties ##### 

pe:voteCount rdf:type owl:DatatypeProperty ;
	rdfs:label "Vote count"@en ;
	rdfs:comment "The number of accepted votes recorded for a candidacy."@en ;
	rdfs:domain pe:CandidacyResult ;
	rdfs:range xsd:integer ;
	rdfs:isDefinedBy <http://parliament.uk/ontologies/election/> .

pe:voteShare rdf:type owl:DatatypeProperty ;
	rdfs:label "Vote share"@en ;
	rdfs:comment "The share of a vote won in an election by a candidate as a fraction of the accepted votes."@en ;
	rdfs:domain pe:CandidacyResult ;
	rdfs:range xsd:decimal ;
	rdfs:isDefinedBy <http://parliament.uk/ontologies/election/> .

pe:resultPosition rdf:type owl:DatatypeProperty ;
	rdfs:label "Result position"@en ;
	rdfs:comment "The relative position of the result of the candidacy in an election."@en ;
	rdfs:domain pe:CandidacyResult ;
	rdfs:range xsd:integer ;
	rdfs:isDefinedBy <http://parliament.uk/ontologies/election/> .
	
pe:populationSize rdf:type owl:DatatypeProperty ;
	rdfs:label "Population size"@en ;
	rdfs:comment "The size of a population, for example: an electorate or constituency group."@en ;
	rdfs:domain pe:Population ;
	rdfs:range xsd:integer ;
	rdfs:isDefinedBy <http://parliament.uk/ontologies/election/> .
	
pe:recordedDate rdf:type owl:DatatypeProperty ;
	rdfs:label "Recorded date"@en ;
	rdfs:comment "The date on which a population size was recorded."@en ;
	rdfs:domain pe:Population ;
	rdfs:range xsd:date ;
	rdfs:isDefinedBy <http://parliament.uk/ontologies/election/> .	
	
pe:partyGained rdf:type owl:DatatypeProperty ;
	rdfs:label "Party gained"@en ;
	rdfs:comment "Whether the party certification of the winning candidate at an election differs from the party certification of the winning candidate at the preceding election."@en ;
	rdfs:domain pe:WinningCandidacyResult ;
	rdfs:range xsd:boolean ;
	rdfs:isDefinedBy <http://parliament.uk/ontologies/election/> .
	
pe:totalVotesCast rdf:type owl:DatatypeProperty ;
	rdfs:label "Total votes cast"@en ;
	rdfs:comment "The total number of votes cast across all candidacies in an election, including spoiled ballots. Turnout is defined by the House of Commons Library as the total number of votes cast and not spoiled, divided by the size of the electorate. This definition conforms to the generally accepted academic usage. Turnout is generally defined by Returning Officers as the total number of votes cast divided by the size of the electorate."@en ;
	rdfs:domain pe:Election ;
	rdfs:range xsd:integer ;
	rdfs:isDefinedBy <http://parliament.uk/ontologies/election/> .
		
pe:ballotsSpoiled rdf:type owl:DatatypeProperty ;
	rdfs:label "Ballots spoiled"@en ;
	rdfs:comment "The number of spoiled ballots cast by an electorate in an election, for example: ballots on which votes are given for more candidates than the voter is entitled to vote for, ballots on which anything is written or marked by which the voter can be identified, or ballots which are unmarked or void for uncertainty."@en ;
	rdfs:domain pe:Election ;
	rdfs:range xsd:integer ;
	rdfs:isDefinedBy <http://parliament.uk/ontologies/election/> .
	
pe:round rdf:type owl:DatatypeProperty ;
	rdfs:label "round"@en ;
	rdfs:comment "The number of the round in an election having more than one round of voting."@en ;
	rdfs:domain pe:Election ;
	rdfs:range xsd:integer ;
	rdfs:isDefinedBy <http://parliament.uk/ontologies/election/> .
	
pe:declarationTime rdf:type owl:DatatypeProperty ;
	rdfs:label "declarationTime"@en ;
	rdfs:comment "The date and time at which results were declared for an election, for example: the declaration of the results in a constituency election, by the Returning Officer."@en ;
	rdfs:domain pe:Election ;
	rdfs:range xsd:dateTime ;
	rdfs:isDefinedBy <http://parliament.uk/ontologies/election/> .