@prefix ppr: <http://parliament.uk/ontologies/procedure/> . 
@prefix xsd: <http://www.w3.org/2001/XMLSchema#> . 
@prefix rdf: <http://www.w3.org/1999/02/22-rdf-syntax-ns#> .
@prefix dcterms: <http://purl.org/dc/terms/> .
@prefix owl:     <http://www.w3.org/2002/07/owl#> .
@prefix rdfs:    <http://www.w3.org/2000/01/rdf-schema#> .
@prefix foaf:	<http://xmlns.com/foaf/0.1/> .

<http://parliament.uk/ontologies/procedure/> 
    rdf:type owl:Ontology ;
    dcterms:title "Procedure ontology"@en ;
    dcterms:created "2018-02-20"^^xsd:date ;
	dcterms:rights "Open Parliament Licence v3.0"@en ;
    dcterms:description "A general purpose process flow model used to describe parliamentary procedure as a set of steps connected by routes. A step is a waypoint in a process, a route is a direction between steps and a procedure is analogous to a map of all possible routes. The model also describes the package of work in Parliament resulting from a bill or an instrument subject to a procedure."@en ;
	foaf:depiction <https://ukparliament.github.io/ontologies/procedure/procedure.png> ;
	foaf:maker
		[ foaf:name "Chris Alcock" ],
		[ foaf:name "David Beamish" ],
		[ foaf:name "Robert Brook"; foaf:homepage <https://robert-brook.com/> ],
		[ foaf:name "Gordon Clarke" ],
		[ foaf:name "Jack Dent" ],
		[ foaf:name "Samu Lang" ],
		[ foaf:name "Silver Oliver" ],
		[ foaf:name "Michael Smethurst"; foaf:homepage <http://smethur.st/> ],
	    [ foaf:name "Anya Somerville" ],
	    [ foaf:name "Dominic Stockbridge" ],
	    [ foaf:name "Jayne Sunley" ],
		[ foaf:name "James Vinter" ],
		[ foaf:name "Jane White" ],
		[ foaf:name "Ben Woodhams" ].


#######  Classes #####
	
ppr:Procedure rdf:type owl:Class ;
	rdfs:label "Procedure"@en ;
	rdfs:comment "A procedure in a House or Houses. For example, the passage of a made affirmative statutory instrument in both Houses. A procedure may consist of business in a particular House, such as a division; business undertaken by both Houses jointly, such as a joint committee; processes applying to either House, such as a time period; and activities outside Parliament, such as the making of a statutory instrument. In this model a procedure that consists of business in both Houses is considered as a single procedure. Procedures may be constructed from commonly occurring sets of routes. For example, the set of routes involved in EVEL certification."@en ;
	rdfs:isDefinedBy <http://parliament.uk/ontologies/procedure/> .
	
ppr:Route rdf:type owl:Class ;
	rdfs:label "Route"@en ;
	rdfs:comment "A route is a link from one step to another. The source of a route may also be its destination. A route is available when the from step is True, actualised by a business item having a date in the past, or by the input from a logic gate step being True. The validity period of a route may be indicated by its start or end date. A route linking a business step actualised by a business item with a date in the past to a business step which has not been actualised indicates that actualisation of the step will happen in the future, being a causal relationship."@en ;
	rdfs:isDefinedBy <http://parliament.uk/ontologies/procedure/> .

ppr:Step rdf:type owl:Class ;
	rdfs:label "Step"@en ;
	rdfs:comment "A step is either a business step, a logic gate step or a decision step. Steps are joined by routes to form procedures. For example, within the SI procedures there exists a step named 'English Votes for English Laws (EVEL) consideration'. Steps may occur in more than one procedure. For example, all statutory instrument procedures include the EVEL consideration step."@en ;
	rdfs:isDefinedBy <http://parliament.uk/ontologies/procedure/> .
	
ppr:StepType rdf:type owl:Class ;
	rdfs:label "Step type"@en ;
	rdfs:comment "A step has one type: a business step type, a decision step type, a logical NOT step type, a logical AND step type or a logical OR step type. Business step: a step that can be actualised by a business item. Decision step: a step that is used to describe the requirement for a decision to be made before the subsequent route can be followed. Routes including a decision step indicate that the target step is allowed and not caused: a route linking a business step actualised by a business item with a date in the past to a business step which has not been actualised by means of a decision step indicates that actualisation of the step may happen in the future, being an allowed relationship. Logical step: a step that describes logical operations performed over routes. Inputs and outputs of a logic gate are either TRUE or FALSE. The output from a business step which has been actualised by a business item with a date in the past is TRUE. The output from a business step which has not been actualised, or which has been actualised with a business item with a date in the future, is neither TRUE nor FALSE: this is recorded as NULL. A NULL route entering a logic step acts as a bypass to that step: a logic gate with a NULL input outputs the other given input, or NULL if there is no other input."@en ;
	rdfs:seeAlso <https://ukparliament.github.io/ontologies/procedure/flowcharts/meta/design-notes/> ;
	rdfs:isDefinedBy <http://parliament.uk/ontologies/procedure/> .
	
ppr:House rdf:type owl:Class ;
	rdfs:label "House"@en ;
	rdfs:comment "A parliamentary House, for example: the House of Lords."@en ;
	rdfs:isDefinedBy <http://parliament.uk/ontologies/procedure/> .
	
ppr:BusinessItem rdf:type owl:Class ;
	rdfs:label "Business item"@en ;
	rdfs:comment "An item of business conducted either within or outside Parliament. For example: a second reading debate, the tabling of an early day motion, a laying of a paper, the making of a statutory instrument by a government minister."@en ;
	rdfs:isDefinedBy <http://parliament.uk/ontologies/procedure/> .
	
ppr:WorkPackage rdf:type owl:Class ;
	rdfs:label "Work package"@en ;
	rdfs:comment "A group of business items under a procedure or as determined by a committee, for example: business items considered during the passage of a particular Statutory Instrument or Public Bill, or during an inquiry by a Select Committee."@en ;
	rdfs:isDefinedBy <http://parliament.uk/ontologies/procedure/> .
	
ppr:WorkPackageableThing rdf:type owl:Class ;
	rdfs:label "Work packageable thing"@en ;
	rdfs:comment "A thing which is the focus of a work package. For example a statutory instrument paper or the work of a government department."@en ;
	rdfs:isDefinedBy <http://parliament.uk/ontologies/procedure/> .

ppr:StepCollection rdf:type owl:Class ;
	rdfs:label "Step collection"@en ;
	rdfs:comment "A grouping of steps in a procedure. A step grouping may belong to one or both Houses, or neither."@en ;
	rdfs:isDefinedBy <http://parliament.uk/ontologies/procedure/> .
	
ppr:StepCollectionType rdf:type owl:Class ;
	rdfs:label "Step collection type"@en ;
	rdfs:comment "The type of a step collection, for example: starting steps, concluding steps, key steps, bill stage steps, or Member action steps. A step grouping of type ‘starting steps’ collects steps in a procedure which, when actualised in a work package, denote that that work package is considered to be started. A procedure may have one or more starting steps. A step grouping of type ‘concluding steps’ collects steps in a procedure which, when actualised in a work package, denote that that work package is considered to be concluded. A procedure may have one or more concluding steps. A step grouping of type ‘bill stage steps’ collects steps forming a stage in the passage of a bill. A step grouping of type ‘key steps’ collects steps in a procedure which are considered to be key to that procedure. A procedure may have one or more steps described as key steps. A step grouping of type ‘Member action steps’ collects steps in a procedure which are considered to be steps at which a Member is able to take an action. A procedure may have one or more steps described as Member action steps."@en ;
	rdfs:isDefinedBy <http://parliament.uk/ontologies/procedure/> .
	
ppr:Citation rdf:type owl:Class ;
	rdfs:label "Citation"@en ;
	rdfs:comment "A citation of a document. A citation may be from a procedure, for example: the proposed negative statutory instrument procedure citing Schedule 7 to the European Union (Withdrawal) Act 2018. A citation may be from a step in a procedure, for example: the step 'CF - AND' in the made negative statutory instrument procedure citing Section 4(1) of the Statutory Instrument Act 1946. A citation may be from a step without reference to a particular procedure, for example: the step 'Considered for English votes for English laws (EVEL) certification' citing House of Commons public Standing Order 83P."@en ;
	rdfs:isDefinedBy <http://parliament.uk/ontologies/procedure/> .
	
ppr:DocumentType rdf:type owl:Class ;
	rdfs:label "Document type"@en ;
	rdfs:comment "The type of a document being cited, for example: a standing order or a section of legislation."@en ;
	rdfs:isDefinedBy <http://parliament.uk/ontologies/procedure/> .
	


#######  Object properties ##### 

ppr:formsPartOf rdf:type owl:ObjectProperty ;
	rdfs:label "Forms part of"@en ;
	rdfs:comment "Relates a business item to a work package it forms part of. One or more business items may form part of a work package. A business item may form part of one or more work packages, for example: a meeting of the Joint Committee on Statutory Instruments may consider one or more SIs, each SI being the focus of a separate work package."@en ;
	rdfs:domain ppr:BusinessItem ;
	rdfs:range ppr:WorkPackage ;
	rdfs:isDefinedBy <http://parliament.uk/ontologies/procedure/> .

ppr:subjectTo rdf:type owl:ObjectProperty ;
	rdfs:label "Subject to"@en ;
	rdfs:comment "Relates a work package to the procedure it is subject to. A work package is only subject to one procedure."@en ;
	rdfs:domain ppr:WorkPackage ;
	rdfs:range ppr:Procedure ;
	rdfs:isDefinedBy <http://parliament.uk/ontologies/procedure/> .
	
ppr:actualises rdf:type owl:ObjectProperty ;
	rdfs:label "Actualises"@en ;
	rdfs:comment "Relates a business item to a step in a procedure by means of a route. For example, relating the second reading of a public bill to the second reading step in the procedure. A step may be actualised by more than one business item in different work packages. A business item may actualise one or more steps. For example, a business item appearing in the Order Paper including a debate on several motions may actualise steps relating to each motion."@en ;
	rdfs:domain ppr:BusinessItem ;
	rdfs:range ppr:Step ;
	rdfs:isDefinedBy <http://parliament.uk/ontologies/procedure/> .

ppr:hasStepType rdf:type owl:ObjectProperty ;
	rdfs:label "Has step type"@en ;
	rdfs:comment "Relates a step to its type. A step may only be of one type. A step type may be related to one or more steps, or none."@en ;
	rdfs:domain ppr:Step ;
	rdfs:range ppr:StepType ;
	rdfs:isDefinedBy <http://parliament.uk/ontologies/procedure/> .

ppr:fromStep rdf:type owl:ObjectProperty ;
	rdfs:label "From step"@en ;
	rdfs:comment "Relates a route to its input step."@en ;
	rdfs:domain ppr:Route ;
	rdfs:range ppr:Step ;
	rdfs:isDefinedBy <http://parliament.uk/ontologies/procedure/> .
	
ppr:toStep rdf:type owl:ObjectProperty ;
	rdfs:label "To step"@en ;
	rdfs:comment "Relates a route to its output step."@en ;
	rdfs:domain ppr:Route ;
	rdfs:range ppr:Step ;
	rdfs:isDefinedBy <http://parliament.uk/ontologies/procedure/> .
	
ppr:followsRoute rdf:type owl:ObjectProperty ;
	rdfs:label "Follows route"@en ;
	rdfs:comment "Relates a procedure to a route. A route may appear in one or more procedures. For example, the route between 'Considered for English votes for English laws (EVEL) certification' to 'Certified as England only under the English votes for English laws (EVEL) process' appears in the draft negative, made negative, draft affirmative and made affirmative procedures."@en ;
	rdfs:domain ppr:Procedure ;
	rdfs:range ppr:Route ;
	rdfs:isDefinedBy <http://parliament.uk/ontologies/procedure/> .
	
ppr:stepInHouse rdf:type owl:ObjectProperty ;
	rdfs:label "Step in House"@en ;
	rdfs:comment "Relates a step to one or both Houses where such a relationship exists. A step may exist with no relationship to a House. For example, the making of a statutory instrument takes place outside of Parliament."@en ;
	rdfs:domain ppr:Step ;
	rdfs:range ppr:House ;
	rdfs:isDefinedBy <http://parliament.uk/ontologies/procedure/> .
		
ppr:focus rdf:type owl:ObjectProperty ;
	rdfs:label "Focus"@en ;
	rdfs:comment "Relates a work package to its focus, this being a work packageable thing."@en ;
	rdfs:domain ppr:WorkPackage ;
	rdfs:range ppr:WorkPackageableThing ;
	rdfs:isDefinedBy <http://parliament.uk/ontologies/procedure/> .
	
ppr:stepCollectionInHouse rdf:type owl:ObjectProperty ;
	rdfs:label "Step collection in House"@en ;
	rdfs:comment "Relates a step collection to one or both Houses, or none."@en ;
	rdfs:domain ppr:StepCollection ;
	rdfs:range ppr:House ;
	rdfs:isDefinedBy <http://parliament.uk/ontologies/procedure/> .
	
ppr:hasStepCollectionType rdf:type owl:ObjectProperty ;
	rdfs:label "Has step collection type"@en ;
	rdfs:comment "Related a step collection to its type. A step collection may only be of one type. A step collection type may be related to one or more steps, or none.."@en ;
	rdfs:domain ppr:StepCollection ;
	rdfs:range ppr:StepCollectionType ;
	rdfs:isDefinedBy <http://parliament.uk/ontologies/procedure/> .
	
ppr:isCollectedBy rdf:type owl:ObjectProperty ;
	rdfs:label "Is collected by"@en ;
	rdfs:comment "Relates a step to a step collection the step is collected by. A step collection collects one or more steps. A step may be collected by one or more step collections, or none."@en ;
	rdfs:domain ppr:Step ;
	rdfs:range ppr:StepCollection ;
	rdfs:isDefinedBy <http://parliament.uk/ontologies/procedure/> .
	
ppr:hasProcedure rdf:type owl:ObjectProperty ;
	rdfs:label "Has procedure"@en ;
	rdfs:comment "Relates a step collection to a procedure. A step collection may have one or more procedures, or none. A procedure may have one or more step collections, or none."@en ;
	rdfs:domain ppr:StepCollection ;
	rdfs:range ppr:Procedure ;
	rdfs:isDefinedBy <http://parliament.uk/ontologies/procedure/> .
	
ppr:stepHasCitation rdf:type owl:ObjectProperty ;
	rdfs:label "Step has citation"@en ;
	rdfs:comment "Relates a step to a citation. A step may have more than one citation, or none."@en ;
	rdfs:domain ppr:Step ;
	rdfs:range ppr:Citation ;
	rdfs:isDefinedBy <http://parliament.uk/ontologies/procedure/> .
	
ppr:procedureHasCitation rdf:type owl:ObjectProperty ;
	rdfs:label "Procedure has citation"@en ;
	rdfs:comment "Relates a procedure to a citation. A procedure may have more than one citation, or none."@en ;
	rdfs:domain ppr:Procedure ;
	rdfs:range ppr:Citation ;
	rdfs:isDefinedBy <http://parliament.uk/ontologies/procedure/> .
	
ppr:hasDocumentType rdf:type owl:ObjectProperty ;
	rdfs:label "Has document type"@en ;
	rdfs:comment "Relates a citation to the type of the document being cited."@en ;
	rdfs:domain ppr:Citation ;
	rdfs:range ppr:DocumentType ;
	rdfs:isDefinedBy <http://parliament.uk/ontologies/procedure/> .
				

#######  Data properties ##### 

ppr:title rdf:type owl:DatatypeProperty ;
	rdfs:label "Title"@en ;
	rdfs:comment "Relates a citation to the title of the document being cited."@en ;
	rdfs:domain ppr:Citation ;
	rdfs:range rdf:langString ;
	rdfs:isDefinedBy <http://parliament.uk/ontologies/procedure/> .
	
ppr:uri rdf:type owl:DatatypeProperty ;
	rdfs:label "URI"@en ;
	rdfs:comment "Relates a citation to the URI of the document being cited."@en ;
	rdfs:domain ppr:Citation ;
	rdfs:range rdfs:Literal ;
	rdfs:isDefinedBy <http://parliament.uk/ontologies/procedure/> .