@prefix ppr: <http://parliament.uk/ontologies/procedure/> . 
@prefix xsd: <http://www.w3.org/2001/XMLSchema#> . 
@prefix rdf: <http://www.w3.org/1999/02/22-rdf-syntax-ns#> .
@prefix dcterms: <http://purl.org/dc/terms/> .
@prefix owl:     <http://www.w3.org/2002/07/owl#> .
@prefix rdfs:    <http://www.w3.org/2000/01/rdf-schema#> .
@prefix foaf:	<http://xmlns.com/foaf/0.1/> .

<http://parliament.uk/ontologies/procedure/> 
    rdf:type owl:Ontology ;
    dcterms:title "Procedure ontology"@en ;
    dcterms:created "2018-02-20"^^xsd:date ;
	dcterms:rights "Open Parliament Licence v3.0"@en ;
    dcterms:description "A general purpose process flow model used to describe parliamentary procedure as a set of steps connected by routes. A step is a waypoint in a process, a route is a direction between steps and a procedure is analogous to a map of all possible routes. The model also describes the package of work in Parliament resulting from a bill or an instrument subject to a procedure."@en ;
	foaf:depiction <https://ukparliament.github.io/ontologies/procedure/procedure.png> ;
	foaf:maker
		[ foaf:name "Chris Alcock" ],
		[ foaf:name "David Beamish" ],
		[ foaf:name "Robert Brook"; foaf:homepage <https://robert-brook.com/> ],
		[ foaf:name "Gordon Clarke" ],
		[ foaf:name "Jack Dent" ],
		[ foaf:name "Samu Lang" ],
		[ foaf:name "Silver Oliver" ],
		[ foaf:name "Michael Smethurst"; foaf:homepage <http://smethur.st/> ],
	    [ foaf:name "Anya Somerville" ],
	    [ foaf:name "Dominic Stockbridge" ],
	    [ foaf:name "Jayne Sunley" ],
		[ foaf:name "James Vinter" ],
		[ foaf:name "Jane White" ],
		[ foaf:name "Ben Woodhams" ].


#######  Classes #####
	
ppr:Procedure rdf:type owl:Class ;
	rdfs:label "Procedure"@en ;
	rdfs:comment "A procedure in a House or Houses. For example, the passage of a made affirmative statutory instrument in both Houses. A procedure may consist of business in a particular House, such as a division; business undertaken by both Houses jointly, such as a joint committee; processes applying to either House, such as a time period; and activities outside Parliament, such as the making of a statutory instrument. In this model a procedure that consists of business in both Houses is considered as a single procedure. Procedures may be constructed from commonly occurring sets of routes. For example, the set of routes involved in EVEL certification."@en ;
	rdfs:isDefinedBy <http://parliament.uk/ontologies/procedure/> .
	
ppr:Route rdf:type owl:Class ;
	rdfs:label "Route"@en ;
	rdfs:comment "A route is a link from one step to another. The source of a route may also be its destination. A route is available when the from step is True, actualised by a business item having a date in the past, or by the input from a logic gate step being True. The validity period of a route may be indicated by its start or end date. A route linking a business step actualised by a business item with a date in the past to a business step which has not been actualised indicates that actualisation of the step will happen in the future, being a causal relationship."@en ;
	rdfs:isDefinedBy <http://parliament.uk/ontologies/procedure/> .

ppr:Step rdf:type owl:Class ;
	rdfs:label "Step"@en ;
	rdfs:comment "A step is either a business step, a logic gate step or a decision step. Steps are joined by routes to form procedures. For example, within the SI procedures there exists a step named 'English Votes for English Laws (EVEL) consideration'. Steps may occur in more than one procedure. For example, all statutory instrument procedures include the EVEL consideration step."@en ;
	rdfs:isDefinedBy <http://parliament.uk/ontologies/procedure/> .
	
ppr:StepType rdf:type owl:Class ;
	rdfs:label "Step type"@en ;
	rdfs:comment "A step has one type. The type of a step is a business step, decision step, logical NOT step, logical AND step, logical OR step, arithmetic SUM step, arithmetic INCREMENT step, arithmetic EQUALS step, or summation step."@en ;
	rdfs:seeAlso <https://ukparliament.github.io/ontologies/procedure/flowcharts/meta/design-notes/> ;
	rdfs:isDefinedBy <http://parliament.uk/ontologies/procedure/> .
	
ppr:House rdf:type owl:Class ;
	rdfs:label "House"@en ;
	rdfs:comment "A parliamentary House, for example: the House of Lords."@en ;
	rdfs:isDefinedBy <http://parliament.uk/ontologies/procedure/> .
	
ppr:BusinessItem rdf:type owl:Class ;
	rdfs:label "Business item"@en ;
	rdfs:comment "An item of business conducted either within or outside Parliament. For example: a second reading debate, the tabling of an early day motion, a laying of a paper, the making of a statutory instrument by a government minister."@en ;
	rdfs:isDefinedBy <http://parliament.uk/ontologies/procedure/> .
	
ppr:WorkPackage rdf:type owl:Class ;
	rdfs:label "Work package"@en ;
	rdfs:comment "A group of business items under a procedure or as determined by a committee, for example: business items considered during the passage of a particular Statutory Instrument or Public Bill, or during an inquiry by a Select Committee."@en ;
	rdfs:isDefinedBy <http://parliament.uk/ontologies/procedure/> .
	
ppr:WorkPackageableThing rdf:type owl:Class ;
	rdfs:label "Work packageable thing"@en ;
	rdfs:comment "A thing which is the focus of a work package. For example a statutory instrument paper or the work of a government department."@en ;
	rdfs:isDefinedBy <http://parliament.uk/ontologies/procedure/> .

ppr:StepCollectionMembership rdf:type owl:Class ;
	rdfs:label "Step collection membership"@en ;
	rdfs:comment "The membership of a step in a step collection."@en ;
	rdfs:isDefinedBy <http://parliament.uk/ontologies/procedure/> .

ppr:StepCollection rdf:type owl:Class ;
	rdfs:label "Step collection"@en ;
	rdfs:comment "A collection of steps. Step collections are used to collect steps of one type, for example: starting steps, concluding steps, key steps, bill stage steps, or Member action steps. A step collection named 'Starting steps' collects steps in a procedure which, when actualised in a work package, denote that that work package is considered to be started. A procedure may have one or more starting steps. A step collection named 'Concluding steps' collects steps in a procedure which, when actualised in a work package, denote that that work package is considered to be concluded. A procedure may have one or more concluding steps. A step collection named 'Second reading', within the House of Commons, collects steps forming that stage in that House. A step collection named 'Key steps' collects steps in a procedure which are considered to be key to that procedure. A procedure may have one or more steps described as key steps. A step collection named 'Member action steps' collects steps in a procedure which are considered to be steps at which a Member is able to take an action. A procedure may have one or more steps considered to be Member action steps."@en ;
	rdfs:isDefinedBy <http://parliament.uk/ontologies/procedure/> .
	
ppr:Citation rdf:type owl:Class ;
	rdfs:label "Citation"@en ;
	rdfs:comment "A citation of a document. A citation may be from a procedure, for example: the proposed negative statutory instrument procedure citing Schedule 7 to the European Union (Withdrawal) Act 2018. A citation may be from a step in a procedure, for example: the step 'CF - AND' in the made negative statutory instrument procedure citing Section 4(1) of the Statutory Instrument Act 1946. A citation may be from a step without reference to a particular procedure, for example: the step 'Considered for English votes for English laws (EVEL) certification' citing House of Commons public Standing Order 83P. A citation may be from a route in a procedure, for example: the route from 'Considered by the Joint Committee on Statutory Instruments' to 'Motion to approve the instrument tabled by the Government (House of Lords)' in both affirmative procedures citing House of Lords public Standing Order 72."@en ;
	rdfs:isDefinedBy <http://parliament.uk/ontologies/procedure/> .
	
ppr:DocumentType rdf:type owl:Class ;
	rdfs:label "Document type"@en ;
	rdfs:comment "The type of a document being cited, for example: a standing order or a section of legislation."@en ;
	rdfs:isDefinedBy <http://parliament.uk/ontologies/procedure/> .
	
ppr:StepDisplayDepthInProcedure rdf:type owl:Class ;
	rdfs:label "Step display depth in procedure"@en ;
	rdfs:comment "The display depth of a business step in a procedure. There are occasions on which two business items actualising two different steps happen in the same work package on the same day: this class determines the display depth of those two business items. Because we capture dates rather than times of business items it is not possible to order business items in a way that makes ‘procedural sense’, for example: we may show 'procedure concluded' before an instrument has been approved. Step display depth exists in order to allow a number to be associated with a step in a procedure allowing us to order by the date of the business item, then by the display depth of the step in the procedure. Display depth in this context is not absolute across the procedure. A step with depth 8 may happen before a step with depth 7. The context of display depth is constrained to parts of a procedure map where procedure specifies that if X happens it must happen before Y but that Y may happen without X happening."@en ;
	rdfs:isDefinedBy <http://parliament.uk/ontologies/procedure/> .
	
ppr:RouteAvailability rdf:type owl:Class ;
	rdfs:label "Route availability"@en ;
	rdfs:comment "The availability of a route over time. A route may be open or closed. A route may reopen after being closed. The availability of a route may change as a result of a change to legislation, for example: routes in the procedure for proposed negative statutory instruments laid under Section 8 of the European Union (Withdrawal) Act 2018 will only remain open- as set out under the Act - until two years after completion day. The availability of a route may change as a result of a standing order being introduced, suspended or rescinded, for example: the standing orders setting out rules for English Votes for English Laws were first suspended, then rescinded. The availability of a route may change as a result of an order of a House in Parliament, for example: a formal proceeding may establish a new committee, creating a new route to a step for consideration by that committee."@en ;
	rdfs:isDefinedBy <http://parliament.uk/ontologies/procedure/> .
	
ppr:RouteAvailabilityStatus rdf:type owl:Class ;
	rdfs:label "Route availability status"@en ;
	rdfs:comment "The status of a route’s availability, being either open or closed."@en ;
	rdfs:isDefinedBy <http://parliament.uk/ontologies/procedure/> .

ppr:Legislature rdf:type owl:Class ;
	rdfs:label "Legislature"@en ;
	rdfs:comment "A legislature, being either the UK Parliament or a devolved legislature."@en ;
	rdfs:isDefinedBy <http://parliament.uk/ontologies/procedure/> .
	


#######  Object properties ##### 

ppr:formsPartOf rdf:type owl:ObjectProperty ;
	rdfs:label "Forms part of"@en ;
	rdfs:comment "Relates a business item to a work package it forms part of. One or more business items may form part of a work package. A business item may form part of one or more work packages, for example: a meeting of the Joint Committee on Statutory Instruments may consider one or more SIs, each SI being the focus of a separate work package."@en ;
	rdfs:domain ppr:BusinessItem ;
	rdfs:range ppr:WorkPackage ;
	rdfs:isDefinedBy <http://parliament.uk/ontologies/procedure/> .

ppr:subjectTo rdf:type owl:ObjectProperty ;
	rdfs:label "Subject to"@en ;
	rdfs:comment "Relates a work package to the procedure it is subject to. A work package is only subject to one procedure."@en ;
	rdfs:domain ppr:WorkPackage ;
	rdfs:range ppr:Procedure ;
	rdfs:isDefinedBy <http://parliament.uk/ontologies/procedure/> .
	
ppr:actualises rdf:type owl:ObjectProperty ;
	rdfs:label "Actualises"@en ;
	rdfs:comment "Relates a business item to a step in a procedure by means of a route. For example, relating the second reading of a public bill to the second reading step in the procedure. A step may be actualised by more than one business item in different work packages. A business item may actualise one or more steps. For example, a business item appearing in the Order Paper including a debate on several motions may actualise steps relating to each motion."@en ;
	rdfs:domain ppr:BusinessItem ;
	rdfs:range ppr:Step ;
	rdfs:isDefinedBy <http://parliament.uk/ontologies/procedure/> .

ppr:hasStepType rdf:type owl:ObjectProperty ;
	rdfs:label "Has step type"@en ;
	rdfs:comment "Relates a step to its type. A step may only be of one type. A step type may be related to one or more steps, or none."@en ;
	rdfs:domain ppr:Step ;
	rdfs:range ppr:StepType ;
	rdfs:isDefinedBy <http://parliament.uk/ontologies/procedure/> .

ppr:fromStep rdf:type owl:ObjectProperty ;
	rdfs:label "From step"@en ;
	rdfs:comment "Relates a route to its input step."@en ;
	rdfs:domain ppr:Route ;
	rdfs:range ppr:Step ;
	rdfs:isDefinedBy <http://parliament.uk/ontologies/procedure/> .
	
ppr:toStep rdf:type owl:ObjectProperty ;
	rdfs:label "To step"@en ;
	rdfs:comment "Relates a route to its output step."@en ;
	rdfs:domain ppr:Route ;
	rdfs:range ppr:Step ;
	rdfs:isDefinedBy <http://parliament.uk/ontologies/procedure/> .
	
ppr:followsRoute rdf:type owl:ObjectProperty ;
	rdfs:label "Follows route"@en ;
	rdfs:comment "Relates a procedure to a route. A route may appear in one or more procedures. For example, the route between 'Considered for English votes for English laws (EVEL) certification' to 'Certified as England only under the English votes for English laws (EVEL) process' appears in the draft negative, made negative, draft affirmative and made affirmative procedures."@en ;
	rdfs:domain ppr:Procedure ;
	rdfs:range ppr:Route ;
	rdfs:isDefinedBy <http://parliament.uk/ontologies/procedure/> .
	
ppr:stepInHouse rdf:type owl:ObjectProperty ;
	rdfs:label "Step in House"@en ;
	rdfs:comment "Relates a step to one or both Houses where such a relationship exists. A step may exist with no relationship to a House. For example, the making of a statutory instrument takes place outside of Parliament."@en ;
	rdfs:domain ppr:Step ;
	rdfs:range ppr:House ;
	rdfs:isDefinedBy <http://parliament.uk/ontologies/procedure/> .
	
ppr:stepInLegislature rdf:type owl:ObjectProperty ;
	rdfs:label "Step in legislature"@en ;
	rdfs:comment "Relates a step to the devolved legislature in which that step takes place, for example: a legislative consent motion being tabled in the Scottish Parliament."@en ;
	rdfs:domain ppr:Step ;
	rdfs:range ppr:Legislature ;
	rdfs:isDefinedBy <http://parliament.uk/ontologies/procedure/> .
	
ppr:inLegislature rdf:type owl:ObjectProperty ;
	rdfs:label "In legislature"@en ;
	rdfs:comment "Relates a House to the Legislature it forms part of. This is only used to relate the House of Commons and the House of Lords to the UK Parliament, devolved legislatures being unicameral."@en ;
	rdfs:domain ppr:House ;
	rdfs:range ppr:Legislature ;
	rdfs:isDefinedBy <http://parliament.uk/ontologies/procedure/> .
		
ppr:focus rdf:type owl:ObjectProperty ;
	rdfs:label "Focus"@en ;
	rdfs:comment "Relates a work package to its focus, this being a work packageable thing."@en ;
	rdfs:domain ppr:WorkPackage ;
	rdfs:range ppr:WorkPackageableThing ;
	rdfs:isDefinedBy <http://parliament.uk/ontologies/procedure/> .
	
ppr:hasMembership rdf:type owl:ObjectProperty ;
	rdfs:label "Has membership"@en ;
	rdfs:comment "Relates a step to the membership of that step in a step collection. A step collection membership is of one step. A step may have one or more step collection memberships, or none."@en ;
	rdfs:domain ppr:Step ;
	rdfs:range ppr:StepCollectionMembership ;
	rdfs:isDefinedBy <http://parliament.uk/ontologies/procedure/> .
	
ppr:ofStepCollection rdf:type owl:ObjectProperty ;
	rdfs:label "Of step collection"@en ;
	rdfs:comment "Relates a step collection membership to the collection it is part of. A step collection membership is part of one collection. A step collection may have one or more step collection memberships, or none."@en ;
	rdfs:domain ppr:StepCollectionMembership ;
	rdfs:range ppr:StepCollection ;
	rdfs:isDefinedBy <http://parliament.uk/ontologies/procedure/> .
	
ppr:hasProcedure rdf:type owl:ObjectProperty ;
	rdfs:label "Has procedure"@en ;
	rdfs:comment "Relates a step collection to a procedure. A step collection has one procedure, or none. A procedure may have one or more step collections, or none."@en ;
	rdfs:domain ppr:StepCollection ;
	rdfs:range ppr:Procedure ;
	rdfs:isDefinedBy <http://parliament.uk/ontologies/procedure/> .
	
ppr:stepCollectionInHouse rdf:type owl:ObjectProperty ;
	rdfs:label "Step collection in House"@en ;
	rdfs:comment "Relates a step collection to one House, or none. A House may have one or more step collections, or none."@en ;
	rdfs:domain ppr:StepCollection ;
	rdfs:range ppr:House ;
	rdfs:isDefinedBy <http://parliament.uk/ontologies/procedure/> .
	
ppr:stepHasCitation rdf:type owl:ObjectProperty ;
	rdfs:label "Step has citation"@en ;
	rdfs:comment "Relates a step to a citation. A step may have more than one citation, or none."@en ;
	rdfs:domain ppr:Step ;
	rdfs:range ppr:Citation ;
	rdfs:isDefinedBy <http://parliament.uk/ontologies/procedure/> .
	
ppr:routeHasCitation rdf:type owl:ObjectProperty ;
	rdfs:label "Route has citation"@en ;
	rdfs:comment "Relates a route to a citation. A route may have more than one citation, or none."@en ;
	rdfs:domain ppr:Route ;
	rdfs:range ppr:Citation ;
	rdfs:isDefinedBy <http://parliament.uk/ontologies/procedure/> .
	
ppr:procedureHasCitation rdf:type owl:ObjectProperty ;
	rdfs:label "Procedure has citation"@en ;
	rdfs:comment "Relates a procedure to a citation. A procedure may have more than one citation, or none."@en ;
	rdfs:domain ppr:Procedure ;
	rdfs:range ppr:Citation ;
	rdfs:isDefinedBy <http://parliament.uk/ontologies/procedure/> .
	
ppr:hasDocumentType rdf:type owl:ObjectProperty ;
	rdfs:label "Has document type"@en ;
	rdfs:comment "Relates a citation to the type of the document being cited."@en ;
	rdfs:domain ppr:Citation ;
	rdfs:range ppr:DocumentType ;
	rdfs:isDefinedBy <http://parliament.uk/ontologies/procedure/> .
	
ppr:forStep rdf:type owl:ObjectProperty ;
	rdfs:label "For step"@en ;
	rdfs:comment "Relates a step display depth in a procedure to a business step. A step display depth in a procedure is always related to one step. A step may have different step display depths in different procedures."@en ;
	rdfs:domain ppr:StepDisplayDepthInProcedure ;
	rdfs:range ppr:Step ;
	rdfs:isDefinedBy <http://parliament.uk/ontologies/procedure/> .
	
ppr:inProcedure rdf:type owl:ObjectProperty ;
	rdfs:label "In procedure"@en ;
	rdfs:comment "Relates a step display depth in a procedure to that procedure. A step display depth in a procedure is always related to one procedure. A procedure may have more than one step display depth for individual steps."@en ;
	rdfs:domain ppr:StepDisplayDepthInProcedure ;
	rdfs:range ppr:Procedure ;
	rdfs:isDefinedBy <http://parliament.uk/ontologies/procedure/> .
	
ppr:hasAvailability rdf:type owl:ObjectProperty ;
	rdfs:label "Has availability"@en ;
	rdfs:comment "Relates a route to its availability over a period of time. A route may have a different availability at different times, but only one availability at any one time. Routes with no defined availability are taken to be open."@en ;
	rdfs:domain ppr:Route ;
	rdfs:range ppr:RouteAvailability ;
	rdfs:isDefinedBy <http://parliament.uk/ontologies/procedure/> .
	
ppr:hasAvailabilityStatus rdf:type owl:ObjectProperty ;
	rdfs:label "Has availability status"@en ;
	rdfs:comment "Relates a route availability over a period of time to the status of that availability. A route availability has one route availability status."@en ;
	rdfs:domain ppr:RouteAvailability ;
	rdfs:range ppr:RouteAvailabilityStatus ;
	rdfs:isDefinedBy <http://parliament.uk/ontologies/procedure/> .
	
ppr:routeAvailabilityHasCitation rdf:type owl:ObjectProperty ;
	rdfs:label "Route availability has citation"@en ;
	rdfs:comment "Relates the availability of a route to a citation setting out that availability: this may be by means of a proceeding in Parliament, or by means of legislation. A route availability may have one or more citations, or none."@en ;
	rdfs:domain ppr:RouteAvailability ;
	rdfs:range ppr:Citation ;
	rdfs:isDefinedBy <http://parliament.uk/ontologies/procedure/> .
				
				

#######  Data properties ##### 

ppr:title rdf:type owl:DatatypeProperty ;
	rdfs:label "Title"@en ;
	rdfs:comment "Relates a citation to the title of the document being cited."@en ;
	rdfs:domain ppr:Citation ;
	rdfs:range rdf:langString ;
	rdfs:isDefinedBy <http://parliament.uk/ontologies/procedure/> .
	
ppr:uri rdf:type owl:DatatypeProperty ;
	rdfs:label "URI"@en ;
	rdfs:comment "Relates a citation to the URI of the document being cited."@en ;
	rdfs:domain ppr:Citation ;
	rdfs:range rdfs:Literal ;
	rdfs:isDefinedBy <http://parliament.uk/ontologies/procedure/> .
	
ppr:displayDepthValue rdf:type owl:DatatypeProperty ;
	rdfs:label "Display depth value"@en ;
	rdfs:comment "Relates a step display depth in a procedure to the depth value of the step in that procedure. The depth value is stored as a float in order to allow for the insertion of new steps into a procedure without having to renumber existing steps, for example: 1, 1.12, 2, 3."@en ;
	rdfs:domain ppr:StepDisplayDepthInProcedure ;
	rdfs:range xsd:float ;
	rdfs:isDefinedBy <http://parliament.uk/ontologies/procedure/> .