@prefix precr: <http://parliament.uk/ontologies/record-review/> . 
@prefix xsd: <http://www.w3.org/2001/XMLSchema#> . 
@prefix rdf: <http://www.w3.org/1999/02/22-rdf-syntax-ns#> .
@prefix dcterms: <http://purl.org/dc/terms/> .
@prefix owl:     <http://www.w3.org/2002/07/owl#> .
@prefix rdfs:    <http://www.w3.org/2000/01/rdf-schema#> .
@prefix foaf:	<http://xmlns.com/foaf/0.1/> .

<http://parliament.uk/ontologies/record-review/> 
    rdf:type owl:Ontology ;
    dcterms:title "Record reviews ontology"@en ;
    dcterms:created "2020-12-18"^^xsd:date ;
	dcterms:rights "Open Parliament Licence v3.0"@en ;
    dcterms:description "A model describing editorial reviews of records and actions taken following review."@en ;
	foaf:depiction <https://ukparliament.github.io/ontologies/record-review/record-review.png> ;
	foaf:maker
		[ foaf:name "Robert Brook"; foaf:homepage <https://robert-brook.com/> ],
		[ foaf:name "Michael Smethurst"; foaf:homepage <http://smethur.st/> ],
	    [ foaf:name "Anya Somerville" ] .


#######  Classes #####

precr:Work rdf:type owl:Class ;
	rdfs:label "Work"@en ;
	rdfs:comment "A distinct intellectual creation, similar to a work as defined in FRBR."@en ;
	rdfs:isDefinedBy <http://parliament.uk/ontologies/record-review/> .
	
precr:Manifestation rdf:type owl:Class ;
	rdfs:label "Manifestation"@en ;
	rdfs:comment "A manifestation of an expression of a work, allowing for multiple versions of an expression over time, for example: an edition of a book, or a remastered audio file of a podcast episode."@en ;
	rdfs:isDefinedBy <http://parliament.uk/ontologies/record-review/> .
	
precr:EditorialReview rdf:type owl:Class ;
	rdfs:subClassOf precr:EditorialAction ;
	rdfs:label "Editorial review"@en ;
	rdfs:comment "A review of a manifestation. A decision to review may be triggered by an external event, for example: a change in Government policy, the availability of new data, external work in the same area or the output of parliamentary business; a change in user needs, for example: a new type of enquiry; or a change to library policy or practice, for example: in presentation, citation style, method of acknowledgement, change of portfolio or change of specialist."@en ;
	rdfs:isDefinedBy <http://parliament.uk/ontologies/record-review/> .
	
precr:EditorialAction rdf:type owl:Class ;
	rdfs:label "Editorial action"@en ;
	rdfs:comment "An editorial action is an action taken on a manifestation or a work, for example: archiving a work, reviewing a manifestation, revising a manifestation or withdrawing a manifestation."@en ;
	rdfs:isDefinedBy <http://parliament.uk/ontologies/record-review/> .
	
precr:Archiving rdf:type owl:Class ;
	rdfs:subClassOf precr:EditorialAction ;
	rdfs:label "Archiving"@en ;
	rdfs:comment "The action of archiving a work, indicating that no further revisions are intended to take place. Manifestations of the work which have not been withdrawn remain available, marked with an indication that no further updates are anticipated."@en ;
	rdfs:isDefinedBy <http://parliament.uk/ontologies/record-review/> .
	
precr:Withdrawal rdf:type owl:Class ;
	rdfs:subClassOf precr:EditorialAction ;
	rdfs:label "Withdrawal"@en ;
	rdfs:comment "The action of withdrawing a manifestation. A manifestation may be withdrawn for a period and reinstated, or permanently withdrawn."@en ;
	rdfs:isDefinedBy <http://parliament.uk/ontologies/record-review/> .
	
precr:Revision rdf:type owl:Class ;
	rdfs:subClassOf precr:EditorialAction ;
	rdfs:label "Revision"@en ;
	rdfs:comment The action of revising a manifestation, resulting in a new manifestation.""@en ;
	rdfs:isDefinedBy <http://parliament.uk/ontologies/record-review/> .