@prefix precr: <http://parliament.uk/ontologies/record-review/> . 
@prefix xsd: <http://www.w3.org/2001/XMLSchema#> . 
@prefix rdf: <http://www.w3.org/1999/02/22-rdf-syntax-ns#> .
@prefix dcterms: <http://purl.org/dc/terms/> .
@prefix owl:     <http://www.w3.org/2002/07/owl#> .
@prefix rdfs:    <http://www.w3.org/2000/01/rdf-schema#> .
@prefix foaf:	<http://xmlns.com/foaf/0.1/> .

<http://parliament.uk/ontologies/record-review/> 
    rdf:type owl:Ontology ;
    dcterms:title "Record reviews ontology"@en ;
    dcterms:created "2020-12-18"^^xsd:date ;
	dcterms:rights "Open Parliament Licence v3.0"@en ;
    dcterms:description "A model describing editorial reviews of records and actions taken following review."@en ;
	foaf:depiction <https://ukparliament.github.io/ontologies/record-review/record-review.png> ;
	foaf:maker
		[ foaf:name "Robert Brook"; foaf:homepage <https://robert-brook.com/> ],
		[ foaf:name "Michael Smethurst"; foaf:homepage <http://smethur.st/> ],
	    [ foaf:name "Anya Somerville" ] .


#######  Classes #####

precr:Work rdf:type owl:Class ;
	rdfs:label "Work"@en ;
	rdfs:comment "A distinct intellectual creation, similar to a work as defined in FRBR."@en ;
	rdfs:isDefinedBy <http://parliament.uk/ontologies/record-review/> .
	
precr:Manifestation rdf:type owl:Class ;
	rdfs:label "Manifestation"@en ;
	rdfs:comment "A manifestation of an expression of a work, allowing for multiple versions of an expression over time, for example: an edition of a book, or a remastered audio file of a podcast episode."@en ;
	rdfs:isDefinedBy <http://parliament.uk/ontologies/record-review/> .
	
precr:EditorialReview rdf:type owl:Class ;
	rdfs:subClassOf precr:EditorialAction ;
	rdfs:label "Editorial review"@en ;
	rdfs:comment "A review of a manifestation. A decision to review may be triggered by an external event, for example: a change in Government policy, the availability of new data, external work in the same area or the output of parliamentary business; a change in user needs, for example: a new type of enquiry; or a change to library policy or practice, for example: in presentation, citation style, method of acknowledgement, change of portfolio or change of specialist."@en ;
	rdfs:isDefinedBy <http://parliament.uk/ontologies/record-review/> .
	
precr:EditorialAction rdf:type owl:Class ;
	rdfs:label "Editorial action"@en ;
	rdfs:comment "An editorial action is an action taken on a manifestation or a work, for example: archiving a work, reviewing a manifestation, revising a manifestation or withdrawing a manifestation."@en ;
	rdfs:isDefinedBy <http://parliament.uk/ontologies/record-review/> .
	
precr:Archiving rdf:type owl:Class ;
	rdfs:subClassOf precr:EditorialAction ;
	rdfs:label "Archiving"@en ;
	rdfs:comment "The action of archiving a work, indicating that no further revisions are intended to take place. Manifestations of the work which have not been withdrawn remain available, marked with an indication that no further updates are anticipated."@en ;
	rdfs:isDefinedBy <http://parliament.uk/ontologies/record-review/> .
	
precr:Withdrawal rdf:type owl:Class ;
	rdfs:subClassOf precr:EditorialAction ;
	rdfs:label "Withdrawal"@en ;
	rdfs:comment "The action of withdrawing a manifestation. A manifestation may be withdrawn for a period and reinstated, or permanently withdrawn."@en ;
	rdfs:isDefinedBy <http://parliament.uk/ontologies/record-review/> .
	
precr:Revision rdf:type owl:Class ;
	rdfs:subClassOf precr:EditorialAction ;
	rdfs:label "Revision"@en ;
	rdfs:comment "The action of revising an existing manifestation, resulting in a new manifestation. The existing manifestation remains unchanged."@en ;
	rdfs:isDefinedBy <http://parliament.uk/ontologies/record-review/> .
	
precr:ReviewCycle rdf:type owl:Class ;
	rdfs:label "Review cycle"@en ;
	rdfs:comment "A review cycle describes the period between reviews of a work."@en ;
	rdfs:isDefinedBy <http://parliament.uk/ontologies/record-review/> .
	
precr:Agent rdf:type owl:Class ;
	rdfs:label "Agent"@en ;
	rdfs:comment "Agents include people and groups, including those outside the Parliamentary Service, participating in parliamentary procedure and contributing to the wider work of Parliament."@en ;
	rdfs:isDefinedBy <http://parliament.uk/ontologies/record-review/> .
	
precr:Feedback rdf:type owl:Class ;
	rdfs:label "Feedback"@en ;
	rdfs:comment "Feedback on a record, provided in a submission. An instance of the feedback class may contain the text of the feedback, or a pointer to the substance of the feedback in a separate system."@en ;
	rdfs:isDefinedBy <http://parliament.uk/ontologies/record-review/> .
	
precr:RevisionType rdf:type owl:Class ;
	rdfs:label "Revision type"@en ;
	rdfs:comment "The type of a revision, for example: a major or minor edit."@en ;
	rdfs:isDefinedBy <http://parliament.uk/ontologies/record-review/> .

#######  Object properties ##### 

precr:leadsTo rdf:type owl:ObjectProperty ;
	rdfs:label "Leads to"@en ;
	rdfs:comment "Relates an editorial action to a resulting editorial action, for example: an editorial review leading to a revision of a manifestation."@en ;
	rdfs:domain precr:EditorialAction ;
	rdfs:range precr:EditorialAction ;
	rdfs:isDefinedBy <http://parliament.uk/ontologies/record-review/> .

precr:by rdf:type owl:ObjectProperty ;
	rdfs:label "By"@en ;
	rdfs:comment "Relates an editorial action to the person or group performing that action."@en ;
	rdfs:domain precr:EditorialAction ;
	rdfs:range precr:Agent ;
	rdfs:isDefinedBy <http://parliament.uk/ontologies/record-review/> .

precr:supersedes rdf:type owl:ObjectProperty ;
	rdfs:label "Supersedes"@en ;
	rdfs:comment "Relates a work to a work that supersedes it: used to point from an archived work to its replacement. A work may be superseded by more than one work. A work may supersede more than one work."@en ;
	rdfs:domain precr:Work ;
	rdfs:range precr:Work ;
	rdfs:isDefinedBy <http://parliament.uk/ontologies/record-review/> .
	
precr:archivingOf rdf:type owl:ObjectProperty ;
	rdfs:label "Archiving of"@en ;
	rdfs:comment "Relates an archiving action to the work being archived."@en ;
	rdfs:domain precr:Archiving ;
	rdfs:range precr:Work ;
	rdfs:isDefinedBy <http://parliament.uk/ontologies/record-review/> .
	
precr:hasReviewCycle rdf:type owl:ObjectProperty ;
	rdfs:label "Has review cycle"@en ;
	rdfs:comment "Relates a work to the review cycle of that work. A work has a single review cycle, or none."@en ;
	rdfs:domain precr:Work ;
	rdfs:range precr:ReviewCycle ;
	rdfs:isDefinedBy <http://parliament.uk/ontologies/record-review/> .
	
precr:resultsIn rdf:type owl:ObjectProperty ;
	rdfs:label "Results in"@en ;
	rdfs:comment "Relates a review cycle to resulting editorial reviews."@en ;
	rdfs:domain precr:ReviewCycle ;
	rdfs:range precr:EditorialReview ;
	rdfs:isDefinedBy <http://parliament.uk/ontologies/record-review/> .
	
precr:leadsToNew rdf:type owl:ObjectProperty ;
	rdfs:label "Leads to new"@en ;
	rdfs:comment "Relates an editorial review to the creation of a new work."@en ;
	rdfs:domain precr:EditorialReview ;
	rdfs:range precr:Work ;
	rdfs:isDefinedBy <http://parliament.uk/ontologies/record-review/> .
	
precr:withdrawnBy rdf:type owl:ObjectProperty ;
	rdfs:label "Withdrawn by"@en ;
	rdfs:comment "Relates a manifestation to the action of withdrawing that manifestation."@en ;
	rdfs:domain precr:Manifestation ;
	rdfs:range precr:Withdrawal ;
	rdfs:isDefinedBy <http://parliament.uk/ontologies/record-review/> .
	
precr:reviewOf rdf:type owl:ObjectProperty ;
	rdfs:label "Review of"@en ;
	rdfs:comment "Relates an editorial review to the manifestation being reviewed."@en ;
	rdfs:domain precr:EditorialReview ;
	rdfs:range precr:Manifestation ;
	rdfs:isDefinedBy <http://parliament.uk/ontologies/record-review/> .
	
precr:fromManifestation rdf:type owl:ObjectProperty ;
	rdfs:label "From manifestation"@en ;
	rdfs:comment "Relates an act of revision to an existing manifestation to be revised."@en ;
	rdfs:domain precr:Revision ;
	rdfs:range precr:Manifestation ;
	rdfs:isDefinedBy <http://parliament.uk/ontologies/record-review/> .

precr:toManifestation rdf:type owl:ObjectProperty ;
	rdfs:label "To manifestation"@en ;
	rdfs:comment "Relates an act of revision to a new manifestation resulting from the revision."@en ;
	rdfs:domain precr:Revision ;
	rdfs:range precr:Manifestation ;
	rdfs:isDefinedBy <http://parliament.uk/ontologies/record-review/> .
	
precr:submits rdf:type owl:ObjectProperty ;
	rdfs:label "Makes"@en ;
	rdfs:comment "Relates an agent to the feedback submitted by that agent."@en ;
	rdfs:domain precr:Agent ;
	rdfs:range precr:Feedback ;
	rdfs:isDefinedBy <http://parliament.uk/ontologies/record-review/> .

precr:feedbackLeadsTo rdf:type owl:ObjectProperty ;
	rdfs:label "Feedback leads to"@en ;
	rdfs:comment "Relates feedback to a resulting editorial review. An editorial review may be triggered by one or more items of feedback. The acceptance of feedback does not necessitate an editorial review. Feedback may result in more than one editorial review, or none."@en ;
	rdfs:domain precr:Feedback ;
	rdfs:range precr:EditorialReview ;
	rdfs:isDefinedBy <http://parliament.uk/ontologies/record-review/> .

precr:hasRevisionType rdf:type owl:ObjectProperty ;
	rdfs:label "Has revision type"@en ;
	rdfs:comment "Relates an action of revision to the type of that revision."@en ;
	rdfs:domain precr:Revision ;
	rdfs:range precr:RevisionType ;
	rdfs:isDefinedBy <http://parliament.uk/ontologies/record-review/> .
	
	
											### edited to here

				
	
##### Data properties ####	
	
precr:at rdf:type owl:DatatypeProperty ;
	rdfs:label "At"@en ;
	rdfs:comment ""@en ;
	rdfs:domain precr:EditorialAction ;
	rdfs:range xsd:dateTime ;
	rdfs:isDefinedBy <http://parliament.uk/ontologies/record-review/> .
	
precr:reinstatedAt rdf:type owl:DatatypeProperty ;
	rdfs:label "Reinstated at"@en ;
	rdfs:comment ""@en ;
	rdfs:domain precr:Withdrawal ;
	rdfs:range xsd:dateTime ;
	rdfs:isDefinedBy <http://parliament.uk/ontologies/record-review/> .
	
precr:publishedAt rdf:type owl:DatatypeProperty ;
	rdfs:label "Published at"@en ;
	rdfs:comment ""@en ;
	rdfs:domain precr:Manifestation ;
	rdfs:range xsd:dateTime ;
	rdfs:isDefinedBy <http://parliament.uk/ontologies/record-review/> .
	
precr:reviewedOn rdf:type owl:DatatypeProperty ;
	rdfs:label "Reviewed on"@en ;
	rdfs:comment ""@en ;
	rdfs:domain precr:EditorialReview ;
	rdfs:range xsd:date ;
	rdfs:isDefinedBy <http://parliament.uk/ontologies/record-review/> .
	
precr:receivedAt rdf:type owl:DatatypeProperty ;
	rdfs:label "Received at"@en ;
	rdfs:comment ""@en ;
	rdfs:domain precr:Feedback ;
	rdfs:range xsd:dateTime ;
	rdfs:isDefinedBy <http://parliament.uk/ontologies/record-review/> .
	
precr:feedbackText rdf:type owl:DatatypeProperty ;
	rdfs:label "Feedback text"@en ;
	rdfs:comment ""@en ;
	rdfs:domain precr:Feedback ;
	rdfs:range rdf:langString ;
	rdfs:isDefinedBy <http://parliament.uk/ontologies/record-review/> .
	
precr:hasRevisionDescription rdf:type owl:DatatypeProperty ;
	rdfs:label "Has revision description"@en ;
	rdfs:comment ""@en ;
	rdfs:domain precr:Revision ;
	rdfs:range rdf:langString ;
	rdfs:isDefinedBy <http://parliament.uk/ontologies/record-review/> .
	
precr:hasRevisionTypeDescription rdf:type owl:DatatypeProperty ;
	rdfs:label "Has revision type description"@en ;
	rdfs:comment ""@en ;
	rdfs:domain precr:RevisionType ;
	rdfs:range rdf:langString ;
	rdfs:isDefinedBy <http://parliament.uk/ontologies/record-review/> .